Hybrid/Semantics.v
@@ -7,7 +7,7 @@ Require Import PPermutLib.
 Require Import OkLib.
 Require Import EmptyEquivLib.
 
-Open Scope label_free_is5_scope.
+Open Scope hybrid_is5_scope.
 Open Scope is5_scope.
 Open Scope permut_scope.
 
@@ -22,81 +22,81 @@ Global Reserved Notation " G '|=' Ctx '|-' M ':::' A " (at level 70).
    For each full context (that is, context and background), we require
    that the variables - both for terms and worlds - are unique.
 *)
-Inductive types_LF: Background_LF -> Context_LF -> te_LF -> ty -> Prop :=
+Inductive types_Hyb: bg_Hyb -> ctx_Hyb -> te_Hyb -> ty -> Prop :=
 
-| t_hyp_LF: forall A G w (Gamma: list (prod var ty)) v
-  (Ok_Bg: ok_Bg ((w, Gamma) :: G))
+| t_hyp_Hyb: forall A G w (Gamma: list (prod var ty)) v
+  (Ok_Bg: ok_Bg_Hyb ((w, Gamma) :: G))
   (HT: Mem (v, A) Gamma),
-  G |= (w, Gamma) |- hyp_LF (fte v) ::: A
+  G |= (w, Gamma) |- hyp_Hyb (fte v) ::: A
 
-| t_lam_LF: forall L A B G w Gamma M
-  (Ok_Bg: ok_Bg ((w, Gamma) :: G))
+| t_lam_Hyb: forall L A B G w Gamma M
+  (Ok_Bg: ok_Bg_Hyb ((w, Gamma) :: G))
   (HT: forall v', v' \notin L ->
-    G |= (w, (v', A) :: Gamma) |- M ^t^ (hyp_LF (fte v')) ::: B),
-  G |= (w, Gamma) |- (lam_LF A M) ::: A ---> B
+    G |= (w, (v', A) :: Gamma) |- M ^t^ (hyp_Hyb (fte v')) ::: B),
+  G |= (w, Gamma) |- (lam_Hyb A M) ::: A ---> B
 
-| t_appl_LF: forall A B G w Gamma M N
-  (Ok_Bg: ok_Bg ((w, Gamma) :: G))
+| t_appl_Hyb: forall A B G w Gamma M N
+  (Ok_Bg: ok_Bg_Hyb ((w, Gamma) :: G))
   (HT1: G |= (w, Gamma) |- M ::: A ---> B)
   (HT2: G |= (w, Gamma) |- N ::: A),
-  G |= (w, Gamma) |- (appl_LF M N) ::: B
+  G |= (w, Gamma) |- (appl_Hyb M N) ::: B
 
-| t_box_LF: forall L A G w Gamma M
-  (Ok_Bg: ok_Bg (G & (w, Gamma)))
+| t_box_Hyb: forall L A G w Gamma M
+  (Ok_Bg: ok_Bg_Hyb (G & (w, Gamma)))
   (HT: forall w', w' \notin L ->
     G & (w, Gamma) |= (w', nil) |- M ^w^ (fwo w') ::: A),
-  G |= (w, Gamma) |- box_LF M ::: [*] A
+  G |= (w, Gamma) |- box_Hyb M ::: [*] A
 
-| t_unbox_LF: forall A G w Gamma M
-  (Ok_Bg: ok_Bg ((w, Gamma) :: G))
+| t_unbox_Hyb: forall A G w Gamma M
+  (Ok_Bg: ok_Bg_Hyb ((w, Gamma) :: G))
   (HT: G |= (w, Gamma) |- M ::: [*] A),
-  G |= (w, Gamma) |- unbox_fetch_LF (fwo w) M ::: A
+  G |= (w, Gamma) |- unbox_fetch_Hyb (fwo w) M ::: A
 
-| t_unbox_fetch_LF: forall A G w Gamma w' Gamma' M
-  (Ok_Bg: ok_Bg ((w, Gamma) :: G & (w', Gamma')))
+| t_unbox_fetch_Hyb: forall A G w Gamma w' Gamma' M
+  (Ok_Bg: ok_Bg_Hyb ((w, Gamma) :: G & (w', Gamma')))
   (HT: (G & (w', Gamma')) |= (w, Gamma) |- M ::: [*] A),
   forall G', (G & (w, Gamma)) ~=~ G' ->
-    G' |= (w', Gamma') |- unbox_fetch_LF (fwo w) M ::: A
+    G' |= (w', Gamma') |- unbox_fetch_Hyb (fwo w) M ::: A
 
-| t_here_LF: forall A G w Gamma M
-  (Ok_Bg: ok_Bg ((w, Gamma) :: G))
+| t_here_Hyb: forall A G w Gamma M
+  (Ok_Bg: ok_Bg_Hyb ((w, Gamma) :: G))
   (HT: G |= (w, Gamma) |- M ::: A),
-  G |= (w, Gamma) |- get_here_LF (fwo w) M ::: <*> A
+  G |= (w, Gamma) |- get_here_Hyb (fwo w) M ::: <*> A
 
-| t_get_here_LF: forall A G w Gamma w' Gamma' M
-  (Ok_Bg: ok_Bg ((w, Gamma) :: G & (w', Gamma')))
+| t_get_here_Hyb: forall A G w Gamma w' Gamma' M
+  (Ok_Bg: ok_Bg_Hyb ((w, Gamma) :: G & (w', Gamma')))
   (HT: G & (w', Gamma') |= (w, Gamma) |- M ::: A),
   forall G', (G & (w, Gamma)) ~=~ G' ->
-    G' |= (w', Gamma') |- get_here_LF (fwo w) M ::: <*> A
+    G' |= (w', Gamma') |- get_here_Hyb (fwo w) M ::: <*> A
 
-| t_letdia_LF: forall L_w L_t A B G w Gamma M N
-  (Ok_Bg: ok_Bg ((w, Gamma) :: G))
+| t_letdia_Hyb: forall L_w L_t A B G w Gamma M N
+  (Ok_Bg: ok_Bg_Hyb ((w, Gamma) :: G))
   (HT1: G |= (w, Gamma) |- M ::: <*> A)
   (HT2: forall v', v' \notin L_t -> forall w', w' \notin L_w ->
     (w', (v', A) :: nil) :: G |=
-      (w, Gamma) |- (N ^w^ (fwo w')) ^t^ (hyp_LF (fte v')) ::: B),
-  G |= (w, Gamma) |- letdia_get_LF (fwo w) M N ::: B
+      (w, Gamma) |- (N ^w^ (fwo w')) ^t^ (hyp_Hyb (fte v')) ::: B),
+  G |= (w, Gamma) |- letdia_get_Hyb (fwo w) M N ::: B
 
-| t_letdia_get_LF: forall L_w L_t A B G w (Gamma: list (prod var ty)) Ctx' M N
-  (Ok_Bg: ok_Bg ((w, Gamma) :: G & Ctx'))
+| t_letdia_get_Hyb: forall L_w L_t A B G w (Gamma: list (prod var ty)) Ctx' M N
+  (Ok_Bg: ok_Bg_Hyb ((w, Gamma) :: G & Ctx'))
   (HT1: G & Ctx' |= (w, Gamma) |- M ::: <*> A)
   (HT2: forall v', v' \notin L_t -> forall w', w' \notin L_w ->
     (w', ((v', A) :: nil)) :: G & (w, Gamma) |=
-      Ctx' |- (N ^w^ (fwo w')) ^t^ (hyp_LF (fte v')) ::: B),
+      Ctx' |- (N ^w^ (fwo w')) ^t^ (hyp_Hyb (fte v')) ::: B),
   forall G0, (G & (w, Gamma)) ~=~ G0 ->
-    G0 |= Ctx' |- letdia_get_LF (fwo w) M N ::: B
+    G0 |= Ctx' |- letdia_get_Hyb (fwo w) M N ::: B
 
-where " G '|=' Ctx '|-' M ':::' A " := (types_LF G Ctx M A)
-  : label_free_is5_scope.
+where " G '|=' Ctx '|-' M ':::' A " := (types_Hyb G Ctx M A)
+  : hybrid_is5_scope.
 
 
 (*** Definitions ::: Dynamics ***)
 
 
-Inductive value_LF: te_LF -> Prop :=
-| val_lam_LF: forall A M, value_LF (lam_LF A M)
-| val_box_LF: forall M, value_LF (box_LF M)
-| val_get_here_LF: forall M Ctx, value_LF M -> value_LF (get_here_LF Ctx M)
+Inductive value_Hyb: te_Hyb -> Prop :=
+| val_lam_Hyb: forall A M, value_Hyb (lam_Hyb A M)
+| val_box_Hyb: forall M, value_Hyb (box_Hyb M)
+| val_get_here_Hyb: forall M Ctx, value_Hyb M -> value_Hyb (get_here_Hyb Ctx M)
 .
 
 
@@ -106,60 +106,55 @@ Global Reserved Notation " M |-> N " (at level 70).
    In order to define a step of reduction we require that certain terms
    are locally closed.
 *)
-Inductive step_LF: (te_LF * vwo) -> (te_LF * vwo) -> Prop :=
-| red_appl_lam_LF: forall ctx M A N,
-  lc_w_LF M ->
-  lc_t_n_LF 1 M -> (* or (forall x, x \notin L -> lc_t_LF (M ^t^ (fte x))) -> *)
-  lc_w_LF N -> lc_t_LF N ->
-  (appl_LF (lam_LF A M) N, ctx) |-> ( M ^t^ N , ctx)
+Inductive step_Hyb: (te_Hyb * vwo) -> (te_Hyb * vwo) -> Prop :=
+| red_appl_lam_Hyb: forall ctx M A N,
+  lc_w_Hyb M ->
+  lc_t_n_Hyb 1 M ->
+  lc_w_Hyb N -> lc_t_Hyb N ->
+  (appl_Hyb (lam_Hyb A M) N, ctx) |-> ( M ^t^ N , ctx)
 
-| red_unbox_fetch_box_LF: forall ctx ctx' M,
-   lc_w_n_LF 1 M -> (* or
-     (forall x, x \notin L -> lc_w_LF (M ^w^ (fwo x))) -> *)
-  lc_t_LF M ->
-  (unbox_fetch_LF ctx' (box_LF M), ctx) |-> (M ^w^ ctx, ctx)
+| red_unbox_fetch_box_Hyb: forall ctx ctx' M,
+   lc_w_n_Hyb 1 M ->
+  lc_t_Hyb M ->
+  (unbox_fetch_Hyb ctx' (box_Hyb M), ctx) |-> (M ^w^ ctx, ctx)
 
-| red_letdia_get_get_here_LF: forall ctx ctx' ctx'' M N,
-  lc_w_LF M -> lc_t_LF M ->
-  lc_w_n_LF 1 N -> (* or
-     (forall x, x \notin L_w -> lc_w_LF (N ^w^ (fwo x))) -> *)
-  lc_t_n_LF 1 N -> (* or
-     (forall x, x \notin L_t -> lc_t_LF (N ^t^ (fte x))) -> *)
-  (letdia_get_LF ctx' (get_here_LF ctx'' M) N, ctx) |->
+| red_letdia_get_get_here_Hyb: forall ctx ctx' ctx'' M N,
+  lc_w_Hyb M -> lc_t_Hyb M ->
+  lc_w_n_Hyb 1 N ->
+  lc_t_n_Hyb 1 N ->
+  (letdia_get_Hyb ctx' (get_here_Hyb ctx'' M) N, ctx) |->
     ((N ^w^ ctx'') ^t^ M, ctx)
 
-| red_appl_LF: forall ctx M N M'
+| red_appl_Hyb: forall ctx M N M'
   (HT: (M, ctx) |-> (M', ctx)),
-  lc_w_LF M -> lc_t_LF M ->
-  lc_w_LF N -> lc_t_LF N ->
-  (appl_LF M N, ctx) |-> (appl_LF M' N, ctx)
+  lc_w_Hyb M -> lc_t_Hyb M ->
+  lc_w_Hyb N -> lc_t_Hyb N ->
+  (appl_Hyb M N, ctx) |-> (appl_Hyb M' N, ctx)
 
-| red_unbox_fetch_LF: forall ctx' M M' ctx
+| red_unbox_fetch_Hyb: forall ctx' M M' ctx
   (HT: (M, ctx') |-> (M', ctx')),
-  lc_w_LF M -> lc_t_LF M ->
-  (unbox_fetch_LF ctx' M, ctx) |-> (unbox_fetch_LF ctx' M', ctx)
+  lc_w_Hyb M -> lc_t_Hyb M ->
+  (unbox_fetch_Hyb ctx' M, ctx) |-> (unbox_fetch_Hyb ctx' M', ctx)
 
-| red_get_here_LF: forall ctx ctx' M M'
+| red_get_here_Hyb: forall ctx ctx' M M'
   (HT: (M, ctx) |-> (M', ctx)),
-  lc_w_LF M -> lc_t_LF M ->
-  (get_here_LF ctx M, ctx') |-> (get_here_LF ctx M', ctx')
+  lc_w_Hyb M -> lc_t_Hyb M ->
+  (get_here_Hyb ctx M, ctx') |-> (get_here_Hyb ctx M', ctx')
 
-| red_letdia_get_LF: forall ctx ctx' M N M'
+| red_letdia_get_Hyb: forall ctx ctx' M N M'
   (HT: (M, ctx) |-> (M', ctx)),
-  lc_w_LF M -> lc_t_LF M ->
-  lc_w_n_LF 1 N -> (* or
-     (forall x, x \notin L_w -> lc_w_LF (N ^w^ (fwo x))) -> *)
-  lc_t_n_LF 1 N -> (* or
-     (forall x, x \notin L_t -> lc_t_LF (N ^t^ (fte x))) -> *)
-  (letdia_get_LF ctx M N, ctx') |-> (letdia_get_LF ctx M' N, ctx')
+  lc_w_Hyb M -> lc_t_Hyb M ->
+  lc_w_n_Hyb 1 N ->
+  lc_t_n_Hyb 1 N ->
+  (letdia_get_Hyb ctx M N, ctx') |-> (letdia_get_Hyb ctx M' N, ctx')
 
-where " M |-> N " := (step_LF M N ) : label_free_is5_scope.
+where " M |-> N " := (step_Hyb M N ) : hybrid_is5_scope.
 
-Inductive steps_LF : te_LF * vwo -> te_LF * vwo -> Prop :=
-| single_step_LF: forall M M' w, (M, w) |-> (M', w) -> steps_LF (M, w) (M', w)
-| multi_step_LF: forall M M' M'' w,
-  (M, w) |-> (M', w) -> steps_LF (M', w) (M'', w)
-  -> steps_LF (M, w) (M'', w)
+Inductive steps_Hyb : te_Hyb * vwo -> te_Hyb * vwo -> Prop :=
+| single_step_Hyb: forall M M' w, (M, w) |-> (M', w) -> steps_Hyb (M, w) (M', w)
+| multi_step_Hyb: forall M M' M'' w,
+  (M, w) |-> (M', w) -> steps_Hyb (M', w) (M'', w)
+  -> steps_Hyb (M, w) (M'', w)
 .
 
 
@@ -177,11 +172,11 @@ Inductive steps_LF : te_LF * vwo -> te_LF * vwo -> Prop :=
 *)
 
 (* Proof: simple induction on typing rules *)
-Lemma BackgroundSubsetImpl:
+Lemma BackgroundSubsetImpl_Hyb:
 forall G G' Ctx M A
   (HT: G |= Ctx |- M ::: A)
   (HSubst: exists GT, (G++GT) ~=~ G')
-  (H_ok: ok_Bg (Ctx :: G')),
+  (H_ok: ok_Bg_Hyb (Ctx :: G')),
   G' |= Ctx |- M ::: A.
 intros;
 generalize dependent G';
@@ -189,63 +184,63 @@ induction HT; intros.
 (* hyp *)
 constructor; auto.
 (* lam *)
-apply t_lam_LF with (L:=L \u used_t_vars ((w, Gamma)::G'));
+apply t_lam_Hyb with (L:=L \u used_t_vars_Hyb ((w, Gamma)::G'));
 [assumption | intros; eapply H; auto].
 (* appl *)
 econstructor; auto.
 (* box *)
 destruct HSubst as [GT];
-apply t_box_LF with (L:=L \u used_w_vars (G' & (w, Gamma))); intros;
-[ apply ok_Bg_cons_last |
-  apply H; [ | exists GT | ] ]; auto; try PPermut_simpl;
-eapply ok_Bg_fresh_wo;
-[ apply ok_Bg_cons_last |
+apply t_box_Hyb with (L:=L \u used_w_vars_Hyb (G' & (w, Gamma))); intros;
+[ apply ok_Bg_Hyb_cons_last |
+  apply H; [ | exists GT | ] ]; auto; try PPermut_Hyb_simpl;
+eapply ok_Bg_Hyb_fresh_wo;
+[ apply ok_Bg_Hyb_cons_last |
   rewrite notin_union in H1; destruct H1]; auto.
 (* unbox *)
 constructor; auto.
 (* unbox_fetch *)
 destruct HSubst as [GT];
-apply t_unbox_fetch_LF with (Gamma:=Gamma) (G:=G++GT).
-apply ok_Bg_ppermut with (G:=(w', Gamma')::G'0);
+apply t_unbox_fetch_Hyb with (Gamma:=Gamma) (G:=G++GT).
+apply ok_Bg_Hyb_ppermut with (G:=(w', Gamma')::G'0);
   [rewrite <- H0; rewrite <- H; rew_app | ]; auto.
-apply IHHT; [exists GT | ]; auto; try PPermut_simpl.
-apply ok_Bg_ppermut with (G:=(w', Gamma')::G'0); auto.
+apply IHHT; [exists GT | ]; auto; try PPermut_Hyb_simpl.
+apply ok_Bg_Hyb_ppermut with (G:=(w', Gamma')::G'0); auto.
 rewrite <- H0; rewrite <- H; rew_app; auto.
-transitivity (G' ++ GT); PPermut_simpl; auto.
+transitivity (G' ++ GT); PPermut_Hyb_simpl; auto.
 (* here *)
 constructor; auto.
 (* get_here *)
 destruct HSubst as [GT];
-apply t_get_here_LF with (Gamma:=Gamma) (G:=G++GT).
-apply ok_Bg_ppermut with (G:=(w', Gamma')::G'0);
+apply t_get_here_Hyb with (Gamma:=Gamma) (G:=G++GT).
+apply ok_Bg_Hyb_ppermut with (G:=(w', Gamma')::G'0);
   [rewrite <- H0; rewrite <- H; rew_app | ]; auto.
-apply IHHT; [exists GT | ]; auto; try PPermut_simpl;
-  apply ok_Bg_ppermut with (G:=(w', Gamma')::G'0); auto;
+apply IHHT; [exists GT | ]; auto; try PPermut_Hyb_simpl;
+  apply ok_Bg_Hyb_ppermut with (G:=(w', Gamma')::G'0); auto;
   rewrite <- H0; rewrite <- H; rew_app; auto.
 rewrite <- H0; rewrite <- H; rew_app; auto.
 (* letdia *)
-apply t_letdia_LF with (A:=A) (L_t:=L_t \u used_t_vars ((w, Gamma) :: G'))
-  (L_w:=L_w \u used_w_vars ((w, Gamma)::G'));
+apply t_letdia_Hyb with (A:=A) (L_t:=L_t \u used_t_vars_Hyb ((w, Gamma) :: G'))
+  (L_w:=L_w \u used_w_vars_Hyb ((w, Gamma)::G'));
 [  | | intros; apply H]; auto;
 destruct HSubst as [GT];
 [ exists GT; rew_app; auto |
   rewrite notin_union in *; destruct H1; destruct H0];
-apply ok_Bg_ppermut with (G:= (w', (v', A) :: nil ) :: (w, Gamma) :: G');
-[ | apply ok_Bg_fresh_wo_te]; auto.
+apply ok_Bg_Hyb_ppermut with (G:= (w', (v', A) :: nil ) :: (w, Gamma) :: G');
+[ | apply ok_Bg_Hyb_fresh_wo_te]; auto.
 (* letdia_get *)
 destruct HSubst as [GT];
-apply t_letdia_get_LF with (A:=A) (Gamma:=Gamma) (G:=G++GT)
-                           (L_t:=L_t \u used_t_vars (Ctx'::G'))
-                           (L_w:=L_w \u used_w_vars (Ctx'::G')).
-apply ok_Bg_ppermut with (G:=Ctx' :: G');
+apply t_letdia_get_Hyb with (A:=A) (Gamma:=Gamma) (G:=G++GT)
+                           (L_t:=L_t \u used_t_vars_Hyb (Ctx'::G'))
+                           (L_w:=L_w \u used_w_vars_Hyb (Ctx'::G')).
+apply ok_Bg_Hyb_ppermut with (G:=Ctx' :: G');
   [rewrite <- H1; rewrite <- H0; rew_app | ]; auto.
 apply IHHT.
   exists GT; rew_app; auto.
-  apply ok_Bg_ppermut with (G:=Ctx' :: G');
+  apply ok_Bg_Hyb_ppermut with (G:=Ctx' :: G');
   [ rewrite <- H1; rewrite <- H0; rew_app | ]; auto.
   intros; apply H; auto.
   exists GT; rew_app; auto.
-  apply ok_Bg_ppermut with (G:=(w', (v', A) :: nil) :: Ctx' :: G'); auto;
+  apply ok_Bg_Hyb_ppermut with (G:=(w', (v', A) :: nil) :: Ctx' :: G'); auto;
   rewrite <- H1; rewrite <- H0;
   assert ((G & (w, Gamma) ++ GT)  ~=~ (G ++ GT) & (w, Gamma))
     by (symmetry; rew_app; auto);
@@ -255,38 +250,38 @@ Qed.
 
 
 (*
-   Proof: using BackgroundSubsetImpl with some tweaks to remove ok_Bg from
+   Proof: using BackgroundSubsetImpl with some tweaks to remove ok_Bg_Hyb from
    assumptions.
 *)
-Lemma PPermut_bg:
+Lemma PPermut_Hyb_bg:
 forall G Gamma w M A,
   G |= (w, Gamma) |- M ::: A ->
     forall G',
       G ~=~ G' ->
       G' |= (w, Gamma) |- M ::: A.
-intros; apply BackgroundSubsetImpl with (G:=G);
-[ | exists (@nil Context_LF) | ]; rew_app; auto;
+intros; apply BackgroundSubsetImpl_Hyb with (G:=G);
+[ | exists (@nil ctx_Hyb) | ]; rew_app; auto;
 inversion H; subst;
-try (apply ok_Bg_ppermut with (G:=(w, Gamma) :: G); auto);
-apply ok_Bg_cons_last; auto;
+try (apply ok_Bg_Hyb_ppermut with (G:=(w, Gamma) :: G); auto);
+apply ok_Bg_Hyb_cons_last; auto;
 rewrite <- H6 || rewrite <- H1;
-apply ok_Bg_ppermut with (G:=(w0, Gamma0) :: G0 & (w, Gamma)); eauto.
+apply ok_Bg_Hyb_ppermut with (G:=(w0, Gamma0) :: G0 & (w, Gamma)); eauto.
 Qed.
 
 
 (*
-   Adding types_LF as morphism for PPermut will allow us to simply rewrite
-   PPermutations of backgrounds.
+   Adding types_Hyb as morphism for PPermut_Hyb will allow us to simply rewrite
+   PPermut_Hybations of backgrounds.
 *)
-Add Morphism types_LF : PPermut_types.
+Add Morphism types_Hyb : PPermut_Hyb_types.
 split; intros; destruct y0;
-[ apply PPermut_bg with (G:=x) |
-  apply PPermut_bg with (G:=y) ]; auto.
+[ apply PPermut_Hyb_bg with (G:=x) |
+  apply PPermut_Hyb_bg with (G:=y) ]; auto.
 Qed.
 
 
 (* Proof: Simple induction on typing rules *)
-Lemma ContextPermutImpl:
+Lemma ContextPermutImpl_Hyb:
 forall G Gamma Gamma' w M A
   (HPerm: Gamma *=* Gamma')
   (HT: G |= (w, Gamma) |- M ::: A),
@@ -297,35 +292,35 @@ induction HT;
 intros; simpl in *; try (inversion HeqCtx; subst).
 (* hyp *)
 constructor;
-[ eapply ok_Bg_permut |
+[ eapply ok_Bg_Hyb_permut |
   eapply Mem_permut]; eauto.
 (* lam *)
-econstructor; [ eapply ok_Bg_permut | ]; eauto.
+econstructor; [ eapply ok_Bg_Hyb_permut | ]; eauto.
 (* appl *)
-econstructor; [ eapply ok_Bg_permut | | ]; eauto.
+econstructor; [ eapply ok_Bg_Hyb_permut | | ]; eauto.
 (* box *)
-econstructor; [ eapply ok_Bg_permut_last | intros]; eauto;
+econstructor; [ eapply ok_Bg_Hyb_permut_last | intros]; eauto;
 assert (G & (w, Gamma') ~=~ G & (w, Gamma0)) by auto;
 rewrite H1; apply HT; eauto.
 (* unbox *)
-econstructor; [ eapply ok_Bg_permut | ]; eauto.
+econstructor; [ eapply ok_Bg_Hyb_permut | ]; eauto.
 (* unbox_fetch *)
-apply t_unbox_fetch_LF with (G:=G) (Gamma:=Gamma); auto.
-apply ok_Bg_ppermut with (G:=(w0, Gamma) :: G & (w, Gamma0)); auto.
+apply t_unbox_fetch_Hyb with (G:=G) (Gamma:=Gamma); auto.
+apply ok_Bg_Hyb_ppermut with (G:=(w0, Gamma) :: G & (w, Gamma0)); auto.
 assert (G & (w, Gamma'0) ~=~ (G & (w, Gamma0))) as H0 by auto;
 rewrite H0; auto.
 (* here *)
-econstructor; [ eapply ok_Bg_permut | ]; eauto.
+econstructor; [ eapply ok_Bg_Hyb_permut | ]; eauto.
 (* get_here *)
-apply t_get_here_LF with (G:=G) (Gamma:=Gamma); auto.
-apply ok_Bg_ppermut with (G:=(w0, Gamma) :: G & (w, Gamma0)); auto.
+apply t_get_here_Hyb with (G:=G) (Gamma:=Gamma); auto.
+apply ok_Bg_Hyb_ppermut with (G:=(w0, Gamma) :: G & (w, Gamma0)); auto.
 assert (G & (w, Gamma'0) ~=~ (G & (w, Gamma0))) as H1 by auto;
 rewrite H1; auto.
 (* letdia *)
-econstructor; [ eapply ok_Bg_permut | | ]; eauto.
+econstructor; [ eapply ok_Bg_Hyb_permut | | ]; eauto.
 (* letdia_get *)
-apply t_letdia_get_LF with (L_w:=L_w) (L_t:=L_t) (A:=A) (Gamma:=Gamma) (G:=G).
-apply ok_Bg_ppermut with (G:=(w0, Gamma) :: G & (w, Gamma0)); auto.
+apply t_letdia_get_Hyb with (L_w:=L_w) (L_t:=L_t) (A:=A) (Gamma:=Gamma) (G:=G).
+apply ok_Bg_Hyb_ppermut with (G:=(w0, Gamma) :: G & (w, Gamma0)); auto.
 assert (G & (w, Gamma') ~=~ (G & (w, Gamma0))) as H2 by auto;
 rewrite H2; auto.
 intros; eapply H; eauto.
@@ -335,13 +330,13 @@ Qed.
 
 (* Weakening lemmas *)
 
-Lemma GlobalWeakening:
+Lemma GlobalWeakening_Hyb:
 forall G G' Ctx Ctx' M A
   (HT: G ++ G' |= Ctx |- M ::: A)
-  (H_ok: ok_Bg (Ctx :: G & Ctx' ++ G')),
+  (H_ok: ok_Bg_Hyb (Ctx :: G & Ctx' ++ G')),
   G & Ctx' ++ G' |= Ctx |- M ::: A.
 intros; rew_app;
-apply BackgroundSubsetImpl with (G:=G++G'); auto;
+apply BackgroundSubsetImpl_Hyb with (G:=G++G'); auto;
 [ exists (Ctx'::nil); rew_app; symmetry |
   rew_app in *]; auto.
 Qed.
@@ -355,15 +350,15 @@ Proof: induction on typing
   * otherwise we have to deconstruct background in order to extract the context
   that we want to switch
 *)
-Lemma Weakening_general:
+Lemma Weakening_general_Hyb:
   forall G w Gamma M A
   (HT: G |= (w, Gamma) |- M ::: A),
   (forall G' w' Delta Delta',
     G ~=~ (G' & (w', Delta)) ->
-    ok_Bg ((w, Gamma) :: G' & (w', Delta ++ Delta')) ->
+    ok_Bg_Hyb ((w, Gamma) :: G' & (w', Delta ++ Delta')) ->
     G' & (w', Delta ++ Delta') |= (w, Gamma) |- M ::: A) /\
   (forall Gamma',
-    ok_Bg ((w, Gamma ++ Gamma') :: G) ->
+    ok_Bg_Hyb ((w, Gamma ++ Gamma') :: G) ->
     G |= (w, Gamma ++ Gamma') |- M ::: A).
 intros;
 remember (w, Gamma) as Ctx;
@@ -376,44 +371,45 @@ try (inversion HeqCtx; subst).
 constructor; auto.
 constructor; auto; rewrite Mem_app_or_eq; left; assumption.
 (* lam *)
-apply t_lam_LF with
-  (L:=L \u used_t_vars ((w0, Gamma0) :: G' & (w', Delta ++ Delta')));
+apply t_lam_Hyb with
+  (L:=L \u used_t_vars_Hyb ((w0, Gamma0) :: G' & (w', Delta ++ Delta')));
 [ | intros; eapply H]; auto.
-apply t_lam_LF with (L:=L \u used_t_vars ((w0, Gamma0++Gamma')::G));
+apply t_lam_Hyb with (L:=L \u used_t_vars_Hyb ((w0, Gamma0++Gamma')::G));
 [ | intros; eapply H with (v':=v')  (w:=w0) (Gamma:=(v' ,A)::Gamma0)]; auto;
 rew_app; auto.
 (* appl *)
 econstructor; [ | eapply IHHT1| eapply IHHT2]; eauto.
 econstructor; [ | eapply IHHT1| eapply IHHT2]; eauto.
 (* box *)
-apply t_box_LF with
-  (L:=L \u used_w_vars (G' & (w0, Gamma0) & (w', Delta ++ Delta')));
+apply t_box_Hyb with
+  (L:=L \u used_w_vars_Hyb (G' & (w0, Gamma0) & (w', Delta ++ Delta')));
 intros;
 assert (G' & (w', Delta ++ Delta') & (w0, Gamma0) ~=~
         G' & (w0, Gamma0) & (w', Delta ++ Delta')) by (rew_app; auto);
-[ apply ok_Bg_ppermut with (G:=(w0, Gamma0) :: G' & (w', Delta ++ Delta')) |
-  rewrite H3]; auto; try PPermut_simpl;
+[ apply ok_Bg_Hyb_ppermut with (G:=(w0, Gamma0) :: G' & (w', Delta ++ Delta')) |
+  rewrite H3]; auto; try PPermut_Hyb_simpl;
 apply H with (w:=w'0) (Gamma:=nil);
-[ | | rewrite H0 | rewrite H0 in Ok_Bg]; auto; try PPermut_simpl.
-apply ok_Bg_fresh_wo; auto;
-apply ok_Bg_ppermut with
+[ | | rewrite H0 | rewrite H0 in Ok_Bg]; auto; try PPermut_Hyb_simpl.
+apply ok_Bg_Hyb_fresh_wo; auto;
+apply ok_Bg_Hyb_ppermut with
   (G:=((w0, Gamma0) :: G' & (w', Delta ++ Delta')));
 auto.
-apply t_box_LF with (L:=L \u used_w_vars (G & (w0, Gamma0++Gamma')));
-[ apply ok_Bg_ppermut with (G:= (w0, Gamma0++Gamma') :: G) |
-  intros; eapply H]; auto; try PPermut_simpl;
-apply ok_Bg_fresh_wo; auto;
-apply ok_Bg_ppermut with (G:=(w0, Gamma0++Gamma')::G); auto; PPermut_simpl.
+apply t_box_Hyb with (L:=L \u used_w_vars_Hyb (G & (w0, Gamma0++Gamma')));
+[ apply ok_Bg_Hyb_ppermut with (G:= (w0, Gamma0++Gamma') :: G) |
+  intros; eapply H]; auto; try PPermut_Hyb_simpl;
+apply ok_Bg_Hyb_fresh_wo; auto;
+apply ok_Bg_Hyb_ppermut with (G:=(w0, Gamma0++Gamma')::G); auto;
+PPermut_Hyb_simpl.
 (* unbox *)
 constructor; [ | eapply IHHT]; eauto.
 constructor; [ | eapply IHHT]; eauto.
 (* unbox_fetch 1 *)
-destruct (permut_context_LF_dec (w'0, Delta) (w, Gamma)) as [Eq|Neq];
+destruct (permut_context_Hyb_dec (w'0, Delta) (w, Gamma)) as [Eq|Neq];
 simpl in *.
 (* = *)
 destruct Eq; subst;
 assert (G ~=~ G'0) by
-   (apply PPermut_last_rev with (Gamma := Gamma) (Gamma':= Delta) (w:=w);
+   (apply PPermut_Hyb_last_rev with (Gamma := Gamma) (Gamma':= Delta) (w:=w);
     [ apply permut_sym |
       transitivity G' ]; auto);
 assert ((w0, Gamma0) :: G'0 & (w, Delta ++ Delta') ~=~
@@ -422,53 +418,54 @@ assert ((w0, Gamma0) :: G'0 & (w, Delta ++ Delta') ~=~
    transitivity ((w, Delta ++ Delta') :: G'0 & (w0, Gamma0));
      [ transitivity ((w0, Gamma0) :: (w, Delta ++ Delta') :: G'0) | ]; auto;
        transitivity ((w, Delta ++ Delta') :: (w0, Gamma0) :: G'0);
-       auto; PPermut_simpl);
-apply t_unbox_fetch_LF with (G:=G) (Gamma:=Gamma++Delta');
+       auto; PPermut_Hyb_simpl);
+apply t_unbox_fetch_Hyb with (G:=G) (Gamma:=Gamma++Delta');
 [rewrite <- H4 | apply IHHT | rewrite H3]; auto; rewrite <- H4; auto.
 (* <> *)
 assert (exists Gamma', exists G0, exists G1,
   Gamma' *=* Gamma /\ G'0 = G0 & (w, Gamma') ++ G1) as H2 by
-  ( apply PPermut_split_neq with (G':=G) (w:=w'0) (Gamma := Delta);
+  ( apply PPermut_Hyb_split_neq with (G':=G) (w:=w'0) (Gamma := Delta);
     [ symmetry; transitivity G' | ]; auto);
 destruct H2 as (Gamma', (GH, (GT, (H2a, H2b)))); subst;
-apply t_unbox_fetch_LF with
+apply t_unbox_fetch_Hyb with
   (Gamma:=Gamma) (G:=GH ++ GT & (w'0, Delta ++ Delta')).
-apply ok_Bg_ppermut with
+apply ok_Bg_Hyb_ppermut with
   (G := (w0, Gamma0) :: (GH & (w, Gamma) ++ GT) & (w'0, Delta ++ Delta')); auto.
-rew_app; PPermut_simpl.
+rew_app; PPermut_Hyb_simpl.
 assert ((w0, Gamma0) :: (GH & (w, Gamma) ++ GT) & (w'0, Delta ++ Delta') ~=~
        ((w0, Gamma0) :: (GH & (w, Gamma') ++ GT) & (w'0, Delta ++ Delta')))
-  by PPermut_simpl.
+  by PPermut_Hyb_simpl.
 rewrite H2; auto.
-apply PPermut_bg with (G:= (GH ++ GT & (w0, Gamma0)) & (w'0, Delta ++ Delta')).
+apply PPermut_Hyb_bg with
+  (G:= (GH ++ GT & (w0, Gamma0)) & (w'0, Delta ++ Delta')).
   apply IHHT with (w1:=w) (Gamma1:=Gamma) (G':=GH ++ GT & (w0, Gamma0));
   assert (G ~=~ GH ++ GT & (w'0, Delta)) by
-  ( apply PPermut_last_rev_simpl with (a:=(w, Gamma)); auto; transitivity G';
-     [ | rewrite H0]; auto; PPermut_simpl);
-  auto; try PPermut_simpl.
-  apply ok_Bg_ppermut with (G:= (w0, Gamma0) :: GH ++ (w, Gamma) :: GT &
-     (w'0, Delta ++ Delta')); auto; try PPermut_simpl.
+  ( apply PPermut_Hyb_last_rev_simpl with (a:=(w, Gamma)); auto;
+    transitivity G'; [ | rewrite H0]; auto; PPermut_Hyb_simpl);
+  auto; try PPermut_Hyb_simpl.
+  apply ok_Bg_Hyb_ppermut with (G:= (w0, Gamma0) :: GH ++ (w, Gamma) :: GT &
+     (w'0, Delta ++ Delta')); auto; try PPermut_Hyb_simpl.
   assert ((w0, Gamma0) :: GH ++ (w, Gamma) :: GT & (w'0, Delta ++ Delta') ~=~
        ((w0, Gamma0) :: (GH & (w, Gamma') ++ GT) & (w'0, Delta ++ Delta')))
-  by PPermut_simpl.
+  by PPermut_Hyb_simpl.
   rewrite H3; auto.
   transitivity (((w0, Gamma0) :: GH ++ GT) &
-    (w'0, Delta++Delta')); [rew_app | ]; auto; PPermut_simpl.
+    (w'0, Delta++Delta')); [rew_app | ]; auto; PPermut_Hyb_simpl.
   transitivity (((w, Gamma) :: GH ++ GT ) &
-    (w'0, Delta ++ Delta')); [ | rew_app]; auto; PPermut_simpl.
+    (w'0, Delta ++ Delta')); [ | rew_app]; auto; PPermut_Hyb_simpl.
 (* unbox_fetch 2 *)
-apply t_unbox_fetch_LF with (G:=G) (Gamma:=Gamma);
+apply t_unbox_fetch_Hyb with (G:=G) (Gamma:=Gamma);
 rewrite <- H in H0; [ | apply IHHT with (w1:=w) (Gamma1:=Gamma) |]; auto.
 (* here *)
 constructor; [ | apply IHHT with (w:=w0)(Gamma:=Gamma0)]; auto.
 constructor; [ | apply IHHT]; auto.
 (* get_here 1 *)
-destruct (permut_context_LF_dec (w'0, Delta) (w, Gamma)) as [Eq|Neq];
+destruct (permut_context_Hyb_dec (w'0, Delta) (w, Gamma)) as [Eq|Neq];
 simpl in *.
 (* = *)
 destruct Eq; subst;
 assert (G ~=~ G'0) by
-   (apply PPermut_last_rev with (Gamma := Gamma) (Gamma':= Delta) (w:=w);
+   (apply PPermut_Hyb_last_rev with (Gamma := Gamma) (Gamma':= Delta) (w:=w);
     [ apply permut_sym |
       transitivity G' ]; auto);
 assert ((w0, Gamma0) :: G'0 & (w, Delta ++ Delta') ~=~
@@ -477,80 +474,81 @@ assert ((w0, Gamma0) :: G'0 & (w, Delta ++ Delta') ~=~
    transitivity ((w, Delta ++ Delta') :: G'0 & (w0, Gamma0));
      [ transitivity ((w0, Gamma0) :: (w, Delta ++ Delta') :: G'0) | ]; auto;
        transitivity ((w, Delta ++ Delta') :: (w0, Gamma0) :: G'0);
-       auto; PPermut_simpl);
-apply t_get_here_LF with (G:=G) (Gamma:=Gamma++Delta');
+       auto; PPermut_Hyb_simpl);
+apply t_get_here_Hyb with (G:=G) (Gamma:=Gamma++Delta');
 [rewrite <- H4 | apply IHHT | rewrite H3]; auto; rewrite <- H4; auto.
 (* <> *)
 assert (exists Gamma', exists G0, exists G1,
   Gamma' *=* Gamma /\ G'0 = G0 & (w, Gamma') ++ G1) as H2 by
-  ( apply PPermut_split_neq with (G':=G) (w:=w'0) (Gamma := Delta);
+  ( apply PPermut_Hyb_split_neq with (G':=G) (w:=w'0) (Gamma := Delta);
     [ symmetry; transitivity G' | ]; auto);
 destruct H2 as (Gamma', (GH, (GT, (H2a, H2b)))); subst;
-apply t_get_here_LF with
+apply t_get_here_Hyb with
   (Gamma:=Gamma) (G:=GH ++ GT & (w'0, Delta ++ Delta')).
-apply ok_Bg_ppermut with
+apply ok_Bg_Hyb_ppermut with
   (G := (w0, Gamma0) :: (GH & (w, Gamma) ++ GT) & (w'0, Delta ++ Delta')); auto.
-rew_app; PPermut_simpl.
+rew_app; PPermut_Hyb_simpl.
 assert ((w0, Gamma0) :: (GH & (w, Gamma) ++ GT) & (w'0, Delta ++ Delta') ~=~
        ((w0, Gamma0) :: (GH & (w, Gamma') ++ GT) & (w'0, Delta ++ Delta')))
-  by PPermut_simpl.
+  by PPermut_Hyb_simpl.
 rewrite H2; auto.
-apply PPermut_bg with (G:= (GH ++ GT & (w0, Gamma0)) & (w'0, Delta ++ Delta')).
+apply PPermut_Hyb_bg with
+  (G:= (GH ++ GT & (w0, Gamma0)) & (w'0, Delta ++ Delta')).
   apply IHHT with (w1:=w) (Gamma1:=Gamma) (G':=GH ++ GT & (w0, Gamma0));
   assert (G ~=~ GH ++ GT & (w'0, Delta)) by
-  ( apply PPermut_last_rev_simpl with (a:=(w, Gamma)); auto; transitivity G';
-     [ | rewrite H0]; auto; PPermut_simpl);
-  auto; try PPermut_simpl.
-  apply ok_Bg_ppermut with (G:= (w0, Gamma0) :: GH ++ (w, Gamma) :: GT &
-     (w'0, Delta ++ Delta')); auto; try PPermut_simpl.
+  ( apply PPermut_Hyb_last_rev_simpl with (a:=(w, Gamma)); auto;
+    transitivity G'; [ | rewrite H0]; auto; PPermut_Hyb_simpl);
+  auto; try PPermut_Hyb_simpl.
+  apply ok_Bg_Hyb_ppermut with (G:= (w0, Gamma0) :: GH ++ (w, Gamma) :: GT &
+     (w'0, Delta ++ Delta')); auto; try PPermut_Hyb_simpl.
   assert ((w0, Gamma0) :: GH ++ (w, Gamma) :: GT & (w'0, Delta ++ Delta') ~=~
        ((w0, Gamma0) :: (GH & (w, Gamma') ++ GT) & (w'0, Delta ++ Delta')))
-  by PPermut_simpl.
+  by PPermut_Hyb_simpl.
   rewrite H3; auto.
   transitivity (((w0, Gamma0) :: GH ++ GT) &
-    (w'0, Delta++Delta')); [rew_app | ]; auto; PPermut_simpl.
+    (w'0, Delta++Delta')); [rew_app | ]; auto; PPermut_Hyb_simpl.
   transitivity (((w, Gamma) :: GH ++ GT ) &
-    (w'0, Delta ++ Delta')); [ | rew_app]; auto; PPermut_simpl.
+    (w'0, Delta ++ Delta')); [ | rew_app]; auto; PPermut_Hyb_simpl.
 (* get_here 2 *)
-apply t_get_here_LF with (G:=G) (Gamma:=Gamma);
+apply t_get_here_Hyb with (G:=G) (Gamma:=Gamma);
 rewrite <- H in H0; [ | apply IHHT with (w1:=w) (Gamma1:=Gamma) |]; auto.
 (* letdia *)
-apply t_letdia_LF with (A:=A)
-  (L_w:=L_w \u used_w_vars((w0, Gamma0) :: G' & (w', Delta ++ Delta')))
-  (L_t:=L_t \u used_t_vars ((w0, Gamma0) :: G' & (w', Delta ++ Delta')));
+apply t_letdia_Hyb with (A:=A)
+  (L_w:=L_w \u used_w_vars_Hyb((w0, Gamma0) :: G' & (w', Delta ++ Delta')))
+  (L_t:=L_t \u used_t_vars_Hyb ((w0, Gamma0) :: G' & (w', Delta ++ Delta')));
 [ | apply IHHT with (w:=w0) (Gamma:=Gamma0) | ]; auto;
 intros; destruct H with (v':=v') (w':=w'0) (w:=w0) (Gamma:=Gamma0); auto;
 replace ((w'0, (v', A) :: nil) :: G' & (w', Delta ++ Delta')) with
    (((w'0, (v', A) :: nil) :: G') & (w', Delta ++ Delta')) by
    (rew_app; reflexivity);
 apply H4; rew_app; auto;
-apply ok_Bg_ppermut with
+apply ok_Bg_Hyb_ppermut with
   (G:=(w'0, (v', A) :: nil) :: (w0, Gamma0) :: G' & (w', Delta ++ Delta'));
 auto.
-eapply t_letdia_LF with (A:=A)
-  (L_t := L_t \u used_t_vars ((w0, Gamma0 ++ Gamma') :: G))
-  (L_w := L_w \u used_w_vars ((w0, Gamma0 ++ Gamma') :: G));
+eapply t_letdia_Hyb with (A:=A)
+  (L_t := L_t \u used_t_vars_Hyb ((w0, Gamma0 ++ Gamma') :: G))
+  (L_w := L_w \u used_w_vars_Hyb ((w0, Gamma0 ++ Gamma') :: G));
 [ | apply IHHT | ]; auto;
 intros; eapply H; auto;
-apply ok_Bg_ppermut with
+apply ok_Bg_Hyb_ppermut with
   (G:=(w', (v', A) :: nil) :: (w0, Gamma0 ++ Gamma') :: G);
 auto.
 (* letdia_get 1 *)
-destruct (permut_context_LF_dec (w', Delta) (w, Gamma)) as [Eq | Neq];
+destruct (permut_context_Hyb_dec (w', Delta) (w, Gamma)) as [Eq | Neq];
 simpl in *.
 (* = *)
 destruct Eq; subst;
 assert (G ~=~ G') by
-  (apply PPermut_last_rev with (w:=w) (Gamma:=Gamma) (Gamma':=Delta);
+  (apply PPermut_Hyb_last_rev with (w:=w) (Gamma:=Gamma) (Gamma':=Delta);
    [apply permut_sym | transitivity G0]; auto);
-apply t_letdia_get_LF with (Gamma:=Gamma++Delta') (G:=G) (A:=A)
-  (L_w:=L_w \u used_w_vars ((w0, Gamma0) :: G' & (w, Gamma ++ Delta')))
-  (L_t:=L_t \u used_t_vars ((w0, Gamma0) :: G & (w, Gamma ++ Delta'))).
-apply ok_Bg_ppermut with (G:=(w0, Gamma0) :: G' & (w, Delta ++ Delta'));
+apply t_letdia_get_Hyb with (Gamma:=Gamma++Delta') (G:=G) (A:=A)
+  (L_w:=L_w \u used_w_vars_Hyb ((w0, Gamma0) :: G' & (w, Gamma ++ Delta')))
+  (L_t:=L_t \u used_t_vars_Hyb ((w0, Gamma0) :: G & (w, Gamma ++ Delta'))).
+apply ok_Bg_Hyb_ppermut with (G:=(w0, Gamma0) :: G' & (w, Delta ++ Delta'));
 [rewrite <- H4 | auto];
 transitivity ((w, Delta ++ Delta') :: G & (w0, Gamma0)); auto.
 apply IHHT; auto;
-apply ok_Bg_ppermut with (G:=(w0, Gamma0) :: G' & (w, Delta ++ Delta'));
+apply ok_Bg_Hyb_ppermut with (G:=(w0, Gamma0) :: G' & (w, Delta ++ Delta'));
 [rewrite <- H4 | auto];
 transitivity ((w, Delta ++ Delta') :: G & (w0, Gamma0)); auto.
 intros; destruct H with (v':=v') (w':=w') (w1:=w0) (Gamma1:=Gamma0); eauto;
@@ -558,11 +556,12 @@ replace ( (w', (v', A) :: nil) :: G & (w, Gamma ++ Delta') ) with
   (( (w', (v', A) :: nil) :: G) & (w, Gamma ++ Delta')) by
   (rew_app; reflexivity);
 eapply H7; auto;
-apply ok_Bg_ppermut with
+apply ok_Bg_Hyb_ppermut with
   (G:=(w', (v', A) :: nil ) :: (w0, Gamma0) :: G & (w, Gamma ++ Delta'));
 [ rew_app | rewrite H4]; auto;
-apply ok_Bg_fresh_wo_te;
-[ apply ok_Bg_ppermut with (G:=(w0, Gamma0) :: G' & (w, Delta ++ Delta')) | | ];
+apply ok_Bg_Hyb_fresh_wo_te;
+[ apply ok_Bg_Hyb_ppermut
+  with (G:=(w0, Gamma0) :: G' & (w, Delta ++ Delta')) | | ];
 auto.
 rewrite notin_union in *; destruct H5; auto;
 rewrite <- H4; auto.
@@ -570,110 +569,114 @@ rewrite <- H4; auto.
 (* <> *)
 assert (exists Gamma', exists G0, exists G1,
   Gamma' *=* Gamma /\ G' = G0 & (w, Gamma') ++ G1) by
-  ( apply PPermut_split_neq with (G':=G) (w:=w') (Gamma := Delta);
+  ( apply PPermut_Hyb_split_neq with (G':=G) (w:=w') (Gamma := Delta);
     [ symmetry; transitivity G0 | ]; auto).
 destruct H3 as (Gamma', (GH, (GT, (H3a, H3b)))); subst;
 assert ((w0, Gamma0) :: (GH & (w, Gamma') ++ GT) & (w', Delta ++ Delta') ~=~
   (w0, Gamma0) :: (GH & (w, Gamma) ++ GT) & (w', Delta ++ Delta'))
-by PPermut_simpl;
+by PPermut_Hyb_simpl;
 assert (G ~=~ GH ++ GT & (w', Delta)) by
-  ( apply PPermut_last_rev_simpl with (a:=(w, Gamma));
-    transitivity G0; auto; rewrite H1; PPermut_simpl);
-apply t_letdia_get_LF with
+  ( apply PPermut_Hyb_last_rev_simpl with (a:=(w, Gamma));
+    transitivity G0; auto; rewrite H1; PPermut_Hyb_simpl);
+apply t_letdia_get_Hyb with
   (Gamma:=Gamma) (G:=GH ++ GT & (w', Delta ++ Delta'))
-  (L_w:=L_w \u used_w_vars ((w0, Gamma0) :: (GH & (w, Gamma) ++ GT) &
+  (L_w:=L_w \u used_w_vars_Hyb ((w0, Gamma0) :: (GH & (w, Gamma) ++ GT) &
     (w', Delta ++ Delta')))
-  (L_t:=L_t \u used_t_vars ((w0, Gamma0) :: (GH & (w, Gamma) ++ GT) &
+  (L_t:=L_t \u used_t_vars_Hyb ((w0, Gamma0) :: (GH & (w, Gamma) ++ GT) &
     (w', Delta ++ Delta')))(A:=A).
-apply ok_Bg_ppermut with
+apply ok_Bg_Hyb_ppermut with
   (G:=(w0, Gamma0) :: (GH & (w, Gamma') ++ GT) & (w', Delta ++ Delta'));
-rew_app in *; auto; try PPermut_simpl.
-apply PPermut_bg with (G:= (GH ++ GT & (w0, Gamma0)) & (w', Delta ++ Delta'));
+rew_app in *; auto; try PPermut_Hyb_simpl.
+apply PPermut_Hyb_bg with
+  (G:= (GH ++ GT & (w0, Gamma0)) & (w', Delta ++ Delta'));
 [ | rew_app]; auto;
 apply IHHT with (w1:=w) (Gamma1:=Gamma); auto;
 [ rewrite H4 | ]; rew_app; auto;
-rew_app; apply ok_Bg_ppermut with
+rew_app; apply ok_Bg_Hyb_ppermut with
   (G:=(w0, Gamma0) :: (GH & (w, Gamma') ++ GT) & (w', Delta ++ Delta')); auto;
-rew_app; try PPermut_simpl.
+rew_app; try PPermut_Hyb_simpl.
 intros; destruct H with (v':=v')(w':=w'0) (w1:=w0) (Gamma1:=Gamma0); auto;
-apply PPermut_bg with
+apply PPermut_Hyb_bg with
   (G:=((w'0, (v', A)::nil) :: GH++GT & (w, Gamma)) & (w', Delta ++ Delta'));
 [ | rew_app]; auto;
 apply H7; rew_app; [constructor | ]; auto;
 [ rewrite H4; rew_app; auto | ];
-apply ok_Bg_ppermut with
+apply ok_Bg_Hyb_ppermut with
   (G:= ((w'0, (v', A) :: nil) ::(w0, Gamma0) :: GH & (w, Gamma') ++ GT) &
     (w', Delta ++ Delta')); rew_app; auto;
 [ transitivity (((w'0, (v', A) :: nil) ::(w0, Gamma0) :: GH ++GT & (w, Gamma))
   & (w', Delta ++ Delta')); rew_app |
- rew_app in *; apply ok_Bg_fresh_wo_te]; auto; try PPermut_simpl.
+ rew_app in *; apply ok_Bg_Hyb_fresh_wo_te]; auto; try PPermut_Hyb_simpl.
 rewrite H3; auto.
 rewrite H3; auto.
-rew_app; PPermut_simpl.
+rew_app; PPermut_Hyb_simpl.
 (* letdia_get 2 *)
-apply t_letdia_get_LF with (G:=G) (Gamma:=Gamma) (A:=A)
-  (L_w:=L_w \u used_w_vars (((w0, Gamma0 ++ Gamma') :: G & (w, Gamma))))
-  (L_t:=L_t \u used_t_vars ((w0, Gamma0 ++ Gamma') :: G & (w, Gamma))).
-rewrite <- H0 in H1; apply ok_Bg_ppermut with
+apply t_letdia_get_Hyb with (G:=G) (Gamma:=Gamma) (A:=A)
+  (L_w:=L_w \u used_w_vars_Hyb (((w0, Gamma0 ++ Gamma') :: G & (w, Gamma))))
+  (L_t:=L_t \u used_t_vars_Hyb ((w0, Gamma0 ++ Gamma') :: G & (w, Gamma))).
+rewrite <- H0 in H1; apply ok_Bg_Hyb_ppermut with
   (G:=(w0, Gamma0 ++ Gamma') :: G & (w, Gamma)); auto.
 apply IHHT with (w1:=w) (Gamma1:=Gamma); auto.
-rewrite <- H0 in H1; apply ok_Bg_ppermut with
+rewrite <- H0 in H1; apply ok_Bg_Hyb_ppermut with
   (G:=(w0, Gamma0 ++ Gamma') :: G & (w, Gamma)); auto.
 intros; destruct H with (v':=v')(w':=w') (w1:=w0)(Gamma1:=Gamma0); auto;
-apply H5; apply ok_Bg_ppermut with
+apply H5; apply ok_Bg_Hyb_ppermut with
   (G:= (w', (v', A)::nil) :: (w0, Gamma0 ++ Gamma') :: G & (w, Gamma));
-[ | apply ok_Bg_fresh_wo_te ]; auto; rewrite H0; auto.
+[ | apply ok_Bg_Hyb_fresh_wo_te ]; auto; rewrite H0; auto.
 assumption.
 Qed.
 
-Lemma WeakeningBackgroundElem:
+Lemma WeakeningBackgroundElem_Hyb:
 forall G G' w Delta Delta' Ctx M A
-  (H_ok: ok_Bg (Ctx :: G & (w, Delta ++ Delta') ++ G'))
+  (H_ok: ok_Bg_Hyb (Ctx :: G & (w, Delta ++ Delta') ++ G'))
   (HT: G & (w, Delta) ++ G' |= Ctx |- M ::: A),
   G & (w, Delta ++ Delta') ++ G' |= Ctx |- M ::: A.
 intros;
 assert ( G & (w, Delta ++ Delta') ++ G' ~=~ (G++G') & (w, Delta ++ Delta'))
   by (rew_app; auto);
 rewrite H;
-destruct Ctx; eapply Weakening_general; auto.
+destruct Ctx; eapply Weakening_general_Hyb; auto.
 rew_app; assert (G ++ G' & (w, Delta) ~=~ G & (w, Delta) ++ G') by auto;
 rewrite H0; assumption.
-apply ok_Bg_ppermut with (G:=(v, l) :: G & (w, Delta ++ Delta') ++ G'); auto.
+apply ok_Bg_Hyb_ppermut with (G:=(v, l) :: G & (w, Delta ++ Delta') ++ G');
+auto.
 Qed.
 
-Lemma Weakening:
+Lemma Weakening_Hyb:
 forall G w Gamma Gamma' M A
-  (H_ok: ok_Bg ((w,Gamma++Gamma')::G))
+  (H_ok: ok_Bg_Hyb ((w,Gamma++Gamma')::G))
   (HT: G |= (w, Gamma) |- M ::: A),
   G |= (w, Gamma ++ Gamma') |- M ::: A.
 intros;
-eapply Weakening_general; eassumption.
+eapply Weakening_general_Hyb; eassumption.
 Qed.
 
 (*
    When we can prove something in empty context and background, then we
    can also do it in any "full" version of this context & background
 *)
-Lemma types_weakened:
+Lemma types_weakened_Hyb:
 forall G G' w Gamma M A
-  (Ok: ok_Bg ((w, Gamma)::G ++ G'))
-  (HT: emptyEquiv G ++ G' |= (w, nil) |- M ::: A),
+  (Ok: ok_Bg_Hyb ((w, Gamma)::G ++ G'))
+  (HT: emptyEquiv_Hyb G ++ G' |= (w, nil) |- M ::: A),
   G ++ G'|= (w, Gamma) |- M ::: A.
 induction G; intros; simpl in *; rew_app in *; auto.
-apply Weakening with (Gamma':=Gamma) in HT; rew_app in *; auto.
+apply Weakening_Hyb with (Gamma':=Gamma) in HT; rew_app in *; auto.
 destruct a; rew_app in *.
-assert ((v,l) :: G ++ G' ~=~ G ++ (v,l)::G') by PPermut_simpl;
+assert ((v,l) :: G ++ G' ~=~ G ++ (v,l)::G') by PPermut_Hyb_simpl;
 rewrite H; apply IHG.
 rewrite <- H; auto.
-assert (emptyEquiv G ++ (v, l) :: G' ~=~ emptyEquiv G & (v, nil ++ l) ++ G')
-  by PPermut_simpl; rewrite H0; eapply WeakeningBackgroundElem.
+assert (emptyEquiv_Hyb G ++ (v, l) :: G' ~=~
+  emptyEquiv_Hyb G & (v, nil ++ l) ++ G')
+  by PPermut_Hyb_simpl; rewrite H0; eapply WeakeningBackgroundElem_Hyb.
 rew_app.
-apply ok_Bg_empty_first in Ok.
+apply ok_Bg_Hyb_empty_first in Ok.
 assert ((w, nil) :: (v, l) :: G ++ G' ~=~ ((w, nil) :: G) ++ (v, l) :: G') by
-  PPermut_simpl; rewrite H1 in Ok;
-eapply emptyEquiv_ok_Bg_part in Ok; simpl in *; rew_app in *; auto.
-assert (emptyEquiv G & (v, nil) ++ G' ~=~  (v, nil) :: emptyEquiv G ++ G') by
-  PPermut_simpl; rewrite H1; auto.
+  PPermut_Hyb_simpl; rewrite H1 in Ok;
+eapply emptyEquiv_Hyb_ok_Bg_Hyb_part in Ok; simpl in *; rew_app in *; auto.
+assert (emptyEquiv_Hyb G & (v, nil) ++ G' ~=~
+  (v, nil) :: emptyEquiv_Hyb G ++ G') by
+  PPermut_Hyb_simpl; rewrite H1; auto.
 Qed.
 
 
@@ -689,15 +692,15 @@ Proof: induction on typing
   options: either it is the marked element or we have to do a manual
   split in order to find it
 *)
-Lemma subst_t_preserv_types:
+Lemma subst_t_Hyb_preserv_types:
 forall G w Gamma B M N v A
-  (H_lc_t: lc_t_LF M)
-  (H_lc_w: lc_w_LF M)
+  (H_lc_t: lc_t_Hyb M)
+  (H_lc_w: lc_w_Hyb M)
   (HT: G |= (w, Gamma) |- N ::: B),
   (* "inner" substitution *)
   ( forall Gamma0,
     permut Gamma ((v, A) :: Gamma0) ->
-    emptyEquiv G |= (w, nil) |- M ::: A ->
+    emptyEquiv_Hyb G |= (w, nil) |- M ::: A ->
     G |= (w, Gamma0) |- [M // fte v] N ::: B)
   /\
   (* "outer" substitution *)
@@ -705,7 +708,7 @@ forall G w Gamma B M N v A
     G ~=~ (G0 & (w', (v,A)::Gamma')) ->
     G' ~=~ (G0 & (w, Gamma)) ->
     G'' ~=~ (G0 & (w', Gamma')) ->
-    emptyEquiv G' |= (w', nil) |- M ::: A ->
+    emptyEquiv_Hyb G' |= (w', nil) |- M ::: A ->
     G'' |= (w, Gamma) |- [M // fte v] N ::: B).
 intros;
 remember (w, Gamma) as Ctx;
@@ -721,121 +724,122 @@ simpl in *.
 (* hyp *)
 case_if.
 inversion H1; subst;
-assert (A = A0) by (eapply ok_Bg_Mem_eq; eauto);
+assert (A = A0) by (eapply ok_Bg_Hyb_Mem_eq; eauto);
 subst; replace G with (G ++ nil) by (rew_app; auto);
-apply types_weakened;
-[eapply ok_Bg_permut_first_tail with (C:=Gamma0) | ]; rew_app; eauto.
+apply types_weakened_Hyb;
+[eapply ok_Bg_Hyb_permut_first_tail with (C:=Gamma0) | ]; rew_app; eauto.
 constructor;
-[ apply ok_Bg_permut_first_tail with (C:=Gamma0) (x:=v0) (A:=A0) |
+[ apply ok_Bg_Hyb_permut_first_tail with (C:=Gamma0) (x:=v0) (A:=A0) |
   apply Mem_permut with (l' := (v0, A0) :: Gamma1) in HT]; eauto.
 rewrite Mem_cons_eq in HT; destruct HT; auto;
 inversion H2; subst; elim H1; reflexivity.
 
 case_if.
 inversion H3; subst;
-eapply ok_Bg_Mem_contradict in Ok_Bg;
+eapply ok_Bg_Hyb_Mem_contradict in Ok_Bg;
 contradiction || eauto.
 constructor; auto;
-apply ok_Bg_ppermut with (G:=((w0, Gamma0)::G0) & (w', Gamma'));
+apply ok_Bg_Hyb_ppermut with (G:=((w0, Gamma0)::G0) & (w', Gamma'));
 [ rewrite H1 |
-  eapply ok_Bg_permut_no_last; rewrite H in Ok_Bg; rew_app]; eauto.
+  eapply ok_Bg_Hyb_permut_no_last; rewrite H in Ok_Bg; rew_app]; eauto.
 
 (* lam *)
-apply t_lam_LF with (L:=L \u \{v});
-[ apply ok_Bg_permut_first_tail with (C:=Gamma0) (x:=v) (A:=A0) |
+apply t_lam_Hyb with (L:=L \u \{v});
+[ apply ok_Bg_Hyb_permut_first_tail with (C:=Gamma0) (x:=v) (A:=A0) |
   intros]; auto;
 rewrite notin_union in H2; rewrite notin_singleton in H2; destruct H2;
-unfold open_t in *;
-rewrite <- subst_t_comm; auto;
+unfold open_t_Hyb in *;
+rewrite <- subst_t_Hyb_comm; auto;
 eapply H; auto;
 permut_simpl || rew_app; eauto.
 
-apply t_lam_LF with (L:=L \u \{v});
-[ apply ok_Bg_ppermut with (G:=((w0, Gamma0)::G0) & (w', Gamma'));
+apply t_lam_Hyb with (L:=L \u \{v});
+[ apply ok_Bg_Hyb_ppermut with (G:=((w0, Gamma0)::G0) & (w', Gamma'));
   [ rewrite H2 |
     rewrite H0 in Ok_Bg; rew_app] |
-  intros]; eauto with ok_bg_rew;
+  intros]; eauto with ok_bg_hyb_rew;
 rewrite notin_union in H4; rewrite notin_singleton in H4; destruct H4;
-unfold open_t in *;
-rewrite <- subst_t_comm; auto;
+unfold open_t_Hyb in *;
+rewrite <- subst_t_Hyb_comm; auto;
 eapply H with (G0:=G0) (w':=w'); eauto;
-assert (emptyEquiv G' ~=~ emptyEquiv (G0 ++ nil & (w0, (v', A) :: Gamma0))) as E
- by (rewrite H1; rew_app; eapply emptyEquiv_last_change; auto);
+assert (emptyEquiv_Hyb G' ~=~
+  emptyEquiv_Hyb (G0 ++ nil & (w0, (v', A) :: Gamma0))) as E
+ by (rewrite H1; rew_app; eapply emptyEquiv_Hyb_last_change; auto);
 rew_app in *; rewrite <- E; auto.
 
 (* appl *)
 econstructor;  [ | eapply IHHT1 | eapply IHHT2];
-try apply ok_Bg_permut_first_tail with (C:=Gamma0) (x:=v) (A:=A0); eauto.
+try apply ok_Bg_Hyb_permut_first_tail with (C:=Gamma0) (x:=v) (A:=A0); eauto.
 
 econstructor;
-[ apply ok_Bg_ppermut with (G:=((w0, Gamma0)::G0) & (w', Gamma'));
+[ apply ok_Bg_Hyb_ppermut with (G:=((w0, Gamma0)::G0) & (w', Gamma'));
   [rewrite H1 | rewrite H in Ok_Bg] |
   eapply IHHT1 |
   eapply IHHT2]; eauto;
-apply ok_Bg_permut_no_last_spec in Ok_Bg; rew_app; auto.
+apply ok_Bg_Hyb_permut_no_last_spec in Ok_Bg; rew_app; auto.
 
 (* box *)
-apply t_box_LF with (L:=L \u used_w_vars (emptyEquiv G & (w0, nil)));
-[ apply ok_Bg_permut_no_last with (v:=v) (A:=A0);
-  eapply ok_Bg_permut_last |
-  intros; unfold open_w]; eauto;
-rewrite <- subst_order_irrelevant_bound;
+apply t_box_Hyb with (L:=L \u used_w_vars_Hyb (emptyEquiv_Hyb G & (w0, nil)));
+[ apply ok_Bg_Hyb_permut_no_last with (v:=v) (A:=A0);
+  eapply ok_Bg_Hyb_permut_last |
+  intros; unfold open_w_Hyb]; eauto;
+rewrite <- subst_Hyb_order_irrelevant_bound;
 [ eapply H; eauto |
-  repeat rewrite emptyEquiv_rewrite];
+  repeat rewrite emptyEquiv_Hyb_rewrite];
 simpl; rew_app; auto;
-apply BackgroundSubsetImpl with (G:=emptyEquiv G); auto;
+apply BackgroundSubsetImpl_Hyb with (G:=emptyEquiv_Hyb G); auto;
 [ exists ((w', (@nil (prod var ty))) :: nil); rew_app; auto |
-  assert ((w0, nil) :: emptyEquiv G & (w', nil) ~=~
-    (w', nil) :: emptyEquiv G & (w0, nil)) by auto];
-rew_app; rewrite emptyEquiv_rewrite_last; simpl; auto;
+  assert ((w0, nil) :: emptyEquiv_Hyb G & (w', nil) ~=~
+    (w', nil) :: emptyEquiv_Hyb G & (w0, nil)) by auto];
+rew_app; rewrite emptyEquiv_Hyb_rewrite_last; simpl; auto;
 rewrite H3;
-apply ok_Bg_fresh_wo; auto;
-apply emptyEquiv_ok_Bg in Ok_Bg;
-rewrite emptyEquiv_rewrite in Ok_Bg;
+apply ok_Bg_Hyb_fresh_wo; auto;
+apply emptyEquiv_Hyb_ok_Bg_Hyb in Ok_Bg;
+rewrite emptyEquiv_Hyb_rewrite in Ok_Bg;
 simpl in *; auto.
 
-apply t_box_LF with
-  (L:=L \u used_w_vars(emptyEquiv G0 ++ (w', nil) :: (w0, nil) :: nil));
+apply t_box_Hyb with
+  (L:=L \u used_w_vars_Hyb(emptyEquiv_Hyb G0 ++ (w', nil) :: (w0, nil) :: nil));
 [ rewrite H2; rewrite H0 in Ok_Bg |
-  intros; unfold open_w; rewrite <- subst_order_irrelevant_bound];
-eauto with ok_bg_rew;
+  intros; unfold open_w_Hyb; rewrite <- subst_Hyb_order_irrelevant_bound];
+eauto with ok_bg_hyb_rew;
 eapply H with (G'' := G'' & (w0, Gamma0)) (G0:=G0 & (w0, Gamma0)) (w'0:=w')
   (Gamma':=Gamma') (A0:=A0); auto;
-repeat rewrite emptyEquiv_rewrite;
-simpl; rew_app; try PPermut_simpl;
-apply BackgroundSubsetImpl with (G:=emptyEquiv G0 & (w0, nil));
-[ rewrite H1 in H3; rewrite emptyEquiv_rewrite in H3 |
+repeat rewrite emptyEquiv_Hyb_rewrite;
+simpl; rew_app; try PPermut_Hyb_simpl;
+apply BackgroundSubsetImpl_Hyb with (G:=emptyEquiv_Hyb G0 & (w0, nil));
+[ rewrite H1 in H3; rewrite emptyEquiv_Hyb_rewrite in H3 |
   exists ((w'0, (@nil (var * ty)))::nil); rew_app |
-  apply emptyEquiv_ok_Bg in Ok_Bg; rewrite H0 in Ok_Bg]; auto;
-repeat rewrite emptyEquiv_rewrite in Ok_Bg;
+  apply emptyEquiv_Hyb_ok_Bg_Hyb in Ok_Bg; rewrite H0 in Ok_Bg]; auto;
+repeat rewrite emptyEquiv_Hyb_rewrite in Ok_Bg;
 simpl in *; rew_app in *;
-apply ok_Bg_ppermut with
-  (G:=(w'0, nil) :: emptyEquiv G0 ++ (w', nil) :: (w0, nil) :: nil);
-[eauto with ppermut_rew | apply ok_Bg_fresh_wo ]; auto.
+apply ok_Bg_Hyb_ppermut with
+  (G:=(w'0, nil) :: emptyEquiv_Hyb G0 ++ (w', nil) :: (w0, nil) :: nil);
+[eauto with ppermut_rew | apply ok_Bg_Hyb_fresh_wo ]; auto.
 
 (* unbox *)
 econstructor; [ | eapply IHHT];
-try apply ok_Bg_permut_first_tail with (C:=Gamma0) (x:=v) (A:=A0); eauto.
+try apply ok_Bg_Hyb_permut_first_tail with (C:=Gamma0) (x:=v) (A:=A0); eauto.
 
 econstructor;
 [ rewrite H1; rewrite H in Ok_Bg |
-  eapply IHHT]; eauto with ok_bg_rew.
+  eapply IHHT]; eauto with ok_bg_hyb_rew.
 
 (* unbox_fetch *)
-apply t_unbox_fetch_LF with (G:=G) (Gamma:=Gamma); auto;
-[ apply ok_Bg_permut_no_last_spec with (v:=v) (A:=A0);
-  apply ok_Bg_ppermut with (G:= (w, Gamma) :: G & (w0, Gamma0)) |
+apply t_unbox_fetch_Hyb with (G:=G) (Gamma:=Gamma); auto;
+[ apply ok_Bg_Hyb_permut_no_last_spec with (v:=v) (A:=A0);
+  apply ok_Bg_Hyb_ppermut with (G:= (w, Gamma) :: G & (w0, Gamma0)) |
   eapply IHHT; eauto; rewrite <- H in H1; rew_app]; auto.
 
 destruct (eq_var_dec w w'0).
 (* = *)
 subst;
 assert (G ~=~ G0 /\ Gamma *=* (v, A0) :: Gamma'0) as HP by
-  (apply ok_Bg_impl_ppermut with (w:=w'0);
-   [eauto with ok_bg_rew | transitivity G'; auto]);
+  (apply ok_Bg_Hyb_impl_ppermut with (w:=w'0);
+   [eauto with ok_bg_hyb_rew | transitivity G'; auto]);
 destruct HP;
-apply t_unbox_fetch_LF with (G:=G) (Gamma:=Gamma'0);
-eauto with ok_bg_rew;
+apply t_unbox_fetch_Hyb with (G:=G) (Gamma:=Gamma'0);
+eauto with ok_bg_hyb_rew;
 specialize IHHT with (Gamma1:=Gamma) (w:=w'0);
 destruct IHHT with (M0:=M0) (A0:=A0) (v:=v); auto;
 [ apply H6; auto; rewrite H1 in H3; rewrite H4 |
@@ -843,58 +847,59 @@ destruct IHHT with (M0:=M0) (A0:=A0) (v:=v); auto;
 (* <> *)
 assert (exists Gamma', exists GH, exists GT,
   Gamma' *=* (v, A0)::Gamma'0 /\ G = GH & (w'0, Gamma') ++ GT) as HP by
-  (apply PPermut_split_neq with (w:=w) (Gamma:=Gamma) (G':=G0);
+  (apply PPermut_Hyb_split_neq with (w:=w) (Gamma:=Gamma) (G':=G0);
     auto; transitivity G'; auto).
 destruct HP as (Gamma', (GH, (GT, (HPa, HPb)))).
 assert (GH & (w'0, Gamma') ++ GT ~=~ GH & (w'0, (v, A0)::Gamma'0) ++ GT)
-  by PPermut_simpl;
-apply t_unbox_fetch_LF with (G:=GH ++ GT & (w'0, Gamma'0)) (Gamma:=Gamma).
+  by PPermut_Hyb_simpl;
+apply t_unbox_fetch_Hyb with (G:=GH ++ GT & (w'0, Gamma'0)) (Gamma:=Gamma).
 subst;
-apply ok_Bg_ppermut with
+apply ok_Bg_Hyb_ppermut with
   (G:= (((w, Gamma) :: (GH & (w0, Gamma0) ++ GT)) & (w'0, Gamma'0)));
 [rew_app | ]; auto;
-apply ok_Bg_permut_no_last_spec with (v:=v)(A:=A0).
-apply ok_Bg_ppermut with
+apply ok_Bg_Hyb_permut_no_last_spec with (v:=v)(A:=A0).
+apply ok_Bg_Hyb_ppermut with
   (G:=(w, Gamma):: (GH & (w'0, Gamma') ++ GT) & (w0, Gamma0));
-rew_app in *; auto; PPermut_simpl.
+rew_app in *; auto; PPermut_Hyb_simpl.
 eapply IHHT with (w1:=w) (Gamma1:=Gamma) (w':=w'0) (Gamma':=Gamma'0)
                  (G0:=GH ++ GT & (w0, Gamma0)); rew_app; auto; subst;
 rew_app; auto;
 rewrite H1 in H3;
 assert (GH ++ (w, Gamma) :: GT ~=~ G0) by
-  (apply PPermut_last_rev_simpl with (a:=(w'0, (v, A0) :: Gamma'0));
-  rew_app in *; rewrite <- H0; rewrite <- H; auto; PPermut_simpl).
-PPermut_simpl; eauto.
+  (apply PPermut_Hyb_last_rev_simpl with (a:=(w'0, (v, A0) :: Gamma'0));
+  rew_app in *; rewrite <- H0; rewrite <- H; auto; PPermut_Hyb_simpl).
+PPermut_Hyb_simpl; eauto.
 assert (GH ++ (w, Gamma) :: GT & (w0, Gamma0) ~=~ G0 & (w0,Gamma0)) by
-  (rewrite <- H5; rew_app; auto; PPermut_simpl);
+  (rewrite <- H5; rew_app; auto; PPermut_Hyb_simpl);
 rewrite H6; auto.
-subst; rewrite H2; PPermut_simpl.
-apply PPermut_last_rev with (w:=w'0) (Gamma:=Gamma') (Gamma':=(v,A0)::Gamma'0);
-[ | symmetry]; auto; transitivity G'; auto; rewrite <- H; PPermut_simpl.
+subst; rewrite H2; PPermut_Hyb_simpl.
+apply PPermut_Hyb_last_rev with (w:=w'0) (Gamma:=Gamma')
+  (Gamma':=(v,A0)::Gamma'0);
+[ | symmetry]; auto; transitivity G'; auto; rewrite <- H; PPermut_Hyb_simpl.
 
 (* here *)
 econstructor; [ | eapply IHHT];
-try apply ok_Bg_permut_first_tail with (C:=Gamma0) (x:=v) (A:=A0); eauto.
+try apply ok_Bg_Hyb_permut_first_tail with (C:=Gamma0) (x:=v) (A:=A0); eauto.
 
 econstructor;
 [ rewrite H1; rewrite H in Ok_Bg |
-  eapply IHHT]; eauto with ok_bg_rew.
+  eapply IHHT]; eauto with ok_bg_hyb_rew.
 
 (* get_here *)
-apply t_get_here_LF with (G:=G) (Gamma:=Gamma); auto;
-[ apply ok_Bg_permut_no_last_spec with (v:=v) (A:=A0);
-  apply ok_Bg_ppermut with (G:= (w, Gamma) :: G & (w0, Gamma0)) |
+apply t_get_here_Hyb with (G:=G) (Gamma:=Gamma); auto;
+[ apply ok_Bg_Hyb_permut_no_last_spec with (v:=v) (A:=A0);
+  apply ok_Bg_Hyb_ppermut with (G:= (w, Gamma) :: G & (w0, Gamma0)) |
   eapply IHHT; eauto; rewrite <- H in H1; rew_app]; auto.
 
 destruct (eq_var_dec w w'0).
 (* = *)
 subst;
 assert (G ~=~ G0 /\ Gamma *=* (v, A0) :: Gamma'0) as HP by
-  (apply ok_Bg_impl_ppermut with (w:=w'0);
-   [eauto with ok_bg_rew | transitivity G'; auto]);
+  (apply ok_Bg_Hyb_impl_ppermut with (w:=w'0);
+   [eauto with ok_bg_hyb_rew | transitivity G'; auto]);
 destruct HP;
-apply t_get_here_LF with (G:=G) (Gamma:=Gamma'0);
-eauto with ok_bg_rew;
+apply t_get_here_Hyb with (G:=G) (Gamma:=Gamma'0);
+eauto with ok_bg_hyb_rew;
 specialize IHHT with (Gamma1:=Gamma) (w:=w'0);
 destruct IHHT with (M0:=M0) (A0:=A0) (v:=v); auto;
 [ apply H6; auto; rewrite H1 in H3; rewrite H4 |
@@ -902,135 +907,141 @@ destruct IHHT with (M0:=M0) (A0:=A0) (v:=v); auto;
 (* <> *)
 assert (exists Gamma', exists GH, exists GT,
   Gamma' *=* (v, A0)::Gamma'0 /\ G = GH & (w'0, Gamma') ++ GT) as HP by
-  (apply PPermut_split_neq with (w:=w) (Gamma:=Gamma) (G':=G0);
+  (apply PPermut_Hyb_split_neq with (w:=w) (Gamma:=Gamma) (G':=G0);
     eauto; transitivity G'; auto).
 destruct HP as (Gamma', (GH, (GT, (HPa, HPb)))).
 assert (GH & (w'0, Gamma') ++ GT ~=~ GH & (w'0, (v, A0)::Gamma'0) ++ GT)
-  by PPermut_simpl;
-apply t_get_here_LF with (G:=GH ++ GT & (w'0, Gamma'0)) (Gamma:=Gamma).
+  by PPermut_Hyb_simpl;
+apply t_get_here_Hyb with (G:=GH ++ GT & (w'0, Gamma'0)) (Gamma:=Gamma).
 subst;
-apply ok_Bg_ppermut with
+apply ok_Bg_Hyb_ppermut with
   (G:= (((w, Gamma) :: (GH & (w0, Gamma0) ++ GT)) & (w'0, Gamma'0)));
 [rew_app | ]; auto;
-apply ok_Bg_permut_no_last_spec with (v:=v)(A:=A0).
-apply ok_Bg_ppermut with
+apply ok_Bg_Hyb_permut_no_last_spec with (v:=v)(A:=A0).
+apply ok_Bg_Hyb_ppermut with
   (G:=(w, Gamma):: (GH & (w'0, Gamma') ++ GT) & (w0, Gamma0));
-rew_app in *; auto; PPermut_simpl.
+rew_app in *; auto; PPermut_Hyb_simpl.
 eapply IHHT with (w1:=w) (Gamma1:=Gamma) (w':=w'0) (Gamma':=Gamma'0)
                  (G0:=GH ++ GT & (w0, Gamma0)) (A0:=A0); rew_app; auto; subst;
 rew_app; auto;
 rewrite H1 in H3;
 assert (GH ++ (w, Gamma) :: GT ~=~ G0) by
-  (apply PPermut_last_rev_simpl with (a:=(w'0, (v, A0) :: Gamma'0));
-  rew_app in *; rewrite <- H0; rewrite <- H; auto; PPermut_simpl).
-PPermut_simpl; auto.
+  (apply PPermut_Hyb_last_rev_simpl with (a:=(w'0, (v, A0) :: Gamma'0));
+  rew_app in *; rewrite <- H0; rewrite <- H; auto; PPermut_Hyb_simpl).
+PPermut_Hyb_simpl; auto.
 assert (GH ++ (w, Gamma) :: GT & (w0, Gamma0) ~=~ G0 & (w0,Gamma0)) by
-  (rewrite <- H5; rew_app; auto; PPermut_simpl);
+  (rewrite <- H5; rew_app; auto; PPermut_Hyb_simpl);
 rewrite H6; auto.
-subst; rewrite H2; PPermut_simpl.
-apply PPermut_last_rev with (w:=w'0) (Gamma:=Gamma') (Gamma':=(v,A0)::Gamma'0);
-[ | symmetry]; auto; transitivity G'; auto; rewrite <- H; PPermut_simpl.
+subst; rewrite H2; PPermut_Hyb_simpl.
+apply PPermut_Hyb_last_rev with (w:=w'0) (Gamma:=Gamma')
+  (Gamma':=(v,A0)::Gamma'0);
+[ | symmetry]; auto; transitivity G'; auto; rewrite <- H; PPermut_Hyb_simpl.
 
 (* letdia *)
-apply t_letdia_LF with
+apply t_letdia_Hyb with
   (L_t := L_t \u \{v})
-  (L_w := L_w \u used_w_vars ((w0, nil) :: emptyEquiv G)) (A:=A);
-[ apply ok_Bg_permut_first_tail with (C:=Gamma0) (x:=v) (A:=A0) |
+  (L_w := L_w \u used_w_vars_Hyb ((w0, nil) :: emptyEquiv_Hyb G)) (A:=A);
+[ apply ok_Bg_Hyb_permut_first_tail with (C:=Gamma0) (x:=v) (A:=A0) |
   eapply IHHT |
   intros]; eauto;
-unfold open_t in *; unfold open_w in *;
+unfold open_t_Hyb in *; unfold open_w_Hyb in *;
 rewrite notin_union in H2; rewrite notin_singleton in H2; destruct H2;
-rewrite <- subst_order_irrelevant_bound;
-[ rewrite <- subst_t_comm | assumption ];
+rewrite <- subst_Hyb_order_irrelevant_bound;
+[ rewrite <- subst_t_Hyb_comm | assumption ];
 [ eapply H | |] ; eauto;
-apply BackgroundSubsetImpl with (G:=emptyEquiv G); auto;
+apply BackgroundSubsetImpl_Hyb with (G:=emptyEquiv_Hyb G); auto;
 [ exists ((w', (@nil (var*ty)))::nil);
-  PPermut_simpl ; rew_app; PPermut_simpl | ].
-assert ((w0, nil) :: (w', nil) :: emptyEquiv G ~=~
-  (w',nil) :: (w0, nil) :: emptyEquiv G) by PPermut_simpl;
-rewrite H5; apply ok_Bg_fresh_wo;
-[ apply emptyEquiv_ok_Bg in Ok_Bg;  simpl in * | ]; auto.
+  PPermut_Hyb_simpl ; rew_app; PPermut_Hyb_simpl | ].
+assert ((w0, nil) :: (w', nil) :: emptyEquiv_Hyb G ~=~
+  (w',nil) :: (w0, nil) :: emptyEquiv_Hyb G) by PPermut_Hyb_simpl;
+rewrite H5; apply ok_Bg_Hyb_fresh_wo;
+[ apply emptyEquiv_Hyb_ok_Bg_Hyb in Ok_Bg;  simpl in * | ]; auto.
 
-eapply t_letdia_LF with
+eapply t_letdia_Hyb with
   (L_t := L_t \u \{v})
-  (L_w := L_w \u  used_w_vars ((w', nil) :: emptyEquiv (G0 & (w0, Gamma0))));
-[ rewrite H2; rewrite H0 in Ok_Bg | eapply IHHT | intros]; eauto with ok_bg_rew;
-unfold open_t in *; unfold open_w in *.
+  (L_w := L_w \u  used_w_vars_Hyb ((w', nil) ::
+    emptyEquiv_Hyb (G0 & (w0, Gamma0))));
+[ rewrite H2; rewrite H0 in Ok_Bg | eapply IHHT | intros];
+eauto with ok_bg_hyb_rew;
+unfold open_t_Hyb in *; unfold open_w_Hyb in *.
 rewrite notin_union in H4; rewrite notin_singleton in H4; destruct H4;
-rewrite <- subst_order_irrelevant_bound;
-[ rewrite <- subst_t_comm | assumption ];
+rewrite <- subst_Hyb_order_irrelevant_bound;
+[ rewrite <- subst_t_Hyb_comm | assumption ];
 [ eapply H with (G0:=(w'0, (v',A)::nil)::G0) (w'0:=w')
   (Gamma':=Gamma') (A0:=A0) | | ]; auto;
-rew_app; rewrite H1 in H3; rew_app in *; simpl; try PPermut_simpl;
-apply BackgroundSubsetImpl with (G:= emptyEquiv (G0 & (w0, Gamma0))); auto;
-[exists ((w'0, (@nil (var*ty))):: nil); PPermut_simpl | ];
-assert ((w'0, nil) :: (w', nil)::emptyEquiv(G0 & (w0, Gamma0)) ~=~
-  (w', nil) :: (w'0, nil) :: emptyEquiv (G0 & (w0, Gamma0))) by auto;
-rewrite <- H7; apply ok_Bg_fresh_wo;
-[rewrite H0 in Ok_Bg; apply emptyEquiv_ok_Bg in Ok_Bg | ]; auto;
-  assert (emptyEquiv((w', (v, A0) :: Gamma') :: G0 & (w0, Gamma0)) ~=~
-    (w', nil) :: emptyEquiv (G0 & (w0, Gamma0))) by (simpl; auto);
+rew_app; rewrite H1 in H3; rew_app in *; simpl; try PPermut_Hyb_simpl;
+apply BackgroundSubsetImpl_Hyb with (G:= emptyEquiv_Hyb (G0 & (w0, Gamma0)));
+auto; [exists ((w'0, (@nil (var*ty))):: nil); PPermut_Hyb_simpl | ];
+assert ((w'0, nil) :: (w', nil)::emptyEquiv_Hyb(G0 & (w0, Gamma0)) ~=~
+  (w', nil) :: (w'0, nil) :: emptyEquiv_Hyb (G0 & (w0, Gamma0))) by auto;
+rewrite <- H7; apply ok_Bg_Hyb_fresh_wo;
+[rewrite H0 in Ok_Bg; apply emptyEquiv_Hyb_ok_Bg_Hyb in Ok_Bg | ]; auto;
+  assert (emptyEquiv_Hyb((w', (v, A0) :: Gamma') :: G0 & (w0, Gamma0)) ~=~
+    (w', nil) :: emptyEquiv_Hyb (G0 & (w0, Gamma0))) by (simpl; auto);
 rewrite <- H8;
 assert ((w0, Gamma0) :: G0 & (w', (v, A0) :: Gamma') ~=~
   ((w', (v, A0) :: Gamma') :: G0 & (w0, Gamma0))) by auto;
 rewrite <- H9; auto.
 
 (* letdia_get *)
-assert (w <> w0) by eauto with ok_bg_rew;
-eapply t_letdia_get_LF with (G:=G) (Gamma:=Gamma) (L_t := L_t \u \{v}) (A:=A)
-  (L_w:=L_w \u used_w_vars ((w0, nil) :: emptyEquiv (G & (w, Gamma)))); auto.
-apply ok_Bg_permut_no_last_spec with (v:=v) (A:=A0);
-apply ok_Bg_ppermut with (G:= (w, Gamma) :: G & (w0, Gamma0)); auto.
+assert (w <> w0) by eauto with ok_bg_hyb_rew;
+eapply t_letdia_get_Hyb with (G:=G) (Gamma:=Gamma) (L_t := L_t \u \{v}) (A:=A)
+  (L_w:=L_w \u used_w_vars_Hyb ((w0, nil) :: emptyEquiv_Hyb (G & (w, Gamma))));
+auto.
+apply ok_Bg_Hyb_permut_no_last_spec with (v:=v) (A:=A0);
+apply ok_Bg_Hyb_ppermut with (G:= (w, Gamma) :: G & (w0, Gamma0)); auto.
 eapply IHHT with (w':=w0) (Gamma':=Gamma1) (v:=v) (A0:=A0); auto.
 rew_app; rewrite <- H0 in H2; auto.
-intros; unfold open_t in *; unfold open_w in *;
+intros; unfold open_t_Hyb in *; unfold open_w_Hyb in *;
 rewrite notin_union in H5; rewrite notin_singleton in H5; destruct H5;
-rewrite <- subst_order_irrelevant_bound;
-[rewrite <- subst_t_comm | ]; auto.
+rewrite <- subst_Hyb_order_irrelevant_bound;
+[rewrite <- subst_t_Hyb_comm | ]; auto.
 eapply H with (v:=v) (A0:=A0); auto.
 rewrite <- H0 in H2;
-apply BackgroundSubsetImpl with (G:=emptyEquiv (G & (w, Gamma))); auto;
-[ exists ((w', (@ nil (var * ty)))::nil); PPermut_simpl | ];
-assert ((w0, nil) :: (w', nil) :: emptyEquiv (G & (w, Gamma)) ~=~
-  (w', nil) :: (w0, nil) ::emptyEquiv (G & (w, Gamma))) by PPermut_simpl;
+apply BackgroundSubsetImpl_Hyb with (G:=emptyEquiv_Hyb (G & (w, Gamma))); auto;
+[ exists ((w', (@ nil (var * ty)))::nil); PPermut_Hyb_simpl | ];
+assert ((w0, nil) :: (w', nil) :: emptyEquiv_Hyb (G & (w, Gamma)) ~=~
+  (w', nil) :: (w0, nil) ::emptyEquiv_Hyb (G & (w, Gamma)))
+by PPermut_Hyb_simpl;
 rewrite H8;
-apply ok_Bg_fresh_wo; [apply emptyEquiv_ok_Bg in Ok_Bg | auto];
+apply ok_Bg_Hyb_fresh_wo; [apply emptyEquiv_Hyb_ok_Bg_Hyb in Ok_Bg | auto];
 assert ((w, Gamma) :: G & (w0, Gamma0) ~=~ (w0, Gamma0):: G & (w, Gamma)) by
   auto;
 rewrite H9 in Ok_Bg; simpl in Ok_Bg; auto.
 
-assert (w <> w0) by eauto with ok_bg_rew;
+assert (w <> w0) by eauto with ok_bg_hyb_rew;
 destruct (eq_var_dec w w'); subst.
 (* = *)
 assert (G ~=~ G1 /\ Gamma *=* (v, A0) :: Gamma') by
-  (apply ok_Bg_impl_ppermut with (w:=w');
+  (apply ok_Bg_Hyb_impl_ppermut with (w:=w');
     [ | rewrite H0; rewrite <- H1]; eauto);
 destruct H7; rewrite H3; rewrite <- H7;
-apply t_letdia_get_LF with (G:=G) (Gamma:=Gamma') (L_t:=L_t \u \{v}) (A:=A)
-  (L_w:=L_w \u used_w_vars ((w', nil) :: emptyEquiv (G1 & (w0, Gamma0)))).
-eauto with ok_bg_rew.
+apply t_letdia_get_Hyb with (G:=G) (Gamma:=Gamma') (L_t:=L_t \u \{v}) (A:=A)
+  (L_w:=L_w \u used_w_vars_Hyb ((w', nil) ::
+    emptyEquiv_Hyb (G1 & (w0, Gamma0)))).
+eauto with ok_bg_hyb_rew.
 eapply IHHT with (v:=v) (A0:=A0); auto;
 rewrite H2 in H4; rewrite H7; auto.
-intros; unfold open_t in *; unfold open_w in *;
+intros; unfold open_t_Hyb in *; unfold open_w_Hyb in *;
 rewrite notin_union in H9; rewrite notin_singleton in H9; destruct H9;
-rewrite <- subst_order_irrelevant_bound;
-[ rewrite <- subst_t_comm | ]; auto.
+rewrite <- subst_Hyb_order_irrelevant_bound;
+[ rewrite <- subst_t_Hyb_comm | ]; auto.
 edestruct H with (v:=v) (w'0 := w'0) (Gamma1:=Gamma0) (A0:=A0)
   (v':=v') (M:=M0) as (Ha, Hb);
 auto.
 eapply Hb with (G0 := (w'0, (v',A)::nil) ::G) (w'1 := w') (Gamma':=Gamma');
-[ | auto |  | ]; try PPermut_simpl.
+[ | auto |  | ]; try PPermut_Hyb_simpl.
 rewrite H2 in H4; rewrite H7.
-apply BackgroundSubsetImpl with (G:=emptyEquiv (G1 & (w0, Gamma0))); auto.
-exists (((w'0, (@nil (prod var ty))) :: nil)); rew_app; simpl; auto;
-PPermut_simpl.
-assert ((w', nil) :: (w'0, nil) :: emptyEquiv (G1 & (w0, Gamma0)) ~=~
-  (w'0, nil) :: (w',nil) :: emptyEquiv (G1 & (w0, Gamma0))) by auto;
-rewrite H12; apply ok_Bg_fresh_wo; auto;
-assert ((w', nil) :: emptyEquiv (G1 & (w0, Gamma0)) ~=~
-  emptyEquiv ((w', Gamma) :: G & (w0, Gamma0))) by
+apply BackgroundSubsetImpl_Hyb with (G:=emptyEquiv_Hyb (G1 & (w0, Gamma0)));
+auto. exists (((w'0, (@nil (prod var ty))) :: nil)); rew_app; simpl; auto;
+PPermut_Hyb_simpl.
+assert ((w', nil) :: (w'0, nil) :: emptyEquiv_Hyb (G1 & (w0, Gamma0)) ~=~
+  (w'0, nil) :: (w',nil) :: emptyEquiv_Hyb (G1 & (w0, Gamma0))) by auto;
+rewrite H12; apply ok_Bg_Hyb_fresh_wo; auto;
+assert ((w', nil) :: emptyEquiv_Hyb (G1 & (w0, Gamma0)) ~=~
+  emptyEquiv_Hyb ((w', Gamma) :: G & (w0, Gamma0))) by
   (simpl in *; rewrite H7; auto);
-rewrite H13; apply emptyEquiv_ok_Bg in Ok_Bg; auto.
+rewrite H13; apply emptyEquiv_Hyb_ok_Bg_Hyb in Ok_Bg; auto.
 auto.
 (* <> *)
 assert (G & (w, Gamma) ~=~ G1 & (w', (v, A0) :: Gamma')) by
@@ -1038,93 +1049,98 @@ assert (G & (w, Gamma) ~=~ G1 & (w', (v, A0) :: Gamma')) by
 symmetry in H7;
 assert (exists Gamma0, exists GH, exists GT,
   Gamma0 *=* Gamma /\ G1 = GH & (w, Gamma0) ++ GT) by
-  (apply PPermut_split_neq with (w:=w') (Gamma:=(v,A0) :: Gamma') (G':=G);
+  (apply PPermut_Hyb_split_neq with (w:=w') (Gamma:=(v,A0) :: Gamma') (G':=G);
     auto);
 destruct H8 as (Gamma'', (GH, H8)); destruct H8 as (GT, H8);
 destruct H8.
-apply t_letdia_get_LF with (G:=GH++GT & (w', Gamma')) (Gamma:=Gamma) (A:=A)
-  (L_t:=L_t \u \{v}) (L_w:=L_w \u used_w_vars
-     ((w', nil) :: emptyEquiv (GH ++ GT ++ (w, Gamma) :: (w0, Gamma0) :: nil))).
+apply t_letdia_get_Hyb with (G:=GH++GT & (w', Gamma')) (Gamma:=Gamma) (A:=A)
+  (L_t:=L_t \u \{v}) (L_w:=L_w \u used_w_vars_Hyb
+     ((w', nil) :: emptyEquiv_Hyb
+       (GH ++ GT ++ (w, Gamma) :: (w0, Gamma0) :: nil))).
 assert (G & (w, Gamma) & (w0, Gamma0) ~=~ (w, Gamma) :: G & (w0, Gamma0)) by
   auto.
 rewrite <- H10 in Ok_Bg; rewrite <- H7 in Ok_Bg;
-subst; apply ok_Bg_ppermut with
+subst; apply ok_Bg_Hyb_ppermut with
   (G:=((w, Gamma) :: (GH & (w', Gamma') ++ GT) & (w0, Gamma0))); [ | rew_app];
 auto.
-apply ok_Bg_ppermut with
+apply ok_Bg_Hyb_ppermut with
   (G:= (((w, Gamma) :: (GH & (w0, Gamma0) ++ GT)) & (w', Gamma')));
-[rew_app; PPermut_simpl | apply ok_Bg_permut_no_last_spec with (v:=v)(A:=A0)];
-apply ok_Bg_ppermut with
+[rew_app; PPermut_Hyb_simpl | apply ok_Bg_Hyb_permut_no_last_spec
+  with (v:=v)(A:=A0)];
+apply ok_Bg_Hyb_ppermut with
   ((GH & (w, Gamma'') ++ GT) & (w', (v, A0) :: Gamma') & (w0, Gamma0));
-[ rew_app | ]; auto; try PPermut_simpl.
+[ rew_app | ]; auto; try PPermut_Hyb_simpl.
 eapply IHHT with (w1:=w) (Gamma1:=Gamma) (A0:=A0) (w':=w')
   (G0:=GH++GT & (w0,Gamma0)) (Gamma':=Gamma'); auto;
 [ symmetry; subst; rew_app in * | rew_app | ]; auto.
-PPermut_simpl; apply PPermut_last_rev_simpl with (a:=(w, Gamma));
-rewrite <- H7; PPermut_simpl.
+PPermut_Hyb_simpl; apply PPermut_Hyb_last_rev_simpl with (a:=(w, Gamma));
+rewrite <- H7; PPermut_Hyb_simpl.
 rewrite H2 in H4; rewrite H9 in H4;
 assert ((GH & (w, Gamma'') ++ GT) & (w0, Gamma0) ~=~
-  (GH ++ GT & (w0, Gamma0)) ++ nil & (w, Gamma)) by (rew_app; PPermut_simpl);
+  (GH ++ GT & (w0, Gamma0)) ++ nil & (w, Gamma))
+  by (rew_app; PPermut_Hyb_simpl);
 rewrite <- H10; auto.
-intros; unfold open_t in *; unfold open_w in *;
+intros; unfold open_t_Hyb in *; unfold open_w_Hyb in *;
 rewrite notin_union in H10; rewrite notin_singleton in H10; destruct H10;
-rewrite <- subst_order_irrelevant_bound;
-[rewrite <- subst_t_comm | ]; auto;
+rewrite <- subst_Hyb_order_irrelevant_bound;
+[rewrite <- subst_t_Hyb_comm | ]; auto;
 eapply H with (v':=v') (w':=w'0) (Gamma1:=Gamma0) (w1:=w0) (A0:=A0)
               (v:=v) (G0:=(w'0, (v', A) :: nil) :: (GH ++ GT) & (w, Gamma))
-              (w'0:=w') (Gamma':=Gamma'); auto; try PPermut_simpl.
-apply PPermut_last_rev_simpl with (a:=(w, Gamma)); rewrite <- H7;
-subst; PPermut_simpl.
+              (w'0:=w') (Gamma':=Gamma'); auto; try PPermut_Hyb_simpl.
+apply PPermut_Hyb_last_rev_simpl with (a:=(w, Gamma)); rewrite <- H7;
+subst; PPermut_Hyb_simpl.
 rew_app; rewrite H2 in H4; rewrite H9 in H4; simpl;
-apply BackgroundSubsetImpl with
-  (G:=emptyEquiv (GH ++ GT ++ (w, Gamma) :: (w0, Gamma0) :: nil)); auto.
+apply BackgroundSubsetImpl_Hyb with
+  (G:=emptyEquiv_Hyb (GH ++ GT ++ (w, Gamma) :: (w0, Gamma0) :: nil)); auto.
 assert (GH ++ GT ++ (w, Gamma) :: (w0, Gamma0) :: nil ~=~
-  (GH & (w, Gamma'') ++ GT) & (w0, Gamma0)) by (rew_app; PPermut_simpl);
+  (GH & (w, Gamma'') ++ GT) & (w0, Gamma0)) by (rew_app; PPermut_Hyb_simpl);
 rewrite H13; auto.
-exists ((w'0, (@nil (var*ty))) :: nil); PPermut_simpl.
+exists ((w'0, (@nil (var*ty))) :: nil); PPermut_Hyb_simpl.
 assert ((w, Gamma) :: G & (w0, Gamma0) ~=~ G0 & (w0, Gamma0)) by
   (rewrite <- H0; auto);
 rewrite H13 in Ok_Bg; rewrite H1 in Ok_Bg; subst;
 assert ((w', nil)
       :: (w'0, nil)
-         :: emptyEquiv (GH ++ GT ++ (w, Gamma) :: (w0, Gamma0) :: nil) ~=~
+         :: emptyEquiv_Hyb (GH ++ GT ++ (w, Gamma) :: (w0, Gamma0) :: nil) ~=~
       (w'0, nil)
       :: (w', nil)
-         :: emptyEquiv (GH ++ GT ++ (w, Gamma) :: (w0, Gamma0) :: nil)) by auto;
-rewrite H9; apply ok_Bg_fresh_wo;
+         :: emptyEquiv_Hyb (GH ++ GT ++ (w, Gamma) :: (w0, Gamma0) :: nil))
+by auto;
+rewrite H9; apply ok_Bg_Hyb_fresh_wo;
 assert (((GH & (w, Gamma'') ++ GT) & (w', (v, A0) :: Gamma')) & (w0, Gamma0) ~=~
   ((w', (v, A0) :: Gamma') :: GH ++ GT ++ (w, Gamma) :: nil) &  (w0, Gamma0)) by
-  (eapply PPermut_last_rev; auto; try PPermut_simpl);
+  (eapply PPermut_Hyb_last_rev; auto; try PPermut_Hyb_simpl);
 rew_app in *; [rewrite H14 in Ok_Bg | auto];
-apply emptyEquiv_ok_Bg in Ok_Bg; simpl in *; auto.
-symmetry; transitivity (G1 & (w', Gamma')); subst; rew_app in *; PPermut_simpl.
+apply emptyEquiv_Hyb_ok_Bg_Hyb in Ok_Bg; simpl in *; auto.
+symmetry; transitivity (G1 & (w', Gamma')); subst; rew_app in *;
+PPermut_Hyb_simpl.
 Existential 1 := v'.
 Existential 1 := Gamma.
 Existential 1 := v'.
 Existential 1 := Gamma.
 Qed.
 
-Lemma subst_t_preserv_types_inner:
+Lemma subst_t_Hyb_preserv_types_inner:
 forall G w Gamma A B M N v
-  (H_lc_t: lc_t_LF M)
-  (H_lc_w: lc_w_LF M)
+  (H_lc_t: lc_t_Hyb M)
+  (H_lc_w: lc_w_Hyb M)
   (HT: G |= (w, (v, A) :: Gamma) |- N ::: B)
-  (HM: emptyEquiv G |= (w, nil) |- M ::: A),
+  (HM: emptyEquiv_Hyb G |= (w, nil) |- M ::: A),
   G |= (w, Gamma) |- [M//fte v] N ::: B.
-intros; eapply subst_t_preserv_types with (Gamma := (v, A) :: Gamma); eauto.
+intros; eapply subst_t_Hyb_preserv_types with (Gamma := (v, A) :: Gamma); eauto.
 Qed.
 
-Lemma subst_t_preserv_types_outer:
+Lemma subst_t_Hyb_preserv_types_outer:
 forall G0 G G' G'' w w' Gamma Gamma' A B M N v
-  (H_lc_t: lc_t_LF M)
-  (H_lc_w: lc_w_LF M)
+  (H_lc_t: lc_t_Hyb M)
+  (H_lc_w: lc_w_Hyb M)
   (G0G: G ~=~ (G0 & (w', (v, A) :: Gamma')))
   (G0G': G' ~=~ (G0 & (w, Gamma)))
   (G0G'': G'' ~=~ (G0 & (w', Gamma')))
-  (HM: emptyEquiv G' |= (w', nil) |- M ::: A)
+  (HM: emptyEquiv_Hyb G' |= (w', nil) |- M ::: A)
   (HT: G |= (w, Gamma) |- N ::: B),
   G'' |= (w, Gamma) |- [M // fte v] N ::: B.
-intros; eapply subst_t_preserv_types; eauto.
+intros; eapply subst_t_Hyb_preserv_types; eauto.
 Qed.
 
 (*
@@ -1132,7 +1148,7 @@ Proof: induction on typing
   * for terms with world change: we again have to check whether the
   world which we will switch into is one of those in renaming
 *)
-Lemma rename_w_preserv_types:
+Lemma rename_w_Hyb_preserv_types:
 forall G w Gamma A M G' w' Gamma'
   (HT: G |= (w, Gamma) |- M ::: A),
   (* "new" substitution *)
@@ -1161,595 +1177,610 @@ simpl in *.
 constructor;
 [ rewrite H in Ok_Bg  |
   rewrite Mem_app_or_eq; left ]; auto;
-eapply ok_Bg_split2; eauto.
+eapply ok_Bg_Hyb_split2; eauto.
 constructor;
 [ rewrite H in Ok_Bg |
   rewrite Mem_app_or_eq; right ]; auto;
-eapply ok_Bg_split2; eauto.
+eapply ok_Bg_Hyb_split2; eauto.
 constructor;
 [ rewrite H in Ok_Bg; rewrite H0 | ]; auto;
-eapply ok_Bg_split3; eauto.
+eapply ok_Bg_Hyb_split3; eauto.
 (* lam *)
-apply t_lam_LF with (L := L);
-[ rewrite H0 in Ok_Bg; eapply ok_Bg_split2; eauto |
-  intros; unfold open_t in *];
-rewrite subst_order_irrelevant_free; simpl; auto;
+apply t_lam_Hyb with (L := L);
+[ rewrite H0 in Ok_Bg; eapply ok_Bg_Hyb_split2; eauto |
+  intros; unfold open_t_Hyb in *];
+rewrite subst_Hyb_order_irrelevant_free; simpl; auto;
 apply H with (v':=v') (G':=G') (Gamma := (v',A)::Gamma0); auto.
-apply t_lam_LF with (L := L);
-[ rewrite H0 in Ok_Bg; eapply ok_Bg_split2; eauto |
-  intros]; unfold open_t in *;
-rewrite subst_order_irrelevant_free;
+apply t_lam_Hyb with (L := L);
+[ rewrite H0 in Ok_Bg; eapply ok_Bg_Hyb_split2; eauto |
+  intros]; unfold open_t_Hyb in *;
+rewrite subst_Hyb_order_irrelevant_free;
 edestruct H; eauto; destruct H3;
-[ apply ContextPermutImpl with (Gamma := (Gamma' ++ (v', A) :: Gamma0));
+[ apply ContextPermutImpl_Hyb with (Gamma := (Gamma' ++ (v', A) :: Gamma0));
   [permut_simpl | ] | simpl; apply notin_empty ]; eauto.
-apply t_lam_LF with (L := L);
+apply t_lam_Hyb with (L := L);
 [ rewrite H0 in Ok_Bg |
   intros];
-rewrite H1; try eapply ok_Bg_split3; eauto;
-unfold open_t in *;
-rewrite subst_order_irrelevant_free;
+rewrite H1; try eapply ok_Bg_Hyb_split3; eauto;
+unfold open_t_Hyb in *;
+rewrite subst_Hyb_order_irrelevant_free;
 edestruct H; eauto; destruct H4;
 eauto;
 simpl; apply notin_empty.
 
 (* appl *)
-apply t_appl_LF with (A:=A);
+apply t_appl_Hyb with (A:=A);
 [ rewrite H in Ok_Bg |
   apply IHHT1 with (Gamma:=Gamma0) |
   apply IHHT2 with (Gamma:=Gamma0) ];
-eauto; eapply ok_Bg_split2; eauto.
-apply t_appl_LF with (A:=A);
+eauto; eapply ok_Bg_Hyb_split2; eauto.
+apply t_appl_Hyb with (A:=A);
 [ rewrite H in Ok_Bg |
   apply IHHT1 with (Gamma:=Gamma0) |
   apply IHHT2 with (Gamma:=Gamma0) ];
-eauto; eapply ok_Bg_split2; eauto.
-apply t_appl_LF with (A:=A);
+eauto; eapply ok_Bg_Hyb_split2; eauto.
+apply t_appl_Hyb with (A:=A);
 [ rewrite H in Ok_Bg; rewrite H0 |
   eapply IHHT1 |
   eapply IHHT2 ]; eauto;
-eapply ok_Bg_split3; eauto.
+eapply ok_Bg_Hyb_split3; eauto.
 
 (* box *)
-apply t_box_LF with (L:=\{w'} \u L);
-[ rewrite H0 in Ok_Bg; eapply ok_Bg_split4; eauto |
+apply t_box_Hyb with (L:=\{w'} \u L);
+[ rewrite H0 in Ok_Bg; eapply ok_Bg_Hyb_split4; eauto |
   intros];
-unfold open_w in *; rewrite notin_union in H1; destruct H1;
-rewrite notin_singleton in *; rewrite <- subst_w_comm; auto;
-eapply H; eauto; PPermut_simpl.
-apply t_box_LF with (L:=\{w0} \u L);
-[ rewrite H0 in Ok_Bg; apply ok_Bg_split4 with (w:=w0);
-  apply ok_Bg_ppermut with (G:=G' & (w', Gamma') & (w0, Gamma0)); auto |
-  intros]; try PPermut_simpl;
-unfold open_w in *; rewrite notin_union in H1; destruct H1;
-rewrite notin_singleton in *; rewrite <- subst_w_comm; auto;
+unfold open_w_Hyb in *; rewrite notin_union in H1; destruct H1;
+rewrite notin_singleton in *; rewrite <- subst_w_Hyb_comm; auto;
+eapply H; eauto; PPermut_Hyb_simpl.
+apply t_box_Hyb with (L:=\{w0} \u L);
+[ rewrite H0 in Ok_Bg; apply ok_Bg_Hyb_split4 with (w:=w0);
+  apply ok_Bg_Hyb_ppermut with (G:=G' & (w', Gamma') & (w0, Gamma0)); auto |
+  intros]; try PPermut_Hyb_simpl;
+unfold open_w_Hyb in *; rewrite notin_union in H1; destruct H1;
+rewrite notin_singleton in *; rewrite <- subst_w_Hyb_comm; auto;
 eapply H; eauto.
-apply t_box_LF with (L:=\{w''} \u L);
-[ rewrite H0 in Ok_Bg; rewrite H1; eapply ok_Bg_split6; eauto |
+apply t_box_Hyb with (L:=\{w''} \u L);
+[ rewrite H0 in Ok_Bg; rewrite H1; eapply ok_Bg_Hyb_split6; eauto |
   intros];
-unfold open_w in *;
+unfold open_w_Hyb in *;
 rewrite notin_union in H2; destruct H2;
 rewrite notin_singleton in *;
-rewrite <- subst_w_comm; auto;
+rewrite <- subst_w_Hyb_comm; auto;
 eapply H with (G0:=G0 & (w0, Gamma0)) (Gamma':=Gamma') (Gamma'':=Gamma''); auto;
-try PPermut_simpl; rewrite H0; PPermut_simpl.
+try PPermut_Hyb_simpl; rewrite H0; PPermut_Hyb_simpl.
 
 (* unbox *)
 case_if.
 inversion H0; subst; rewrite H in Ok_Bg;
-apply ok_Bg_first_last_neq in Ok_Bg; elim Ok_Bg; auto.
+apply ok_Bg_Hyb_first_last_neq in Ok_Bg; elim Ok_Bg; auto.
 constructor; [rewrite H in Ok_Bg | apply IHHT with (Gamma:=Gamma0)]; eauto;
-eapply ok_Bg_split2; eauto.
+eapply ok_Bg_Hyb_split2; eauto.
 
 case_if; constructor;
 [ rewrite H in Ok_Bg |
   apply IHHT with (Gamma:=Gamma0) ]; eauto;
-eapply ok_Bg_split2; eauto.
+eapply ok_Bg_Hyb_split2; eauto.
 
 case_if.
 inversion H1; subst; rewrite H in Ok_Bg;
-apply ok_Bg_first_last_neq in Ok_Bg; elim Ok_Bg; auto.
+apply ok_Bg_Hyb_first_last_neq in Ok_Bg; elim Ok_Bg; auto.
 constructor; [rewrite H0; rewrite H in Ok_Bg | eapply IHHT]; eauto;
-eapply ok_Bg_split3; eauto.
+eapply ok_Bg_Hyb_split3; eauto.
 
 (* unbox_fetch *)
 case_if.
 inversion H1; subst;
 assert (G ~=~ G'0 /\ Gamma *=* Gamma'0) as HP by
-  (apply ok_Bg_impl_ppermut with (w:=w'0);
+  (apply ok_Bg_Hyb_impl_ppermut with (w:=w'0);
    [eauto | rewrite H; rewrite H0; auto]);
 destruct HP; constructor.
-rewrite <- H2; apply ok_Bg_split2 with (w:=w'0);
-eapply ok_Bg_permut; eauto.
-apply ContextPermutImpl with (Gamma:=Gamma0 ++ Gamma);
+rewrite <- H2; apply ok_Bg_Hyb_split2 with (w:=w'0);
+eapply ok_Bg_Hyb_permut; eauto.
+apply ContextPermutImpl_Hyb with (Gamma:=Gamma0 ++ Gamma);
 [ permut_simpl |
   apply IHHT] ; auto.
 assert (G'0 & (w'0, Gamma'0) ~=~ G & (w, Gamma)) by
   (symmetry; transitivity G'; auto);
 assert (exists Gamma'', exists GH, exists GT,
   Gamma'' *=* Gamma /\ G'0 = GH & (w, Gamma'') ++ GT) as Split by
-  (eapply PPermut_split_neq; eauto; right; intro; subst; elim H1; reflexivity);
+  (eapply PPermut_Hyb_split_neq; eauto; right; intro; subst;
+    elim H1; reflexivity);
 destruct Split as (Gamma'', (GH, Split)); destruct Split as (GT, H3);
 destruct H3 as (H3a, H3b).
-apply t_unbox_fetch_LF with (G:=GH++GT) (Gamma:=Gamma).
+apply t_unbox_fetch_Hyb with (G:=GH++GT) (Gamma:=Gamma).
 assert ((w, Gamma) :: G & (w0, Gamma0) ~=~ G & (w, Gamma) & (w0, Gamma0)) by
   auto.
 rewrite H3 in Ok_Bg; rewrite <- H2 in Ok_Bg; rew_app in *;
-assert (GH & (w, Gamma) ++ GT ~=~ (w, Gamma) :: GH ++ GT) by (PPermut_simpl);
-apply ok_Bg_ppermut with
+assert (GH & (w, Gamma) ++ GT ~=~ (w, Gamma) :: GH ++ GT)
+  by (PPermut_Hyb_simpl);
+apply ok_Bg_Hyb_ppermut with
   (G:= (GH & (w, Gamma) ++ GT) & (w0, Gamma0 ++ Gamma'0));
 [ rewrite H4 |
-  apply ok_Bg_split4 with (w:=w'0)]; rew_app; auto.
+  apply ok_Bg_Hyb_split4 with (w:=w'0)]; rew_app; auto.
 subst; rew_app in *;
-apply ok_Bg_ppermut with
+apply ok_Bg_Hyb_ppermut with
   (G:=(GH ++ (w, Gamma'') :: GT ++ (w'0, Gamma'0) :: (w0, Gamma0) :: nil));
-try PPermut_simpl; auto.
-eapply IHHT with (w1:=w) (Gamma1:=Gamma); auto; subst; symmetry; PPermut_simpl;
-apply PPermut_last_rev_simpl with (a:=(w, Gamma)); rew_app in *; auto;
-rew_app; auto; rewrite <- H2; PPermut_simpl.
-apply PPermut_last_rev_simpl with (a:=(w, Gamma)); rew_app in *; auto; subst;
-PPermut_simpl.
+try PPermut_Hyb_simpl; auto.
+eapply IHHT with (w1:=w) (Gamma1:=Gamma); auto; subst; symmetry;
+PPermut_Hyb_simpl;
+apply PPermut_Hyb_last_rev_simpl with (a:=(w, Gamma)); rew_app in *; auto;
+rew_app; auto; rewrite <- H2; PPermut_Hyb_simpl.
+apply PPermut_Hyb_last_rev_simpl with (a:=(w, Gamma)); rew_app in *;
+auto; subst; PPermut_Hyb_simpl.
 
 case_if;
-[ inversion H1; subst; apply ok_Bg_first_last_neq in Ok_Bg; elim Ok_Bg; auto |
-  destruct (eq_var_dec w w'0)].
+[ inversion H1; subst; apply ok_Bg_Hyb_first_last_neq in Ok_Bg;
+  elim Ok_Bg; auto | destruct (eq_var_dec w w'0)].
 subst; assert (G ~=~ G'0 /\ Gamma *=* Gamma'0) by
-  (apply ok_Bg_impl_ppermut with (w:=w'0); [ | rewrite <- H0]; eauto);
+  (apply ok_Bg_Hyb_impl_ppermut with (w:=w'0); [ | rewrite <- H0]; eauto);
 destruct H2; constructor.
-rewrite <- H2; apply ok_Bg_permut with (Ctx := (Gamma ++ Gamma0)); eauto;
-eapply ok_Bg_split2; eauto.
-apply ContextPermutImpl with (Gamma:=Gamma ++ Gamma0);
+rewrite <- H2; apply ok_Bg_Hyb_permut with (Ctx := (Gamma ++ Gamma0)); eauto;
+eapply ok_Bg_Hyb_split2; eauto.
+apply ContextPermutImpl_Hyb with (Gamma:=Gamma ++ Gamma0);
 [ permut_simpl |
   eapply IHHT with (w:=w'0) (Gamma1:=Gamma) (Gamma':=Gamma0)] ; auto.
 assert (G'0 & (w'0, Gamma'0) ~=~ G & (w, Gamma)) by
   (symmetry; transitivity G'; auto);
 assert (exists Gamma'', exists GH, exists GT,
   Gamma'' *=* Gamma /\ G'0 = GH & (w, Gamma'') ++ GT) as Split by
-  (eapply PPermut_split_neq; eauto; right; intro; subst; elim H1; reflexivity);
+  (eapply PPermut_Hyb_split_neq; eauto; right; intro; subst;
+    elim H1; reflexivity);
 destruct Split as (Gamma'', (GH, Split));
 destruct Split as (GT, (Ha, Hb)); subst;
-apply t_unbox_fetch_LF with (G:=GH++GT) (Gamma:=Gamma).
+apply t_unbox_fetch_Hyb with (G:=GH++GT) (Gamma:=Gamma).
 assert (GH & (w, Gamma) ++ GT ~=~ (w, Gamma) :: GH ++ GT)
-  by PPermut_simpl;
-apply ok_Bg_ppermut with
+  by PPermut_Hyb_simpl;
+apply ok_Bg_Hyb_ppermut with
   (G:= (GH & (w, Gamma'') ++ GT) & (w'0, Gamma0 ++ Gamma'0));
-[ PPermut_simpl | apply ok_Bg_split4 with (w:=w0)]; rew_app; auto.
+[ PPermut_Hyb_simpl | apply ok_Bg_Hyb_split4 with (w:=w0)]; rew_app; auto.
 assert ((w, Gamma) :: G & (w0, Gamma0) ~=~
   (G & (w, Gamma)) & (w0, Gamma0)) by auto;
 rewrite H4 in Ok_Bg; rewrite <- H2 in Ok_Bg; rew_app in *;
 remember (GH ++ (w, Gamma'') :: GT) as GHT;
 assert (GH ++ (w, Gamma'') :: GT ++ (w0, Gamma'0) :: (w'0, Gamma0) :: nil ~=~
   GHT & (w0, Gamma'0) & (w'0, Gamma0)) by (subst; rew_app; auto).
-rewrite H5; apply ok_Bg_swap_worlds; subst; rew_app in *; auto.
-eapply IHHT; auto; PPermut_simpl.
-apply PPermut_last_rev_simpl with (a:=(w, Gamma)); rew_app in *;
-rewrite H; rewrite H0; PPermut_simpl.
-transitivity (GH & (w, Gamma) ++ GT); PPermut_simpl.
+rewrite H5; apply ok_Bg_Hyb_swap_worlds; subst; rew_app in *; auto.
+eapply IHHT; auto; PPermut_Hyb_simpl.
+apply PPermut_Hyb_last_rev_simpl with (a:=(w, Gamma)); rew_app in *;
+rewrite H; rewrite H0; PPermut_Hyb_simpl.
+transitivity (GH & (w, Gamma) ++ GT); PPermut_Hyb_simpl.
 
 case_if.
 inversion H2; subst;
 assert (G ~=~ G0 & (w'0, Gamma'0) /\ Gamma *=* Gamma'') by
-  (apply ok_Bg_impl_ppermut with (w:=w''); [ | rewrite H; rewrite H0]; eauto);
-destruct H3; apply t_unbox_fetch_LF with (G:=G0) (Gamma := Gamma'0 ++ Gamma);
+  (apply ok_Bg_Hyb_impl_ppermut with (w:=w''); [ | rewrite H; rewrite H0];
+    eauto);
+destruct H3; apply t_unbox_fetch_Hyb with (G:=G0) (Gamma := Gamma'0 ++ Gamma);
 [ rewrite H3 in Ok_Bg | apply IHHT | rewrite H1]; eauto.
-apply ok_Bg_split9 with (w':=w'');
-apply ok_Bg_ppermut with (G:= (w'', Gamma)::G0 & (w'0, Gamma'0) & (w0, Gamma0));
-eauto; PPermut_simpl.
-rewrite H3; PPermut_simpl.
+apply ok_Bg_Hyb_split9 with (w':=w'');
+apply ok_Bg_Hyb_ppermut with (G:= (w'', Gamma)::G0 & (w'0, Gamma'0) &
+  (w0, Gamma0));
+eauto; PPermut_Hyb_simpl.
+rewrite H3; PPermut_Hyb_simpl.
 destruct (eq_var_dec w w'0).
 subst; assert (G ~=~ G0 & (w'', Gamma'') /\ Gamma *=* Gamma'0) by
-  (apply ok_Bg_impl_ppermut with (w:=w'0); [ | rewrite H; rewrite H0];
-   eauto; PPermut_simpl);
+  (apply ok_Bg_Hyb_impl_ppermut with (w:=w'0); [ | rewrite H; rewrite H0];
+   eauto; PPermut_Hyb_simpl);
 destruct H3;
-apply t_unbox_fetch_LF with (G:=G0) (Gamma := Gamma ++ Gamma'');
+apply t_unbox_fetch_Hyb with (G:=G0) (Gamma := Gamma ++ Gamma'');
 [ rewrite H3 in Ok_Bg |
   eapply IHHT with (G':=G0 & (w0, Gamma0)) (Gamma' := Gamma'') |
   rewrite H1]; eauto.
-eapply ok_Bg_split9; eauto.
-rewrite H3; PPermut_simpl.
+eapply ok_Bg_Hyb_split9; eauto.
+rewrite H3; PPermut_Hyb_simpl.
 assert (G0 & (w'0, Gamma'0) & (w'', Gamma'')  ~=~ G & (w, Gamma)) by
   (symmetry; transitivity G'; auto);
 assert (exists Gamma'', exists GH, exists GT,
   Gamma'' *=* Gamma /\ G0 & (w'0, Gamma'0) = GH & (w, Gamma'') ++ GT)
   as Split.
-apply PPermut_split_neq with (w:=w'')
+apply PPermut_Hyb_split_neq with (w:=w'')
   (Gamma:=Gamma'') (G':= G); auto; right; intro; subst; elim H2; auto.
 assert (exists Gamma'', exists GH, exists GT,
   Gamma'' *=* Gamma /\ G0 = GH & (w, Gamma'') ++ GT) as Split' by
   (destruct Split as (Gamma''', (GH, Split));
     destruct Split as (GT, (Ha, Hb));
-   apply PPermut_split_neq with (w:=w'0) (Gamma:=Gamma'0) (G':=GH ++ GT);
+   apply PPermut_Hyb_split_neq with (w:=w'0) (Gamma:=Gamma'0) (G':=GH ++ GT);
    [ rew_app; transitivity (GH & (w, Gamma) ++ GT) |
      right; intro; subst; elim n]; auto; rewrite Hb; auto);
 destruct Split' as (Gamma''',(GH, Split'));
 destruct Split' as (GT, (Ha, Hb));
-apply t_unbox_fetch_LF with (G:=GH++GT & (w'0, Gamma'0++Gamma''))
+apply t_unbox_fetch_Hyb with (G:=GH++GT & (w'0, Gamma'0++Gamma''))
   (Gamma:=Gamma).
-apply ok_Bg_ppermut with (G':=(G' & (w0, Gamma0))) in Ok_Bg;
+apply ok_Bg_Hyb_ppermut with (G':=(G' & (w0, Gamma0))) in Ok_Bg;
 [ | rewrite <- H; auto]; rewrite H0 in Ok_Bg; subst G0.
-apply ok_Bg_ppermut with
+apply ok_Bg_Hyb_ppermut with
   (G:= (GH & (w, Gamma''') ++ GT) & (w'0, Gamma'0 ++ Gamma'') & (w0, Gamma0));
-[ rew_app | ]; auto; try PPermut_simpl; eapply ok_Bg_split6; eauto.
+[ rew_app | ]; auto; try PPermut_Hyb_simpl; eapply ok_Bg_Hyb_split6; eauto.
 eapply IHHT with (w1:=w) (Gamma1:=Gamma) (G0:=GH++GT & (w0,Gamma0))
   (Gamma':=Gamma'0) (Gamma'':=Gamma''); auto.
-PPermut_simpl. apply PPermut_last_rev_simpl with (a:=(w, Gamma));
-rewrite <- H3; subst; PPermut_simpl.
-PPermut_simpl.
-rewrite H1; subst; PPermut_simpl.
+PPermut_Hyb_simpl. apply PPermut_Hyb_last_rev_simpl with (a:=(w, Gamma));
+rewrite <- H3; subst; PPermut_Hyb_simpl.
+PPermut_Hyb_simpl.
+rewrite H1; subst; PPermut_Hyb_simpl.
 
 (* here *)
 case_if.
 inversion H0; subst; rewrite H in Ok_Bg;
-apply ok_Bg_first_last_neq in Ok_Bg; elim Ok_Bg; auto.
+apply ok_Bg_Hyb_first_last_neq in Ok_Bg; elim Ok_Bg; auto.
 constructor;
 [ rewrite H in Ok_Bg | apply IHHT with (Gamma:=Gamma0)]; eauto;
-eapply ok_Bg_split2; eauto.
+eapply ok_Bg_Hyb_split2; eauto.
 
 case_if; constructor;
 [ rewrite H in Ok_Bg |
   apply IHHT with (Gamma:=Gamma0) ]; eauto;
-eapply ok_Bg_split2; eauto.
+eapply ok_Bg_Hyb_split2; eauto.
 
 case_if.
 inversion H1; subst; rewrite H in Ok_Bg;
-apply ok_Bg_first_last_neq in Ok_Bg; elim Ok_Bg; auto.
+apply ok_Bg_Hyb_first_last_neq in Ok_Bg; elim Ok_Bg; auto.
 constructor; [rewrite H0; rewrite H in Ok_Bg | eapply IHHT]; eauto;
-eapply ok_Bg_split3; eauto.
+eapply ok_Bg_Hyb_split3; eauto.
 
 (* get_here *)
 case_if.
 inversion H1; subst;
 assert (G ~=~ G'0 /\ Gamma *=* Gamma'0) as HP by
-  (apply ok_Bg_impl_ppermut with (w:=w'0);
+  (apply ok_Bg_Hyb_impl_ppermut with (w:=w'0);
    [eauto | rewrite H; rewrite H0; auto]);
 destruct HP; constructor.
-rewrite <- H2; apply ok_Bg_split2 with (w:=w'0);
-eapply ok_Bg_permut; eauto.
-apply ContextPermutImpl with (Gamma:=Gamma0 ++ Gamma);
+rewrite <- H2; apply ok_Bg_Hyb_split2 with (w:=w'0);
+eapply ok_Bg_Hyb_permut; eauto.
+apply ContextPermutImpl_Hyb with (Gamma:=Gamma0 ++ Gamma);
 [ permut_simpl |
   apply IHHT] ; auto.
 assert (G'0 & (w'0, Gamma'0) ~=~ G & (w, Gamma)) by
   (symmetry; transitivity G'; auto);
 assert (exists Gamma'', exists GH, exists GT,
   Gamma'' *=* Gamma /\ G'0 = GH & (w, Gamma'') ++ GT) as Split by
-  (eapply PPermut_split_neq; eauto; right; intro; subst; elim H1; reflexivity);
+  (eapply PPermut_Hyb_split_neq; eauto; right; intro; subst; elim H1;
+    reflexivity);
 destruct Split as (Gamma'', (GH, Split)); destruct Split as (GT, H3);
 destruct H3 as (H3a, H3b).
-apply t_get_here_LF with (G:=GH++GT) (Gamma:=Gamma).
+apply t_get_here_Hyb with (G:=GH++GT) (Gamma:=Gamma).
 assert ((w, Gamma) :: G & (w0, Gamma0) ~=~ G & (w, Gamma) & (w0, Gamma0)) by
   auto.
 rewrite H3 in Ok_Bg; rewrite <- H2 in Ok_Bg; rew_app in *;
-assert (GH & (w, Gamma) ++ GT ~=~ (w, Gamma) :: GH ++ GT) by (PPermut_simpl);
-apply ok_Bg_ppermut with
+assert (GH & (w, Gamma) ++ GT ~=~ (w, Gamma) :: GH ++ GT)
+  by (PPermut_Hyb_simpl);
+apply ok_Bg_Hyb_ppermut with
   (G:= (GH & (w, Gamma) ++ GT) & (w0, Gamma0 ++ Gamma'0));
 [ rewrite H4 |
-  apply ok_Bg_split4 with (w:=w'0)]; rew_app; auto.
+  apply ok_Bg_Hyb_split4 with (w:=w'0)]; rew_app; auto.
 subst; rew_app in *;
-apply ok_Bg_ppermut with
+apply ok_Bg_Hyb_ppermut with
   (G:=(GH ++ (w, Gamma'') :: GT ++ (w'0, Gamma'0) :: (w0, Gamma0) :: nil));
-try PPermut_simpl; auto.
-eapply IHHT with (w1:=w) (Gamma1:=Gamma); auto; subst; symmetry; PPermut_simpl;
-apply PPermut_last_rev_simpl with (a:=(w, Gamma)); rew_app in *; auto;
-rew_app; auto; rewrite <- H2; PPermut_simpl.
-apply PPermut_last_rev_simpl with (a:=(w, Gamma)); rew_app in *; auto; subst;
-PPermut_simpl.
+try PPermut_Hyb_simpl; auto.
+eapply IHHT with (w1:=w) (Gamma1:=Gamma); auto; subst; symmetry;
+PPermut_Hyb_simpl;
+apply PPermut_Hyb_last_rev_simpl with (a:=(w, Gamma)); rew_app in *; auto;
+rew_app; auto; rewrite <- H2; PPermut_Hyb_simpl.
+apply PPermut_Hyb_last_rev_simpl with (a:=(w, Gamma)); rew_app in *; auto;
+subst; PPermut_Hyb_simpl.
 
 case_if;
-[ inversion H1; subst; apply ok_Bg_first_last_neq in Ok_Bg; elim Ok_Bg; auto |
-  destruct (eq_var_dec w w'0)].
+[ inversion H1; subst; apply ok_Bg_Hyb_first_last_neq in Ok_Bg; elim Ok_Bg;
+  auto | destruct (eq_var_dec w w'0)].
 subst; assert (G ~=~ G'0 /\ Gamma *=* Gamma'0) by
-  (apply ok_Bg_impl_ppermut with (w:=w'0); [ | rewrite <- H0]; eauto);
+  (apply ok_Bg_Hyb_impl_ppermut with (w:=w'0); [ | rewrite <- H0]; eauto);
 destruct H2; constructor.
-rewrite <- H2; apply ok_Bg_permut with (Ctx := (Gamma ++ Gamma0)); eauto;
-eapply ok_Bg_split2; eauto.
-apply ContextPermutImpl with (Gamma:=Gamma ++ Gamma0);
+rewrite <- H2; apply ok_Bg_Hyb_permut with (Ctx := (Gamma ++ Gamma0)); eauto;
+eapply ok_Bg_Hyb_split2; eauto.
+apply ContextPermutImpl_Hyb with (Gamma:=Gamma ++ Gamma0);
 [ permut_simpl |
   eapply IHHT with (w:=w'0) (Gamma1:=Gamma) (Gamma':=Gamma0)] ; auto.
 assert (G'0 & (w'0, Gamma'0) ~=~ G & (w, Gamma)) by
   (symmetry; transitivity G'; auto);
 assert (exists Gamma'', exists GH, exists GT,
   Gamma'' *=* Gamma /\ G'0 = GH & (w, Gamma'') ++ GT) as Split by
-  (eapply PPermut_split_neq; eauto; right; intro; subst; elim H1; reflexivity);
+  (eapply PPermut_Hyb_split_neq; eauto; right; intro; subst; elim H1;
+    reflexivity);
 destruct Split as (Gamma'', (GH, Split));
 destruct Split as (GT, (Ha, Hb)); subst;
-apply t_get_here_LF with (G:=GH++GT) (Gamma:=Gamma).
+apply t_get_here_Hyb with (G:=GH++GT) (Gamma:=Gamma).
 assert (GH & (w, Gamma) ++ GT ~=~ (w, Gamma) :: GH ++ GT)
-  by PPermut_simpl;
-apply ok_Bg_ppermut with
+  by PPermut_Hyb_simpl;
+apply ok_Bg_Hyb_ppermut with
   (G:= (GH & (w, Gamma'') ++ GT) & (w'0, Gamma0 ++ Gamma'0));
-[ PPermut_simpl | apply ok_Bg_split4 with (w:=w0)]; rew_app; auto.
+[ PPermut_Hyb_simpl | apply ok_Bg_Hyb_split4 with (w:=w0)]; rew_app; auto.
 assert ((w, Gamma) :: G & (w0, Gamma0) ~=~
   (G & (w, Gamma)) & (w0, Gamma0)) by auto;
 rewrite H4 in Ok_Bg; rewrite <- H2 in Ok_Bg; rew_app in *;
 remember (GH ++ (w, Gamma'') :: GT) as GHT;
 assert (GH ++ (w, Gamma'') :: GT ++ (w0, Gamma'0) :: (w'0, Gamma0) :: nil ~=~
   GHT & (w0, Gamma'0) & (w'0, Gamma0)) by (subst; rew_app; auto).
-rewrite H5; apply ok_Bg_swap_worlds; subst; rew_app in *; auto.
-eapply IHHT; auto; PPermut_simpl.
-apply PPermut_last_rev_simpl with (a:=(w, Gamma)); rew_app in *;
-rewrite H; rewrite H0; PPermut_simpl.
-transitivity (GH & (w, Gamma) ++ GT); PPermut_simpl.
+rewrite H5; apply ok_Bg_Hyb_swap_worlds; subst; rew_app in *; auto.
+eapply IHHT; auto; PPermut_Hyb_simpl.
+apply PPermut_Hyb_last_rev_simpl with (a:=(w, Gamma)); rew_app in *;
+rewrite H; rewrite H0; PPermut_Hyb_simpl.
+transitivity (GH & (w, Gamma) ++ GT); PPermut_Hyb_simpl.
 
 case_if.
 inversion H2; subst;
 assert (G ~=~ G0 & (w'0, Gamma'0) /\ Gamma *=* Gamma'') by
-  (apply ok_Bg_impl_ppermut with (w:=w''); [ | rewrite H; rewrite H0]; eauto);
-destruct H3; apply t_get_here_LF with (G:=G0) (Gamma := Gamma'0 ++ Gamma);
+  (apply ok_Bg_Hyb_impl_ppermut with (w:=w''); [ | rewrite H; rewrite H0]; eauto);
+destruct H3; apply t_get_here_Hyb with (G:=G0) (Gamma := Gamma'0 ++ Gamma);
 [ rewrite H3 in Ok_Bg | apply IHHT | rewrite H1]; eauto.
-apply ok_Bg_split9 with (w':=w'');
-apply ok_Bg_ppermut with (G:= (w'', Gamma)::G0 & (w'0, Gamma'0) & (w0, Gamma0));
-eauto; PPermut_simpl.
-rewrite H3; PPermut_simpl.
+apply ok_Bg_Hyb_split9 with (w':=w'');
+apply ok_Bg_Hyb_ppermut with (G:= (w'', Gamma)::G0 & (w'0, Gamma'0) &
+  (w0, Gamma0));
+eauto; PPermut_Hyb_simpl.
+rewrite H3; PPermut_Hyb_simpl.
 destruct (eq_var_dec w w'0).
 subst; assert (G ~=~ G0 & (w'', Gamma'') /\ Gamma *=* Gamma'0) by
-  (apply ok_Bg_impl_ppermut with (w:=w'0); [ | rewrite H; rewrite H0];
-   eauto; PPermut_simpl);
+  (apply ok_Bg_Hyb_impl_ppermut with (w:=w'0); [ | rewrite H; rewrite H0];
+   eauto; PPermut_Hyb_simpl);
 destruct H3;
-apply t_get_here_LF with (G:=G0) (Gamma := Gamma ++ Gamma'');
+apply t_get_here_Hyb with (G:=G0) (Gamma := Gamma ++ Gamma'');
 [ rewrite H3 in Ok_Bg |
   eapply IHHT with (G':=G0 & (w0, Gamma0)) (Gamma' := Gamma'') |
   rewrite H1]; eauto.
-eapply ok_Bg_split9; eauto.
-rewrite H3; PPermut_simpl.
+eapply ok_Bg_Hyb_split9; eauto.
+rewrite H3; PPermut_Hyb_simpl.
 assert (G0 & (w'0, Gamma'0) & (w'', Gamma'')  ~=~ G & (w, Gamma)) by
   (symmetry; transitivity G'; auto);
 assert (exists Gamma'', exists GH, exists GT,
   Gamma'' *=* Gamma /\ G0 & (w'0, Gamma'0) = GH & (w, Gamma'') ++ GT)
   as Split.
-apply PPermut_split_neq with (w:=w'')
+apply PPermut_Hyb_split_neq with (w:=w'')
   (Gamma:=Gamma'') (G':= G); auto; right; intro; subst; elim H2; auto.
 assert (exists Gamma'', exists GH, exists GT,
   Gamma'' *=* Gamma /\ G0 = GH & (w, Gamma'') ++ GT) as Split' by
   (destruct Split as (Gamma''', (GH, Split));
     destruct Split as (GT, (Ha, Hb));
-   apply PPermut_split_neq with (w:=w'0) (Gamma:=Gamma'0) (G':=GH ++ GT);
+   apply PPermut_Hyb_split_neq with (w:=w'0) (Gamma:=Gamma'0) (G':=GH ++ GT);
    [ rew_app; transitivity (GH & (w, Gamma) ++ GT) |
      right; intro; subst; elim n]; auto; rewrite Hb; auto);
 destruct Split' as (Gamma''',(GH, Split'));
 destruct Split' as (GT, (Ha, Hb));
-apply t_get_here_LF with (G:=GH++GT & (w'0, Gamma'0++Gamma''))
+apply t_get_here_Hyb with (G:=GH++GT & (w'0, Gamma'0++Gamma''))
   (Gamma:=Gamma).
-apply ok_Bg_ppermut with (G':=(G' & (w0, Gamma0))) in Ok_Bg;
+apply ok_Bg_Hyb_ppermut with (G':=(G' & (w0, Gamma0))) in Ok_Bg;
 [ | rewrite <- H; auto]; rewrite H0 in Ok_Bg; subst G0.
-apply ok_Bg_ppermut with
+apply ok_Bg_Hyb_ppermut with
   (G:= (GH & (w, Gamma''') ++ GT) & (w'0, Gamma'0 ++ Gamma'') & (w0, Gamma0));
-[ rew_app | ]; auto; try PPermut_simpl; eapply ok_Bg_split6; eauto.
+[ rew_app | ]; auto; try PPermut_Hyb_simpl; eapply ok_Bg_Hyb_split6; eauto.
 eapply IHHT with (w1:=w) (Gamma1:=Gamma) (G0:=GH++GT & (w0,Gamma0))
   (Gamma':=Gamma'0) (Gamma'':=Gamma''); auto.
-PPermut_simpl. apply PPermut_last_rev_simpl with (a:=(w, Gamma));
-rewrite <- H3; subst; PPermut_simpl.
-PPermut_simpl.
-rewrite H1; subst; PPermut_simpl.
+PPermut_Hyb_simpl. apply PPermut_Hyb_last_rev_simpl with (a:=(w, Gamma));
+rewrite <- H3; subst; PPermut_Hyb_simpl.
+PPermut_Hyb_simpl.
+rewrite H1; subst; PPermut_Hyb_simpl.
 
 (* letdia *)
 case_if.
 inversion H1; subst; rewrite H0 in Ok_Bg;
-apply ok_Bg_first_last_neq in Ok_Bg; elim Ok_Bg; auto.
-apply t_letdia_LF with (L_w:=L_w \u \{w'}) (L_t:=L_t) (A:=A);
+apply ok_Bg_Hyb_first_last_neq in Ok_Bg; elim Ok_Bg; auto.
+apply t_letdia_Hyb with (L_w:=L_w \u \{w'}) (L_t:=L_t) (A:=A);
 [ rewrite H0 in Ok_Bg |
   eapply IHHT with (w:=w0) (Gamma:=Gamma0) | ]; eauto.
-eapply ok_Bg_split2; eauto.
+eapply ok_Bg_Hyb_split2; eauto.
 intros; rewrite notin_union in H3; destruct H3;
 rewrite notin_singleton in H4;
-unfold open_t in *; unfold open_w in *;
-rewrite <- subst_w_comm; auto;
-rewrite subst_order_irrelevant_free;
+unfold open_t_Hyb in *; unfold open_w_Hyb in *;
+rewrite <- subst_w_Hyb_comm; auto;
+rewrite subst_Hyb_order_irrelevant_free;
 [ eapply H with (w:=w0) (Gamma:=Gamma0) (w':=w'0) | simpl]; eauto;
-rewrite H0; PPermut_simpl.
+rewrite H0; PPermut_Hyb_simpl.
 
 case_if.
-apply t_letdia_LF with (L_w:=L_w \u \{w0}) (L_t:=L_t) (A:=A);
+apply t_letdia_Hyb with (L_w:=L_w \u \{w0}) (L_t:=L_t) (A:=A);
 [ rewrite H0 in Ok_Bg | eapply IHHT with (w:=w0) (Gamma:=Gamma0) | ]; eauto.
-eapply ok_Bg_split2; eauto.
+eapply ok_Bg_Hyb_split2; eauto.
 intros; rewrite notin_union in H2; destruct H2;
 rewrite notin_singleton in H3;
-unfold open_t in *; unfold open_w in *;
-rewrite <- subst_w_comm; auto;
-rewrite subst_order_irrelevant_free;
+unfold open_t_Hyb in *; unfold open_w_Hyb in *;
+rewrite <- subst_w_Hyb_comm; auto;
+rewrite subst_Hyb_order_irrelevant_free;
 [ eapply H with (w:=w0) (Gamma:=Gamma0) (w':=w'0) | simpl]; eauto;
-rewrite H0; PPermut_simpl.
+rewrite H0; PPermut_Hyb_simpl.
 
 case_if.
 inversion H2; subst; rewrite H0 in Ok_Bg;
-apply ok_Bg_first_last_neq in Ok_Bg; elim Ok_Bg; auto.
-apply t_letdia_LF with (L_w:=L_w \u \{w''}) (L_t:=L_t) (A:=A);
+apply ok_Bg_Hyb_first_last_neq in Ok_Bg; elim Ok_Bg; auto.
+apply t_letdia_Hyb with (L_w:=L_w \u \{w''}) (L_t:=L_t) (A:=A);
 [ rewrite H0 in Ok_Bg; rewrite H1 |
   eapply IHHT with (w:=w0) (Gamma:=Gamma0) | ]; eauto.
-eapply ok_Bg_split3; eauto.
+eapply ok_Bg_Hyb_split3; eauto.
 intros; rewrite notin_union in H4; destruct H4;
 rewrite notin_singleton in H5;
-unfold open_t in *; unfold open_w in *;
-rewrite <- subst_w_comm; auto;
-rewrite subst_order_irrelevant_free; simpl; auto;
+unfold open_t_Hyb in *; unfold open_w_Hyb in *;
+rewrite <- subst_w_Hyb_comm; auto;
+rewrite subst_Hyb_order_irrelevant_free; simpl; auto;
 eapply H with (w:=w0) (Gamma:=Gamma0) (G0:=G0 & ((w'0, (v', A)::nil)))
   (Gamma':=Gamma') (Gamma'':=Gamma''); auto;
 [ rewrite H0 |rewrite H1 ]; rew_app; auto;
-PPermut_simpl.
+PPermut_Hyb_simpl.
 
 (* letdia_get *)
 case_if.
 inversion H3; subst;
 assert (G ~=~ G' /\ Gamma *=* Gamma') by
-  (apply ok_Bg_impl_ppermut with (w:=w'); [ | transitivity G0]; eauto);
+  (apply ok_Bg_Hyb_impl_ppermut with (w:=w'); [ | transitivity G0]; eauto);
 destruct H4;
-eapply t_letdia_LF with (L_w := L_w \u \{w'}).
-rewrite <- H4; apply ok_Bg_permut with (Ctx:=(Gamma0 ++ Gamma)); auto;
-eapply ok_Bg_split1; eauto.
-apply ContextPermutImpl with (Gamma := Gamma0++Gamma); [permut_simpl|]; auto;
-eapply IHHT; auto.
+eapply t_letdia_Hyb with (L_w := L_w \u \{w'}).
+rewrite <- H4; apply ok_Bg_Hyb_permut with (Ctx:=(Gamma0 ++ Gamma)); auto;
+eapply ok_Bg_Hyb_split1; eauto.
+apply ContextPermutImpl_Hyb with (Gamma := Gamma0++Gamma); [permut_simpl|];
+auto; eapply IHHT; auto.
 intros; rewrite notin_union in H7; destruct H7;
 rewrite notin_singleton in H8;
-unfold open_t in *; unfold open_w in *;
-rewrite <- subst_w_comm; auto;
-rewrite subst_order_irrelevant_free; simpl; auto;
+unfold open_t_Hyb in *; unfold open_w_Hyb in *;
+rewrite <- subst_w_Hyb_comm; auto;
+rewrite subst_Hyb_order_irrelevant_free; simpl; auto;
 eapply H with (v':=v') (w'0:=w'0) (w:=w0); auto;
 [ | rew_app]; eauto.
 destruct (eq_var_dec w w0).
-subst; apply ok_Bg_first_last_neq in Ok_Bg; elim Ok_Bg; auto.
+subst; apply ok_Bg_Hyb_first_last_neq in Ok_Bg; elim Ok_Bg; auto.
 assert (G' & (w', Gamma') ~=~ G & (w, Gamma)) by
   (symmetry; transitivity G0; auto);
 assert (exists Gamma'', exists GH, exists GT,
   Gamma'' *=* Gamma /\ G' = GH & (w, Gamma'') ++ GT) by
-  (eapply PPermut_split_neq; eauto; right; intro; subst; eauto);
+  (eapply PPermut_Hyb_split_neq; eauto; right; intro; subst; eauto);
 destruct H5 as (Gamma'', (GH, (GT, (Ha, Hb))));
 assert (G & (w, Gamma) ~=~
        (GH ++ GT ++ (w', Gamma') :: nil) &  (w, Gamma));
 [subst; symmetry | rew_app]; auto.
-rewrite <- H4; PPermut_simpl.
-apply t_letdia_get_LF with (L_w:=L_w \u \{w'}) (L_t:=L_t) (A:=A)
+rewrite <- H4; PPermut_Hyb_simpl.
+apply t_letdia_get_Hyb with (L_w:=L_w \u \{w'}) (L_t:=L_t) (A:=A)
   (G:=GH++GT) (Gamma:=Gamma);
 assert ((w, Gamma) :: G & (w0, Gamma0) ~=~
   (GH ++ GT & (w', Gamma')) & (w, Gamma) & (w0, Gamma0)) by
-  (PPermut_simpl; apply PPermut_last_rev_simpl with (a:=(w,Gamma)); auto).
+  (PPermut_Hyb_simpl; apply PPermut_Hyb_last_rev_simpl with (a:=(w,Gamma)); auto).
 rewrite H6 in Ok_Bg.
-apply ok_Bg_ppermut with (G:=(GH ++ GT & (w, Gamma)) & (w0, Gamma0 ++ Gamma')).
-PPermut_simpl.
-rew_app in *; eauto. eapply ok_Bg_split8; eauto.
+apply ok_Bg_Hyb_ppermut with (G:=(GH ++ GT & (w, Gamma)) &
+  (w0, Gamma0 ++ Gamma')).
+PPermut_Hyb_simpl.
+rew_app in *; eauto. eapply ok_Bg_Hyb_split8; eauto.
 eapply IHHT with (w1:=w) (G0:=GH++GT) (w':=w0)
   (Gamma':=Gamma0) (Gamma'':=Gamma');
 auto.
-PPermut_simpl; apply PPermut_last_rev_simpl with (a:=(w, Gamma));
-rewrite H5; PPermut_simpl.
+PPermut_Hyb_simpl; apply PPermut_Hyb_last_rev_simpl with (a:=(w, Gamma));
+rewrite H5; PPermut_Hyb_simpl.
 intros; rewrite notin_union in H8; destruct H8;
 rewrite notin_singleton in H9;
-unfold open_t in *; unfold open_w in *;
-rewrite <- subst_w_comm; auto;
-rewrite subst_order_irrelevant_free; simpl; auto;
+unfold open_t_Hyb in *; unfold open_w_Hyb in *;
+rewrite <- subst_w_Hyb_comm; auto;
+rewrite subst_Hyb_order_irrelevant_free; simpl; auto;
 eapply H with (w1:=w0) (Gamma1:=Gamma0); auto.
-rewrite H5; PPermut_simpl.
-subst; PPermut_simpl.
+rewrite H5; PPermut_Hyb_simpl.
+subst; PPermut_Hyb_simpl.
 
 case_if.
 inversion H3; subst;
-apply ok_Bg_first_last_neq in Ok_Bg; elim Ok_Bg; auto.
+apply ok_Bg_Hyb_first_last_neq in Ok_Bg; elim Ok_Bg; auto.
 destruct (eq_var_dec w w').
 subst; assert (G ~=~ G' /\ Gamma *=* Gamma').
-  apply ok_Bg_impl_ppermut with (w:=w'); auto. eauto with ok_bg_rew.
+  apply ok_Bg_Hyb_impl_ppermut with (w:=w'); auto. eauto with ok_bg_hyb_rew.
   transitivity G0; auto.
 destruct H4;
-apply t_letdia_LF with (L_w:=L_w \u \{w0}) (L_t:=L_t) (A:=A).
-rewrite <- H4; apply ok_Bg_permut with (Ctx := Gamma ++ Gamma0); auto;
-eapply ok_Bg_split2; eauto.
-apply ContextPermutImpl with (Gamma:=Gamma++Gamma0); auto;
+apply t_letdia_Hyb with (L_w:=L_w \u \{w0}) (L_t:=L_t) (A:=A).
+rewrite <- H4; apply ok_Bg_Hyb_permut with (Ctx := Gamma ++ Gamma0); auto;
+eapply ok_Bg_Hyb_split2; eauto.
+apply ContextPermutImpl_Hyb with (Gamma:=Gamma++Gamma0); auto;
 eapply IHHT with (Gamma1:=Gamma); eauto.
 intros; rewrite <- H4;
-apply ContextPermutImpl with (Gamma:=Gamma++Gamma0); auto;
-unfold open_t in *; unfold open_w in *;
-rewrite <- subst_w_comm; auto;
-rewrite subst_order_irrelevant_free; simpl; auto.
+apply ContextPermutImpl_Hyb with (Gamma:=Gamma++Gamma0); auto;
+unfold open_t_Hyb in *; unfold open_w_Hyb in *;
+rewrite <- subst_w_Hyb_comm; auto;
+rewrite subst_Hyb_order_irrelevant_free; simpl; auto.
 eapply H with (w'0 := w'0); eauto.
 assert (G' & (w', Gamma') ~=~ G & (w, Gamma)) by
   (symmetry; transitivity G0; auto);
 assert (exists Gamma'', exists GH, exists GT,
   Gamma'' *=* Gamma /\ G' = GH & (w, Gamma'') ++ GT) by
-  (eapply PPermut_split_neq; eauto).
+  (eapply PPermut_Hyb_split_neq; eauto).
 destruct H5 as (Gamma'', (GH, (GT, (Ha, Hb)))).
-apply t_letdia_get_LF with (L_w:=L_w \u \{w0})
+apply t_letdia_get_Hyb with (L_w:=L_w \u \{w0})
   (L_t:=L_t) (A:=A) (G:=GH++GT) (Gamma:=Gamma).
 subst; assert ((w, Gamma) :: G & (w0, Gamma0) ~=~
   (GH & (w, Gamma'') ++ GT) & (w', Gamma') & (w0, Gamma0)) by
 (rewrite H4; auto).
 rewrite H5 in Ok_Bg.
-apply ok_Bg_ppermut with (G:= GH & (w, Gamma'') ++ GT & (w', Gamma' ++ Gamma0));
-rew_app in *; [ PPermut_simpl | ];
-apply ok_Bg_ppermut with
+apply ok_Bg_Hyb_ppermut with (G:= GH & (w, Gamma'') ++ GT &
+  (w', Gamma' ++ Gamma0));
+rew_app in *; [ PPermut_Hyb_simpl | ];
+apply ok_Bg_Hyb_ppermut with
   (G:=(GH ++ (w, Gamma'') :: GT) & (w', Gamma' ++ Gamma0));
-[ | apply ok_Bg_split4 with (w:=w0)]; rew_app; auto;
-apply ok_Bg_ppermut with (G:=GH ++ (w, Gamma'') :: GT ++ (w', Gamma') ::
+[ | apply ok_Bg_Hyb_split4 with (w:=w0)]; rew_app; auto;
+apply ok_Bg_Hyb_ppermut with (G:=GH ++ (w, Gamma'') :: GT ++ (w', Gamma') ::
   (w0, Gamma0) :: nil); eauto.
 eapply IHHT; auto.
-PPermut_simpl; apply PPermut_last_rev_simpl with (a:=(w, Gamma));
-rewrite <- H4; subst; PPermut_simpl.
+PPermut_Hyb_simpl; apply PPermut_Hyb_last_rev_simpl with (a:=(w, Gamma));
+rewrite <- H4; subst; PPermut_Hyb_simpl.
 intros. rewrite notin_union in H6; destruct H6;
-rewrite notin_singleton in H7; unfold open_t in *; unfold open_w in *;
-rewrite <- subst_w_comm; auto;
-rewrite subst_order_irrelevant_free; simpl; auto;
-eapply H with (w1:=w0) (Gamma1:=Gamma0); auto; PPermut_simpl.
-apply PPermut_last_rev_simpl with (a:=(w,Gamma));
-rewrite <- H4; subst; PPermut_simpl.
-subst; PPermut_simpl.
+rewrite notin_singleton in H7; unfold open_t_Hyb in *; unfold open_w_Hyb in *;
+rewrite <- subst_w_Hyb_comm; auto;
+rewrite subst_Hyb_order_irrelevant_free; simpl; auto;
+eapply H with (w1:=w0) (Gamma1:=Gamma0); auto; PPermut_Hyb_simpl.
+apply PPermut_Hyb_last_rev_simpl with (a:=(w,Gamma));
+rewrite <- H4; subst; PPermut_Hyb_simpl.
+subst; PPermut_Hyb_simpl.
 
 case_if.
 inversion H4; subst;
 assert (G ~=~ G1 & (w', Gamma') /\ Gamma *=* Gamma'') by
- (apply ok_Bg_impl_ppermut with (w:=w'');
+ (apply ok_Bg_Hyb_impl_ppermut with (w:=w'');
   [ | transitivity G0]; eauto);
 destruct H5;
-eapply t_letdia_get_LF with (G:=G1) (Gamma:=Gamma'++Gamma) (L_w:=L_w \u \{w''}).
+eapply t_letdia_get_Hyb with (G:=G1) (Gamma:=Gamma'++Gamma)
+  (L_w:=L_w \u \{w''}).
 rewrite H5 in Ok_Bg; eauto.
 clear H HT2 IHHT.
-eapply ok_Bg_split2; eauto; apply ok_Bg_ppermut with
+eapply ok_Bg_Hyb_split2; eauto; apply ok_Bg_Hyb_ppermut with
   (G:=(w'', Gamma) :: G1 & (w', Gamma') & (w0, Gamma0));
-eauto; PPermut_simpl.
+eauto; PPermut_Hyb_simpl.
 eapply IHHT with (Gamma':=Gamma'); auto;
-try PPermut_simpl.
-intros; unfold open_t in *; unfold open_w in *;
-rewrite <- subst_w_comm; auto;
-rewrite subst_order_irrelevant_free; simpl; auto;
+try PPermut_Hyb_simpl.
+intros; unfold open_t_Hyb in *; unfold open_w_Hyb in *;
+rewrite <- subst_w_Hyb_comm; auto;
+rewrite subst_Hyb_order_irrelevant_free; simpl; auto;
 eapply H with (w:=w0) (G0:=(w'0, (v',A)::nil)::G1)
   (Gamma':=Gamma') (Gamma'':=Gamma); auto;
 [ eauto | rew_app]; constructor; [ | symmetry]; auto;
 rewrite H5; rew_app; auto.
-rewrite H2; PPermut_simpl.
+rewrite H2; PPermut_Hyb_simpl.
 destruct (eq_var_dec w w').
 subst.
 assert (G ~=~ G1 & (w'', Gamma'') /\ Gamma *=* Gamma').
-  apply ok_Bg_impl_ppermut with (w:=w'); [ | transitivity G0]; eauto;
-  rewrite H1; PPermut_simpl.
+  apply ok_Bg_Hyb_impl_ppermut with (w:=w'); [ | transitivity G0]; eauto;
+  rewrite H1; PPermut_Hyb_simpl.
 destruct H5;
-eapply t_letdia_get_LF with (G:=G1) (Gamma:=Gamma++Gamma'')
+eapply t_letdia_get_Hyb with (G:=G1) (Gamma:=Gamma++Gamma'')
   (L_w:=L_w \u \{w''}) (L_t := L_t).
 clear H HT2 IHHT.
-rewrite H5 in Ok_Bg; eapply ok_Bg_split9; eauto.
-eapply IHHT with (w:=w'); auto; PPermut_simpl.
-intros; unfold open_t in *; unfold open_w in *;
-rewrite <- subst_w_comm; auto;
-rewrite subst_order_irrelevant_free; simpl; auto;
+rewrite H5 in Ok_Bg; eapply ok_Bg_Hyb_split9; eauto.
+eapply IHHT with (w:=w'); auto; PPermut_Hyb_simpl.
+intros; unfold open_t_Hyb in *; unfold open_w_Hyb in *;
+rewrite <- subst_w_Hyb_comm; auto;
+rewrite subst_Hyb_order_irrelevant_free; simpl; auto;
 eapply H with (w:=w0) (G0:=(w'0, (v',A)::nil)::G1)
   (Gamma':=Gamma) (Gamma'':=Gamma''); auto;
 rew_app; constructor; auto;
 symmetry; transitivity ((G1 ++ (w'', Gamma'')::nil) & (w', Gamma)); auto;
 rew_app; auto.
-rewrite H2; PPermut_simpl.
+rewrite H2; PPermut_Hyb_simpl.
 assert (G & (w, Gamma) ~=~ G1 & (w', Gamma') & (w'', Gamma'')) by
   (symmetry; transitivity G0; symmetry; auto);
 assert (exists Gamma0, exists GH, exists GT,
   Gamma0 *=* Gamma /\ G1 & (w'', Gamma'') = GH & (w, Gamma0) ++ GT) by
-  (apply PPermut_split_neq with (w:=w') (G':=G) (Gamma:=Gamma');
+  (apply PPermut_Hyb_split_neq with (w:=w') (G':=G) (Gamma:=Gamma');
    try symmetry; auto; transitivity (G1 & (w', Gamma') & (w'', Gamma'')); auto;
-  PPermut_simpl).
+  PPermut_Hyb_simpl).
 assert (exists Gamma0, exists GH, exists GT,
   Gamma0 *=* Gamma /\ G1 = GH & (w, Gamma0) ++ GT) by
   (destruct H6 as (Gamma5, (GH, (GT, (H6a, H6b)))); subst;
-   apply PPermut_split_neq with (w:=w'') (G':=GH++GT) (Gamma:=Gamma''); auto;
-   [rewrite H6b; rew_app; auto | right; intro; subst; elim H4; reflexivity];
-  PPermut_simpl).
+   apply PPermut_Hyb_split_neq with (w:=w'') (G':=GH++GT) (Gamma:=Gamma'');
+   auto; [rewrite H6b; rew_app; auto | right; intro; subst; elim H4;
+     reflexivity];
+  PPermut_Hyb_simpl).
 destruct H7 as (Gamma'1, (GH, (GT, (H7a, H7b)))); subst.
-apply t_letdia_get_LF with (L_w:=L_w \u \{w''})
+apply t_letdia_get_Hyb with (L_w:=L_w \u \{w''})
   (L_t:=L_t) (A:=A) (G:=GH++GT & (w', Gamma'++Gamma'')) (Gamma:=Gamma).
 assert ((w, Gamma) :: G & (w0, Gamma0) ~=~ G0  & (w0, Gamma0)) by
   (rewrite <- H0; auto);
 rewrite H7 in Ok_Bg; rewrite H1 in Ok_Bg.
-apply ok_Bg_ppermut with (G:= (GH & (w, Gamma'1) ++ GT) &
+apply ok_Bg_Hyb_ppermut with (G:= (GH & (w, Gamma'1) ++ GT) &
   (w', Gamma' ++ Gamma'') & (w0, Gamma0));
-rew_app in *; eauto; try PPermut_simpl.
-clear IHHT H HT2. eapply ok_Bg_split10; eauto.
+rew_app in *; eauto; try PPermut_Hyb_simpl.
+clear IHHT H HT2. eapply ok_Bg_Hyb_split10; eauto.
 eapply IHHT with (w1:=w) (G0:=GH++GT & (w0, Gamma0))
   (Gamma':=Gamma') (Gamma'':=Gamma''); rew_app; auto;
 rew_app in *; transitivity ((GH ++ GT ++ (w', Gamma') ::
   (w'', Gamma'') :: nil) & (w0, Gamma0));
-[ PPermut_simpl | rew_app]; auto;
-apply PPermut_last_rev_simpl with (a:=(w, Gamma));
+[ PPermut_Hyb_simpl | rew_app]; auto;
+apply PPermut_Hyb_last_rev_simpl with (a:=(w, Gamma));
 rewrite H5; symmetry; transitivity (GH ++ GT ++ (w, Gamma) :: (w', Gamma') ::
-  (w'', Gamma'') :: nil); [rew_app |  apply PPermut_app_head; symmetry]; auto;
-try PPermut_simpl.
-intros; unfold open_t in *; unfold open_w in *;
-rewrite <- subst_w_comm; auto;
-rewrite subst_order_irrelevant_free; simpl; auto;
+  (w'', Gamma'') :: nil); [rew_app |  apply PPermut_Hyb_app_head; symmetry];
+auto; try PPermut_Hyb_simpl.
+intros; unfold open_t_Hyb in *; unfold open_w_Hyb in *;
+rewrite <- subst_w_Hyb_comm; auto;
+rewrite subst_Hyb_order_irrelevant_free; simpl; auto;
 eapply H with (G0:=(w'0, (v', A) :: nil) :: (GH ++ GT) & (w, Gamma))
-  (Gamma':=Gamma') (Gamma'':=Gamma''); auto; PPermut_simpl.
-apply PPermut_last_rev_simpl with (a:=(w, Gamma)); rewrite H5;
-PPermut_simpl.
-rewrite H2; PPermut_simpl.
+  (Gamma':=Gamma') (Gamma'':=Gamma''); auto; PPermut_Hyb_simpl.
+apply PPermut_Hyb_last_rev_simpl with (a:=(w, Gamma)); rewrite H5;
+PPermut_Hyb_simpl.
+rewrite H2; PPermut_Hyb_simpl.
 Existential 1 := G.
 Existential 1 := Gamma'.
 Existential 1 := w'.
@@ -1758,29 +1789,31 @@ Existential 1 := Gamma'.
 Existential 1 := w'.
 Qed.
 
-Lemma rename_w_preserv_types_new:
+Lemma rename_w_Hyb_preserv_types_new:
 forall G w Gamma A M G' w' Gamma'
   (HT: G |= (w, Gamma) |- M ::: A)
-  (GG': PPermut G (G' & (w', Gamma'))),
+  (GG': PPermut_Hyb G (G' & (w', Gamma'))),
   G' |= (w, Gamma ++ Gamma') |- {{ fwo w // fwo w' }} M ::: A.
-intros; apply rename_w_preserv_types with (G := G) (w := w) (w':= w'); eauto.
+intros; apply rename_w_Hyb_preserv_types with (G := G) (w := w) (w':= w');
+eauto.
 Qed.
 
-Lemma rename_w_preserv_types_old:
+Lemma rename_w_Hyb_preserv_types_old:
 forall G w Gamma A M G' w' Gamma'
   (HT: G |= (w, Gamma) |- M ::: A)
-  (GG': PPermut G (G' & (w', Gamma'))),
+  (GG': PPermut_Hyb G (G' & (w', Gamma'))),
   G' |= (w', Gamma' ++ Gamma) |- {{ fwo w' // fwo w }} M ::: A.
-intros; apply rename_w_preserv_types with (G := G) (w := w) (w':= w'); eauto.
+intros; apply rename_w_Hyb_preserv_types with (G := G) (w := w) (w':= w');
+eauto.
 Qed.
 
-Lemma rename_w_preserv_types_outer:
+Lemma rename_w_Hyb_preserv_types_outer:
 forall G G0 w Gamma A M G' w' Gamma' w'' Gamma''
   (HT: G |= (w, Gamma) |- M ::: A)
-  (GG: PPermut G (G0 & (w', Gamma') & (w'', Gamma'')))
-  (GG': PPermut G' (G0 & (w', Gamma' ++ Gamma''))),
+  (GG: PPermut_Hyb G (G0 & (w', Gamma') & (w'', Gamma'')))
+  (GG': PPermut_Hyb G' (G0 & (w', Gamma' ++ Gamma''))),
   G' |= (w, Gamma) |- {{ fwo w' // fwo w'' }} M ::: A.
-intros; eapply rename_w_preserv_types; eauto.
+intros; eapply rename_w_Hyb_preserv_types; eauto.
 Qed.
 
 (*
@@ -1792,19 +1825,19 @@ Proof sketch: double induction: on term and on typing
   * the only exception is here M, where we know it is a value when
   M was also a value
 *)
-Lemma Progress:
+Lemma Progress_Hyb:
 forall G w M A
-  (H_lc_w: lc_w_LF M)
-  (H_lc_t: lc_t_LF M)
-  (HT: emptyEquiv G |= (w, nil) |- M ::: A),
-  value_LF M \/ exists N, (M, fwo w) |-> (N, fwo w).
+  (H_lc_w: lc_w_Hyb M)
+  (H_lc_t: lc_t_Hyb M)
+  (HT: emptyEquiv_Hyb G |= (w, nil) |- M ::: A),
+  value_Hyb M \/ exists N, (M, fwo w) |-> (N, fwo w).
 intros;
 remember (w, (@nil ty)) as Ctx;
 generalize dependent Ctx;
 generalize dependent A;
 generalize dependent w;
 generalize dependent G;
-induction M; intros; eauto using value_LF;
+induction M; intros; eauto using value_Hyb;
 inversion HeqCtx; subst.
 (* hyp *)
 inversion HT; subst;
@@ -1832,7 +1865,7 @@ inversion H1; inversion H2; subst; auto;
 erewrite closed_var_subst_ctx; eauto; constructor.
 (* unbox_fetch *)
 assert (Gamma = nil) by
-  ( apply emptyEquiv_permut_empty with
+  ( apply emptyEquiv_Hyb_permut_empty with
     (G:= (G0 & (w0, Gamma))) (G':=G) (w:=w0); auto;
     apply Mem_last); subst;
 destruct IHM with (A := [*]A)
@@ -1840,9 +1873,9 @@ destruct IHM with (A := [*]A)
                   (G := G0 & (w, nil))
                   (w := w0);
 eauto.
-assert (emptyEquiv (G0 & (w, nil)) = G0 & (w, nil)) by
-  ( repeat rewrite emptyEquiv_rewrite; simpl;
-   apply emptyEquiv_permut_split_last in H6; rewrite H6; reflexivity);
+assert (emptyEquiv_Hyb (G0 & (w, nil)) = G0 & (w, nil)) by
+  ( repeat rewrite emptyEquiv_Hyb_rewrite; simpl;
+   apply emptyEquiv_Hyb_permut_split_last in H6; rewrite H6; reflexivity);
 rewrite H0; auto.
 inversion H0; subst; inversion HT0; subst;
 eexists; constructor; eauto; inversion H2; auto; subst.
@@ -1856,10 +1889,10 @@ inversion H_lc_t; subst.
 edestruct IHM; eauto;
 [ left; econstructor|
   right; destruct H0; eexists];
-eauto using step_LF.
+eauto using step_Hyb.
 (* get_here *)
 assert (Gamma = nil) by
-  ( apply emptyEquiv_permut_empty with
+  ( apply emptyEquiv_Hyb_permut_empty with
     (G:= (G0 & (w0, Gamma))) (G':=G) (w:=w0); auto;
     apply Mem_last); subst;
 destruct IHM with (A := A0)
@@ -1867,14 +1900,14 @@ destruct IHM with (A := A0)
                   (G := G0 & (w, nil))
                   (w := w0);
 eauto.
-assert (emptyEquiv (G0 & (w, nil)) = G0 & (w, nil)) by
-  ( repeat rewrite emptyEquiv_rewrite; simpl;
-   apply emptyEquiv_permut_split_last in H6; rewrite H6; reflexivity);
+assert (emptyEquiv_Hyb (G0 & (w, nil)) = G0 & (w, nil)) by
+  ( repeat rewrite emptyEquiv_Hyb_rewrite; simpl;
+   apply emptyEquiv_Hyb_permut_split_last in H6; rewrite H6; reflexivity);
 rewrite H0; auto.
 left; inversion H0; subst; inversion HT0; subst;
-econstructor; eauto using step_LF.
+econstructor; eauto using step_Hyb.
 right; destruct H0; eexists;
-econstructor; eauto using step_LF.
+econstructor; eauto using step_Hyb.
 (* letdia & letdia_get *)
 right; inversion HT; subst;
 inversion H_lc_w; subst;
@@ -1890,15 +1923,16 @@ inversion H5; subst; auto.
 inversion H7; subst; auto.
 (* letdia_get *)
 assert (Gamma = nil) by
-  ( apply emptyEquiv_permut_empty with (G:= (G0 & (w0, Gamma))) (G':=G) (w:=w0);
+  ( apply emptyEquiv_Hyb_permut_empty
+    with (G:= (G0 & (w0, Gamma))) (G':=G) (w:=w0);
     auto; apply Mem_last); subst;
 edestruct IHM1 with (G := G0 & (w, nil))
                     (w := w0)
                     (Ctx := (w0, (@nil ty)))
                     (A := <*>A0); eauto;
-assert ( emptyEquiv (G0 & (w, nil)) = G0 & (w, nil)) by
-   ( repeat rewrite emptyEquiv_rewrite; simpl;
-     apply emptyEquiv_permut_split_last in H6; rewrite H6; reflexivity).
+assert ( emptyEquiv_Hyb (G0 & (w, nil)) = G0 & (w, nil)) by
+   ( repeat rewrite emptyEquiv_Hyb_rewrite; simpl;
+     apply emptyEquiv_Hyb_permut_split_last in H6; rewrite H6; reflexivity).
 rewrite H0; auto.
 inversion H0; subst; inversion HT1; subst;
 eexists; constructor; eauto;
@@ -1920,14 +1954,14 @@ Qed.
    * for letdia here we combine the two above + use the knowledge
    that term and world substitution can be done in any order
 *)
-Lemma Preservation:
+Lemma Preservation_Hyb:
 forall G M N A w
-  (HT: emptyEquiv G |= (w, nil) |- M ::: A)
+  (HT: emptyEquiv_Hyb G |= (w, nil) |- M ::: A)
   (HS: (M, fwo w) |-> (N, fwo w)),
-  emptyEquiv G |= (w, nil) |- N ::: A.
+  emptyEquiv_Hyb G |= (w, nil) |- N ::: A.
 intros;
 remember (w, (@nil (var * ty))) as Ctx;
-remember (emptyEquiv G) as G';
+remember (emptyEquiv_Hyb G) as G';
 generalize dependent w;
 generalize dependent N;
 generalize dependent G;
@@ -1937,221 +1971,225 @@ try (inversion HeqCtx; subst);
 try (econstructor; eauto).
 (* appl_lam *)
 inversion HT1; subst;
-unfold open_t in *;
-assert (exists v, v \notin L \u free_vars_LF M0) as HF by apply Fresh;
+unfold open_t_Hyb in *;
+assert (exists v, v \notin L \u free_vars_Hyb M0) as HF by apply Fresh;
 destruct HF as (v_fresh).
-rewrite subst_t_neutral_free with (v:=v_fresh);
-[ eapply subst_t_preserv_types_inner; eauto |
+rewrite subst_t_Hyb_neutral_free with (v:=v_fresh);
+[ eapply subst_t_Hyb_preserv_types_inner; eauto |
   rewrite notin_union in H; destruct H]; auto.
-rewrite <- double_emptyEquiv; auto.
+rewrite <- double_emptyEquiv_Hyb; auto.
 (* unbox_box *)
 inversion HT; subst;
-assert (exists v, v \notin L \u (free_worlds_LF M0)) as HF by apply Fresh;
+assert (exists v, v \notin L \u (free_worlds_Hyb M0)) as HF by apply Fresh;
 destruct HF as (w_fresh);
-unfold open_w in *;
+unfold open_w_Hyb in *;
 replace ({{fwo w0 // bwo 0}}M0)
   with ({{fwo w0 // fwo w_fresh}} {{fwo w_fresh // bwo 0}}M0)
-  by (rewrite subst_w_neutral_free; auto);
+  by (rewrite subst_w_Hyb_neutral_free; auto);
 replace (@nil (var * ty)) with (nil ++ (@nil (var * ty))); eauto;
-apply rename_w_preserv_types_old with (G := emptyEquiv G0 & (w0, nil));
+apply rename_w_Hyb_preserv_types_old with (G := emptyEquiv_Hyb G0 & (w0, nil));
 auto.
 (* unbox_fetch_box *)
 inversion HT; subst;
-assert (exists v, v \notin L \u (free_worlds_LF M0)) as HF by apply Fresh;
+assert (exists v, v \notin L \u (free_worlds_Hyb M0)) as HF by apply Fresh;
 destruct HF as (w_fresh);
-unfold open_w in *;
+unfold open_w_Hyb in *;
 replace ({{fwo w0 // bwo 0}}M0)
   with ({{fwo w0 // fwo w_fresh}} {{fwo w_fresh // bwo 0}}M0)
-  by (rewrite subst_w_neutral_free; auto);
+  by (rewrite subst_w_Hyb_neutral_free; auto);
 replace (@nil (var * ty)) with (nil ++ (@nil (var * ty))); eauto;
-apply rename_w_preserv_types_old with (G := G & (w0, nil) & (w, Gamma));
-auto; PPermut_simpl.
+apply rename_w_Hyb_preserv_types_old with (G := G & (w0, nil) & (w, Gamma));
+auto; PPermut_Hyb_simpl.
 (* unbox_fetch *)
 assert (Gamma = nil) by
-  ( apply emptyEquiv_permut_empty with (G:= (G & (w, Gamma))) (G':=G0) (w:=w);
+  ( apply emptyEquiv_Hyb_permut_empty with (G:= (G & (w, Gamma))) (G':=G0)
+    (w:=w);
     auto; apply Mem_last); subst;
 eapply IHHT with (G0:=G & (w0, nil)); eauto;
-repeat rewrite emptyEquiv_rewrite; simpl;
-apply emptyEquiv_permut_split_last in H; rewrite H; reflexivity.
+repeat rewrite emptyEquiv_Hyb_rewrite; simpl;
+apply emptyEquiv_Hyb_permut_split_last in H; rewrite H; reflexivity.
 (* get_here *)
 assert (Gamma = nil) by
-  ( apply emptyEquiv_permut_empty with (G:= (G & (w, Gamma))) (G':=G0) (w:=w);
+  ( apply emptyEquiv_Hyb_permut_empty with (G:= (G & (w, Gamma))) (G':=G0)
+    (w:=w);
     auto; apply Mem_last); subst;
 eapply IHHT with (G0:=G & (w0, nil)); eauto;
-repeat rewrite emptyEquiv_rewrite; simpl;
-apply emptyEquiv_permut_split_last in H; rewrite H; reflexivity.
+repeat rewrite emptyEquiv_Hyb_rewrite; simpl;
+apply emptyEquiv_Hyb_permut_split_last in H; rewrite H; reflexivity.
 (* letdia + (here | get_here ) *)
-assert (exists w1, w1 \notin L_w \u free_worlds_LF N) as HF by apply Fresh;
-assert (exists v1, v1 \notin L_t \u free_vars_LF N) as HF2 by apply Fresh;
+assert (exists w1, w1 \notin L_w \u free_worlds_Hyb N) as HF by apply Fresh;
+assert (exists v1, v1 \notin L_t \u free_vars_Hyb N) as HF2 by apply Fresh;
 destruct HF as (w_fresh); destruct HF2 as (v_fresh);
 inversion HT; subst.
 (* letdia #1 *)
 rewrite notin_union in *; destruct H0; destruct H1;
-unfold open_t in *; unfold open_w in *;
-rewrite subst_t_neutral_free with (v:=v_fresh);
-[ rewrite subst_order_irrelevant_bound |
-  apply subst_world_preserv_free_vars]; auto;
-[ rewrite <- subst_w_neutral_free with (w0:=w_fresh) |
+unfold open_t_Hyb in *; unfold open_w_Hyb in *;
+rewrite subst_t_Hyb_neutral_free with (v:=v_fresh);
+[ rewrite subst_Hyb_order_irrelevant_bound |
+  apply subst_w_Hyb_preserv_free_vars]; auto;
+[ rewrite <- subst_w_Hyb_neutral_free with (w0:=w_fresh) |
   constructor];
-[ apply subst_t_preserv_types_inner with (A:=A) |
-  apply subst_var_preserv_free_worlds]; auto;
-[ | rewrite <- double_emptyEquiv; auto];
+[ apply subst_t_Hyb_preserv_types_inner with (A:=A) |
+  apply subst_t_Hyb_preserv_free_worlds]; auto;
+[ | rewrite <- double_emptyEquiv_Hyb; auto];
 replace ((v_fresh, A) :: nil) with (nil ++ (v_fresh, A) :: nil) by auto;
-apply rename_w_preserv_types_new with
-  (G:= (w_fresh, (v_fresh, A)::nil) :: emptyEquiv G0);
-[ rewrite <- subst_order_irrelevant_bound |
-  rew_app]; auto; try PPermut_simpl; constructor.
+apply rename_w_Hyb_preserv_types_new with
+  (G:= (w_fresh, (v_fresh, A)::nil) :: emptyEquiv_Hyb G0);
+[ rewrite <- subst_Hyb_order_irrelevant_bound |
+  rew_app]; auto; try PPermut_Hyb_simpl; constructor.
 (* letdia #2 *)
 rewrite notin_union in *; destruct H0; destruct H1;
-unfold open_t in *; unfold open_w in *;
-rewrite subst_t_neutral_free with (v:=v_fresh);
-[ rewrite subst_order_irrelevant_bound |
-  apply subst_world_preserv_free_vars]; auto;
-[ rewrite <- subst_w_neutral_free with (w0:=w_fresh) |
+unfold open_t_Hyb in *; unfold open_w_Hyb in *;
+rewrite subst_t_Hyb_neutral_free with (v:=v_fresh);
+[ rewrite subst_Hyb_order_irrelevant_bound |
+  apply subst_w_Hyb_preserv_free_vars]; auto;
+[ rewrite <- subst_w_Hyb_neutral_free with (w0:=w_fresh) |
   constructor];
-[ eapply subst_t_preserv_types_outer with (A:=A) (G0:=G)
+[ eapply subst_t_Hyb_preserv_types_outer with (A:=A) (G0:=G)
   (Gamma':=Gamma) (w':=w) |
-  apply subst_var_preserv_free_worlds]; auto;
+  apply subst_t_Hyb_preserv_free_worlds]; auto;
 rew_app;
-assert ( emptyEquiv (G & (w0, nil)) = G & (w0, nil)) by
-   ( repeat rewrite emptyEquiv_rewrite; simpl;
-     apply emptyEquiv_permut_split_last in H4; rewrite H4; reflexivity);
+assert ( emptyEquiv_Hyb (G & (w0, nil)) = G & (w0, nil)) by
+   ( repeat rewrite emptyEquiv_Hyb_rewrite; simpl;
+     apply emptyEquiv_Hyb_permut_split_last in H4; rewrite H4; reflexivity);
 assert (Gamma = nil) by
-  ( apply emptyEquiv_permut_empty with (G:= (G & (w, Gamma)))
+  ( apply emptyEquiv_Hyb_permut_empty with (G:= (G & (w, Gamma)))
     (G':=G0) (w:=w); auto; apply Mem_last).
 subst; rew_app; rewrite <- H9 in HT0; auto.
-apply rename_w_preserv_types_outer with (G0:=G) (Gamma'':=(v_fresh,A) :: nil)
-      (Gamma':=Gamma) (G:=G & (w, Gamma) & (w_fresh, (v_fresh,A)::nil));
+apply rename_w_Hyb_preserv_types_outer with (G0:=G)
+  (Gamma'':=(v_fresh,A) :: nil)
+  (Gamma':=Gamma) (G:=G & (w, Gamma) & (w_fresh, (v_fresh,A)::nil));
 assert (G & (w, Gamma) & (w_fresh, (v_fresh, A) :: nil) ~=~
-  (w_fresh, (v_fresh, A) :: nil) :: emptyEquiv G0) by PPermut_simpl.
-rewrite H11; rewrite <- subst_order_irrelevant_bound;
+  (w_fresh, (v_fresh, A) :: nil) :: emptyEquiv_Hyb G0) by PPermut_Hyb_simpl.
+rewrite H11; rewrite <- subst_Hyb_order_irrelevant_bound;
 [eapply HT2; auto | constructor].
-PPermut_simpl; auto.
-PPermut_simpl.
+PPermut_Hyb_simpl; auto.
+PPermut_Hyb_simpl.
 (* letdia *)
-assert (exists w1, w1 \notin L_w \u free_worlds_LF N) as HF by apply Fresh;
-assert (exists v1, v1 \notin L_t \u free_vars_LF N) as HF2 by apply Fresh;
+assert (exists w1, w1 \notin L_w \u free_worlds_Hyb N) as HF by apply Fresh;
+assert (exists v1, v1 \notin L_t \u free_vars_Hyb N) as HF2 by apply Fresh;
 destruct HF as (w_fresh); destruct HF2 as (v_fresh);
 inversion HT; subst.
 (* letdia #1 *)
 rewrite notin_union in *; destruct H1; destruct H2;
-unfold open_t in *; unfold open_w in *;
-rewrite subst_t_neutral_free with (v:=v_fresh);
-[ rewrite subst_order_irrelevant_bound |
-  apply subst_world_preserv_free_vars]; auto;
-[ rewrite <- subst_w_neutral_free with (w0:=w_fresh) |
+unfold open_t_Hyb in *; unfold open_w_Hyb in *;
+rewrite subst_t_Hyb_neutral_free with (v:=v_fresh);
+[ rewrite subst_Hyb_order_irrelevant_bound |
+  apply subst_w_Hyb_preserv_free_vars]; auto;
+[ rewrite <- subst_w_Hyb_neutral_free with (w0:=w_fresh) |
   constructor];
-[ eapply subst_t_preserv_types_outer with (A:=A) (G0:=G) (w':=w)
+[ eapply subst_t_Hyb_preserv_types_outer with (A:=A) (G0:=G) (w':=w)
   (Gamma':=Gamma) |
- apply subst_var_preserv_free_worlds]; eauto;
+ apply subst_t_Hyb_preserv_free_worlds]; eauto;
 assert (Gamma = nil) by
-  (apply emptyEquiv_permut_empty with
+  (apply emptyEquiv_Hyb_permut_empty with
     (G:= (G & (w, Gamma))) (G':=G1) (w:=w); auto; apply Mem_last); subst;
 rew_app;
-assert ( emptyEquiv (G & (w0, nil)) = G & (w0, nil)) by
-   ( repeat rewrite emptyEquiv_rewrite; simpl;
-     apply emptyEquiv_permut_split_last in H0; rewrite H0; reflexivity);
+assert ( emptyEquiv_Hyb (G & (w0, nil)) = G & (w0, nil)) by
+   ( repeat rewrite emptyEquiv_Hyb_rewrite; simpl;
+     apply emptyEquiv_Hyb_permut_split_last in H0; rewrite H0; reflexivity);
 [ rewrite <- H5 in HT0 |
-  eapply rename_w_preserv_types_outer
+  eapply rename_w_Hyb_preserv_types_outer
     with (G:= (w_fresh, (v_fresh,A)::nil):: G & (w,nil))
          (Gamma'':=(v_fresh,A)::nil) (Gamma':=nil) (G0:=G)]; auto.
-rewrite <- subst_order_irrelevant_bound;
+rewrite <- subst_Hyb_order_irrelevant_bound;
 [ eapply HT2; eauto | constructor].
-PPermut_simpl.
+PPermut_Hyb_simpl.
 (* letdia #2 *)
 assert (Gamma = nil) by
-  (apply emptyEquiv_permut_empty with
+  (apply emptyEquiv_Hyb_permut_empty with
     (G:= (G & (w, Gamma))) (G':=G1) (w:=w); auto; apply Mem_last); subst.
-assert (w <> w0) by eauto with ok_bg_rew.
-assert (w1 <> w) by eauto with ok_bg_rew.
+assert (w <> w0) by eauto with ok_bg_hyb_rew.
+assert (w1 <> w) by eauto with ok_bg_hyb_rew.
 rewrite <- H0; rewrite notin_union in *; destruct H1; destruct H2;
-unfold open_t in *; unfold open_w in *; destruct (eq_var_dec w1 w0); subst.
+unfold open_t_Hyb in *; unfold open_w_Hyb in *; destruct (eq_var_dec w1 w0);
+subst.
 assert (G0  ~=~ G /\ Gamma0 *=* nil) by
-  (apply ok_Bg_impl_ppermut with (w:=w0); eauto);
+  (apply ok_Bg_Hyb_impl_ppermut with (w:=w0); eauto);
 destruct H12; symmetry in H13; apply permut_nil_eq in H13;
-rewrite subst_t_neutral_free with (v:=v_fresh);
-[ eapply subst_t_preserv_types_inner with (A:=A) |
-  apply subst_world_preserv_free_vars]; eauto;
-[ rewrite subst_order_irrelevant_bound |
-  assert ( emptyEquiv (G & (w, nil)) = G & (w, nil)) by
-    ( repeat rewrite emptyEquiv_rewrite; simpl;
-      apply emptyEquiv_permut_split_last in H0; rewrite H0; reflexivity)];
-[ rewrite <- subst_w_neutral_free with (w0:=w_fresh) |
+rewrite subst_t_Hyb_neutral_free with (v:=v_fresh);
+[ eapply subst_t_Hyb_preserv_types_inner with (A:=A) |
+  apply subst_w_Hyb_preserv_free_vars]; eauto;
+[ rewrite subst_Hyb_order_irrelevant_bound |
+  assert ( emptyEquiv_Hyb (G & (w, nil)) = G & (w, nil)) by
+    ( repeat rewrite emptyEquiv_Hyb_rewrite; simpl;
+      apply emptyEquiv_Hyb_permut_split_last in H0; rewrite H0; reflexivity)];
+[ rewrite <- subst_w_Hyb_neutral_free with (w0:=w_fresh) |
   constructor | ]; auto;
 [ replace ((v_fresh,A)::nil) with (nil++(v_fresh,A)::nil) by auto |
-  apply subst_var_preserv_free_worlds | ]; auto.
-apply rename_w_preserv_types_new with
+  apply subst_t_Hyb_preserv_free_worlds | ]; auto.
+apply rename_w_Hyb_preserv_types_new with
   (G:= (w_fresh, (v_fresh,A)::nil) :: G0 & (w, nil));
-[ rewrite <- subst_order_irrelevant_bound; try constructor; subst |
+[ rewrite <- subst_Hyb_order_irrelevant_bound; try constructor; subst |
   rew_app; eauto].
 rewrite H12; eapply HT2; auto.
-PPermut_simpl.
+PPermut_Hyb_simpl.
 rewrite H14; rewrite <- H12; subst; auto.
 assert (Gamma0 = nil) by
-  ( apply emptyEquiv_permut_empty with (G:= (G0 & (w1, Gamma0)))
+  ( apply emptyEquiv_Hyb_permut_empty with (G:= (G0 & (w1, Gamma0)))
       (G':=G & (w0, nil)) (w:=w1); auto;
-    assert (emptyEquiv G = G) by
-      (apply emptyEquiv_permut_split_last with (C:=(w, nil)) (H:=G1); auto);
-    [ rewrite emptyEquiv_rewrite; simpl | apply Mem_last ]; rewrite H12; auto);
-subst; assert (exists Gamma'', exists GH, exists GT,
+    assert (emptyEquiv_Hyb G = G) by
+      (apply emptyEquiv_Hyb_permut_split_last with (C:=(w, nil)) (H:=G1); auto);
+    [ rewrite emptyEquiv_Hyb_rewrite; simpl | apply Mem_last ];
+rewrite H12; auto); subst; assert (exists Gamma'', exists GH, exists GT,
   Gamma'' *=* nil /\ G = GH & (w1, Gamma'') ++ GT) by
-  ( apply PPermut_split_neq with (w:=w0) (G':=G0) (Gamma:=nil);
+  ( apply PPermut_Hyb_split_neq with (w:=w0) (G':=G0) (Gamma:=nil);
     [ symmetry | right; intro; subst; elim n]; auto);
 destruct H12 as (Gamma'', (GH, (GT, (H12a, H12b))));
 symmetry in H12a; apply permut_nil_eq in H12a; subst;
-rewrite subst_t_neutral_free with (v:=v_fresh);
-[ apply subst_t_preserv_types_outer with (A:=A) (G0 :=GH ++ GT & (w, nil))
+rewrite subst_t_Hyb_neutral_free with (v:=v_fresh);
+[ apply subst_t_Hyb_preserv_types_outer with (A:=A) (G0 :=GH ++ GT & (w, nil))
           (G := GH ++ GT & (w,nil) & (w1, (v_fresh, A) :: nil))
        (G' := GH ++ GT & (w,nil) & (w0, nil)) (w' :=w1) (Gamma':=nil) |
-  apply subst_world_preserv_free_vars]; auto; subst; rew_app; auto.
+  apply subst_w_Hyb_preserv_free_vars]; auto; subst; rew_app; auto.
 assert (G0 & (w, nil) ~=~ GH ++ GT & (w,nil) & (w0, nil)) by
   ( transitivity ((GH++GT & (w0,nil) &(w, nil))); auto;
     assert (G0 & (w1, nil) ~=~  (GH ++ GT & (w0, nil) & (w1, nil))) by
       (transitivity ((GH & (w1, nil) ++ GT) & (w0, nil)); rew_app in *; auto);
     assert (G0 ~=~ GH ++ GT & (w0, nil)) by
-      (apply PPermut_last_rev_simpl with (a:=(w1,nil)); rew_app in *; auto);
-  try PPermut_simpl;
+      (apply PPermut_Hyb_last_rev_simpl with (a:=(w1,nil)); rew_app in *; auto);
+  try PPermut_Hyb_simpl;
   rewrite H13; rew_app; auto); rew_app in *; rewrite <- H12.
-assert (emptyEquiv G0 = G0) by
+assert (emptyEquiv_Hyb G0 = G0) by
 ( assert (G0 ~=~ GH ++ GT & (w0, nil)) by
-    ( apply PPermut_last_rev_simpl with (a:=(w, nil));
+    ( apply PPermut_Hyb_last_rev_simpl with (a:=(w, nil));
       transitivity (GH ++ GT & (w, nil) & (w0, nil)); rew_app in *; auto);
-  apply emptyEquiv_permut_split_last with (C:=(w1, nil)) (H := (w0, nil) ::
+  apply emptyEquiv_Hyb_permut_split_last with (C:=(w1, nil)) (H := (w0, nil) ::
     GH & (w1, nil) ++ GT);
-  assert (emptyEquiv ((w0, nil) :: GH & (w1, nil) ++ GT) = ((w0, nil) ::
+  assert (emptyEquiv_Hyb ((w0, nil) :: GH & (w1, nil) ++ GT) = ((w0, nil) ::
     GH & (w1, nil) ++ GT)) by
-  ( apply emptyEquiv_permut_split_last with (C:=(w, nil)) (H:= (w0,nil)::G1);
-    simpl; rewrite <- H0; rew_app; symmetry; auto);
+  ( apply emptyEquiv_Hyb_permut_split_last with (C:=(w, nil))
+    (H:= (w0,nil)::G1); simpl; rewrite <- H0; rew_app; symmetry; auto);
   rewrite H13; rewrite H14; rew_app;
-  transitivity (GH ++ (w0, nil) :: (w1, nil)::GT); auto; PPermut_simpl);
-rewrite emptyEquiv_rewrite; simpl; rewrite H13; auto.
-rewrite subst_order_irrelevant_bound;
-[ rewrite <- subst_w_neutral_free with (w0:=w_fresh) | constructor];
-[ apply rename_w_preserv_types_outer
+  transitivity (GH ++ (w0, nil) :: (w1, nil)::GT); auto; PPermut_Hyb_simpl);
+rewrite emptyEquiv_Hyb_rewrite; simpl; rewrite H13; auto.
+rewrite subst_Hyb_order_irrelevant_bound;
+[ rewrite <- subst_w_Hyb_neutral_free with (w0:=w_fresh) | constructor];
+[ apply rename_w_Hyb_preserv_types_outer
     with (G0 := GH ++ GT & (w,nil))
          (G := (w_fresh, (v_fresh, A) :: nil) :: (GH & (w1, nil) ++ GT) &
            (w, nil))
          (Gamma':=nil)
          (Gamma'':=(v_fresh, A)::nil) |
-  apply subst_var_preserv_free_worlds]; auto.
-rewrite <- subst_order_irrelevant_bound;
+  apply subst_t_Hyb_preserv_free_worlds]; auto.
+rewrite <- subst_Hyb_order_irrelevant_bound;
 [eapply HT2; eauto | constructor].
-PPermut_simpl.
-PPermut_simpl.
+PPermut_Hyb_simpl.
+PPermut_Hyb_simpl.
 (* letdia_step *)
 destruct (eq_var_dec w0 w); subst.
-eapply ok_Bg_first_last_neq in Ok_Bg;
+eapply ok_Bg_Hyb_first_last_neq in Ok_Bg;
 elim Ok_Bg; auto.
 assert (Gamma = nil) by
-  ( apply emptyEquiv_permut_empty with (G:= (G & (w, Gamma))) (G':=G1) (w:=w);
-    auto; apply Mem_last);
+  ( apply emptyEquiv_Hyb_permut_empty with (G:= (G & (w, Gamma))) (G':=G1)
+    (w:=w); auto; apply Mem_last);
 subst;
 apply IHHT with (G0:=G & (w0,nil)) (w1:=w); auto;
-assert (emptyEquiv G = G) by
-  (apply emptyEquiv_permut_split_last with (C:=(w,nil)) (H:=G1); auto);
-rewrite emptyEquiv_rewrite; simpl; rewrite H1; reflexivity.
+assert (emptyEquiv_Hyb G = G) by
+  (apply emptyEquiv_Hyb_permut_split_last with (C:=(w,nil)) (H:=G1); auto);
+rewrite emptyEquiv_Hyb_rewrite; simpl; rewrite H1; reflexivity.
 Qed.
 
-Close Scope label_free_is5_scope.
+Close Scope hybrid_is5_scope.
 Close Scope is5_scope.
 Close Scope permut_scope.
