Hybrid/Substitution.v
@@ -20,24 +20,24 @@ Term substitution
   We assume here that the term M0 is locally closed, that is it does not
   require any shifts.
 *)
-Fixpoint subst_t (M0: te_LF) (v0: vte) (N0: te_LF) :=
+Fixpoint subst_t_Hyb (M0: te_Hyb) (v0: vte) (N0: te_Hyb) :=
 match N0 with
-| hyp_LF v =>
+| hyp_Hyb v =>
     if (eq_vte_dec v v0) then M0 else N0
-| lam_LF A M =>
-    lam_LF A ([M0 // shift_vte v0] M)
-| appl_LF M N =>
-    appl_LF ([M0//v0]M) ([M0//v0]N)
-| box_LF M =>
-    box_LF ([M0//v0]M)
-| unbox_fetch_LF w M =>
-    unbox_fetch_LF w ([M0//v0]M)
-| get_here_LF w M =>
-    get_here_LF w ([M0//v0]M)
-| letdia_get_LF w M N =>
-    letdia_get_LF w ([M0//v0]M) ([M0//shift_vte v0]N)
+| lam_Hyb A M =>
+    lam_Hyb A ([M0 // shift_vte v0] M)
+| appl_Hyb M N =>
+    appl_Hyb ([M0//v0]M) ([M0//v0]N)
+| box_Hyb M =>
+    box_Hyb ([M0//v0]M)
+| unbox_fetch_Hyb w M =>
+    unbox_fetch_Hyb w ([M0//v0]M)
+| get_here_Hyb w M =>
+    get_here_Hyb w ([M0//v0]M)
+| letdia_get_Hyb w M N =>
+    letdia_get_Hyb w ([M0//v0]M) ([M0//shift_vte v0]N)
 end
-where " [ M // v ] N " := (subst_t M v N) : label_free_is5_scope.
+where " [ M // v ] N " := (subst_t_Hyb M v N) : hybrid_is5_scope.
 
 
 (*
@@ -45,36 +45,36 @@ World substitution
   Replaces one world with another. Since both of the worlds can be free or
   bound, we need to use shift operation on both sides for box and letdia cases.
 *)
-Fixpoint subst_w (w1: vwo) (w2: vwo) (M0: te_LF) :=
+Fixpoint subst_w_Hyb (w1: vwo) (w2: vwo) (M0: te_Hyb) :=
 match M0 with
-| hyp_LF n => hyp_LF n
-| lam_LF A M => lam_LF A ({{w1//w2}}M)
-| appl_LF M N => appl_LF ({{w1//w2}}M) ({{w1//w2}}N)
-| box_LF M =>
-  box_LF ({{ shift_vwo w1 // shift_vwo w2 }} M)
-| unbox_fetch_LF w M =>
+| hyp_Hyb n => hyp_Hyb n
+| lam_Hyb A M => lam_Hyb A ({{w1//w2}}M)
+| appl_Hyb M N => appl_Hyb ({{w1//w2}}M) ({{w1//w2}}N)
+| box_Hyb M =>
+  box_Hyb ({{ shift_vwo w1 // shift_vwo w2 }} M)
+| unbox_fetch_Hyb w M =>
   let w' := if (eq_vwo_dec w w2) then w1 else w in
-    unbox_fetch_LF w' ({{w1//w2}} M)
-| get_here_LF w M =>
+    unbox_fetch_Hyb w' ({{w1//w2}} M)
+| get_here_Hyb w M =>
   let w' := if (eq_vwo_dec w w2) then w1 else w in
-    get_here_LF w' ({{w1//w2}}M)
-| letdia_get_LF w M N =>
+    get_here_Hyb w' ({{w1//w2}}M)
+| letdia_get_Hyb w M N =>
   let w' := if (eq_vwo_dec w w2) then w1 else w in
-    letdia_get_LF w' ({{w1//w2}} M) ({{shift_vwo w1 // shift_vwo w2}} N)
+    letdia_get_Hyb w' ({{w1//w2}} M) ({{shift_vwo w1 // shift_vwo w2}} N)
 end
-where " {{ w1 // w2 }} M " := (subst_w w1 w2 M) : label_free_is5_scope.
+where " {{ w1 // w2 }} M " := (subst_w_Hyb w1 w2 M) : hybrid_is5_scope.
 
 
 (* Opening is defined in terms of substitution *)
 
-Definition open_t (M: te_LF) (t: te_LF) := subst_t t (bte 0) M.
+Definition open_t_Hyb (M: te_Hyb) (t: te_Hyb) := subst_t_Hyb t (bte 0) M.
 
-Definition open_w M w := subst_w w (bwo 0) M.
+Definition open_w_Hyb M w := subst_w_Hyb w (bwo 0) M.
 
-Notation " M '^t^' t " := (open_t M t) (at level 67) : label_free_is5_scope.
-Notation " M ^w^ w  " := (open_w M w) (at level 67) : label_free_is5_scope.
+Notation " M '^t^' t " := (open_t_Hyb M t) (at level 67) : hybrid_is5_scope.
+Notation " M ^w^ w  " := (open_w_Hyb M w) (at level 67) : hybrid_is5_scope.
 
-Open Scope label_free_is5_scope.
+Open Scope hybrid_is5_scope.
 
 
 (*
@@ -82,10 +82,10 @@ List substitution
   Substituting a list of terms for bound variables in term, starting
   from a given index.
 *)
-Fixpoint list_t_subst (L: list te_LF) (n: nat) (M: te_LF) :=
+Fixpoint list_t_subst_Hyb (L: list te_Hyb) (n: nat) (M: te_Hyb) :=
 match L with
 | nil => M
-| t :: L' => [t // bte n] (list_t_subst L' (S n) M)
+| t :: L' => [t // bte n] (list_t_subst_Hyb L' (S n) M)
 end.
 
 
@@ -101,7 +101,7 @@ Simplify substitution in special cases
 *)
 
 
-Lemma subst_w_id:
+Lemma subst_w_Hyb_id:
 forall M w,
   {{w // w}} M = M.
 induction M; intros; simpl in *;
@@ -110,9 +110,9 @@ rewrite IHM || (rewrite IHM1; try rewrite IHM2);
 auto.
 Qed.
 
-Lemma subst_w_2_step_id:
+Lemma subst_w_Hyb_2_step_id:
 forall M w n
-  (HT: w \notin free_worlds_LF M),
+  (HT: w \notin free_worlds_Hyb M),
   {{bwo n//fwo w}}({{fwo w//bwo n}}M) = M.
 induction M; intros; simpl in *;
 repeat case_if; subst; auto;
@@ -124,9 +124,9 @@ Qed.
 
 (* Free variable for which we substitute does not occur in the term *)
 
-Lemma closed_subst_w_free:
+Lemma closed_subst_w_Hyb_free:
 forall M w0 w
-  (H_lc: w0 \notin free_worlds_LF M),
+  (H_lc: w0 \notin free_worlds_Hyb M),
   {{ w // fwo w0}} M  = M.
 induction M; intros; simpl in *;
 repeat case_if; auto;
@@ -135,9 +135,9 @@ rewrite IHM || (rewrite IHM1; try rewrite IHM2); auto;
 destruct H_lc as (Neq, H_lc); elim Neq) || destruct v; auto.
 Qed.
 
-Lemma closed_subst_t_free:
+Lemma closed_subst_t_Hyb_free:
 forall M v0 N
-  (H_lc: v0 \notin free_vars_LF N),
+  (H_lc: v0 \notin free_vars_Hyb N),
   [M // fte v0] N = N.
 induction N; intros; simpl in *;
 repeat case_if;
@@ -150,9 +150,9 @@ Qed.
 (* Term is closed and we try to substitute for bound variable *)
 
 
-Lemma closed_subst_w_bound:
+Lemma closed_subst_w_Hyb_bound:
 forall M w0 w n
-  (H_lc: lc_w_n_LF n M),
+  (H_lc: lc_w_n_Hyb n M),
   {{ w // bwo w0}} M  = M.
 induction M; intros; simpl in *;
 repeat case_if; auto;
@@ -160,9 +160,9 @@ inversion H_lc; subst;
 erewrite IHM || (erewrite IHM1; try erewrite IHM2); eauto.
 Qed.
 
-Lemma closed_subst_t_bound:
+Lemma closed_subst_t_Hyb_bound:
 forall N M v0 n
-  (H_lc: lc_t_n_LF n N),
+  (H_lc: lc_t_n_Hyb n N),
   v0 >= n -> [M // bte v0] N = N.
 induction N; intros; simpl in *;
 repeat case_if; inversion H_lc; subst;
@@ -175,7 +175,7 @@ Qed.
 
 (* Properties of substitution: commutativity *)
 
-Lemma subst_w_comm:
+Lemma subst_w_Hyb_comm:
 forall M w w' w'' n
   (Neq: w'' <> w),
   {{fwo w'//fwo w''}}({{fwo w//bwo n}}M) =
@@ -186,20 +186,20 @@ rewrite IHM || (rewrite IHM1; try rewrite IHM2);
 auto.
 Qed.
 
-Lemma subst_t_comm:
+Lemma subst_t_Hyb_comm:
 forall M v v' n N
-  (Lc: lc_t_LF N),
+  (Lc: lc_t_Hyb N),
   v <> v' ->
-  [ N // fte v] ([ hyp_LF (fte v') // bte n] M) =
-  [hyp_LF (fte v') // bte n] ([N // fte v] M).
+  [ N // fte v] ([ hyp_Hyb (fte v') // bte n] M) =
+  [hyp_Hyb (fte v') // bte n] ([N // fte v] M).
 induction M; intros; simpl;
 [ repeat (case_if; simpl); auto;
-  erewrite closed_subst_t_bound; eauto; omega | | | | | |];
+  erewrite closed_subst_t_Hyb_bound; eauto; omega | | | | | |];
 try (rewrite IHM; auto);
 try (rewrite IHM1; try rewrite IHM2; auto);
 repeat (case_if; simpl); subst; simpl;
 auto;
-erewrite closed_subst_t_bound;
+erewrite closed_subst_t_Hyb_bound;
 eauto;
 replace n with (0+n) by omega;
 apply closed_t_addition; auto.
@@ -208,9 +208,9 @@ Qed.
 
 (* Properties of substitution: expansion with neutral element *)
 
-Lemma subst_w_neutral_free:
+Lemma subst_w_Hyb_neutral_free:
 forall M w w' w0
-  (HT: w0 \notin free_worlds_LF M),
+  (HT: w0 \notin free_worlds_Hyb M),
   {{w//fwo w0}}({{fwo w0// w'}}M) = {{w//w'}}M.
 induction M; intros; simpl in *;
 repeat case_if; subst; simpl; auto;
@@ -220,19 +220,19 @@ auto;
 assert (w0 <> w0) as Neq by eauto; elim Neq; auto.
 Qed.
 
-Lemma subst_t_neutral_free:
+Lemma subst_t_Hyb_neutral_free:
 forall M v n N
-  (HT: v \notin free_vars_LF M),
-  [ N // bte n] M = [N // fte v] [hyp_LF (fte v) // bte n] M.
+  (HT: v \notin free_vars_Hyb M),
+  [ N // bte n] M = [N // fte v] [hyp_Hyb (fte v) // bte n] M.
 induction M; intros; simpl in *;
 try (erewrite IHM || (erewrite IHM1; try erewrite IHM2); eauto);
 repeat (case_if; simpl); subst; auto;
 assert (v0 <> v0) as Neq by eauto; elim Neq; auto.
 Qed.
 
-Lemma subst_w_neutral_bound:
+Lemma subst_w_Hyb_neutral_bound:
 forall M n
-  (HT: lc_w_n_LF n M),
+  (HT: lc_w_n_Hyb n M),
   forall m w w',
     m >= n -> {{w//bwo m}}({{bwo m// w'}}M) = {{w//w'}}M.
 intros M n HT; induction HT; intros; simpl in *; auto.
@@ -246,9 +246,9 @@ Qed.
 
 (* With two different types of substitution, the order does not matter *)
 
-Lemma subst_order_irrelevant_bound:
+Lemma subst_Hyb_order_irrelevant_bound:
 forall N w M v m
-  (HT_M: lc_w_LF M),
+  (HT_M: lc_w_Hyb M),
     [M // v ] ({{w // bwo m}} N)  =
     {{w // bwo m}} ([M // v ] N).
 induction N; intros; simpl in *;
@@ -256,12 +256,12 @@ repeat case_if; simpl;
 unfold shift_vte in *; unfold shift_vwo in *;
 try destruct v; try destruct w; auto;
 try rewrite IHN; try (rewrite IHN1; try rewrite IHN2);
-auto; erewrite closed_subst_w_bound; eauto.
+auto; erewrite closed_subst_w_Hyb_bound; eauto.
 Qed.
 
-Lemma subst_order_irrelevant_free:
+Lemma subst_Hyb_order_irrelevant_free:
 forall N w w' M v
-  (HT_M: w' \notin (free_worlds_LF M)),
+  (HT_M: w' \notin (free_worlds_Hyb M)),
     [M // v ] ({{w // fwo w'}} N)  =
     {{w // fwo w'}} ([M // v ] N).
 induction N; intros; simpl in *;
@@ -269,7 +269,7 @@ repeat case_if; simpl;
 unfold shift_vwo in *;
 try destruct c; try destruct v; auto;
 try rewrite IHN; try (rewrite IHN1; try rewrite IHN2);
-auto; rewrite closed_subst_w_free; auto.
+auto; rewrite closed_subst_w_Hyb_free; auto.
 Qed.
 
 
@@ -278,22 +278,22 @@ Qed.
    of the other type.
 *)
 
-Lemma subst_var_preserv_free_worlds:
+Lemma subst_t_Hyb_preserv_free_worlds:
 forall N v k w,
-  w \notin free_worlds_LF N ->
-  w \notin free_worlds_LF [ hyp_LF (fte v) // bte k ] N.
+  w \notin free_worlds_Hyb N ->
+  w \notin free_worlds_Hyb [ hyp_Hyb (fte v) // bte k ] N.
 induction N; intros; simpl in *;
 repeat case_if;try destruct v;
 simpl; auto.
 Qed.
 
-Lemma subst_world_preserv_free_vars:
+Lemma subst_w_Hyb_preserv_free_vars:
 forall N w w' v,
-  v \notin free_vars_LF N ->
-  v \notin free_vars_LF {{w // w'}} N.
+  v \notin free_vars_Hyb N ->
+  v \notin free_vars_Hyb {{w // w'}} N.
 induction N; intros; simpl in *;
 repeat case_if; try destruct c;
 simpl; auto.
 Qed.
 
-Close Scope label_free_is5_scope.
+Close Scope hybrid_is5_scope.
