Hybrid/Syntax.v
@@ -15,43 +15,43 @@ Terms in label-free IS5 system:
   * using diamond expression (possibly the diamond itself is from a
   different world)
 *)
-Inductive te_LF :=
-| hyp_LF: vte -> te_LF
-| lam_LF: ty -> te_LF -> te_LF
-| appl_LF: te_LF -> te_LF -> te_LF
-| box_LF: te_LF -> te_LF
-| unbox_fetch_LF: vwo -> te_LF -> te_LF
-| get_here_LF: vwo -> te_LF -> te_LF
-| letdia_get_LF: vwo -> te_LF -> te_LF -> te_LF
+Inductive te_Hyb :=
+| hyp_Hyb: vte -> te_Hyb
+| lam_Hyb: ty -> te_Hyb -> te_Hyb
+| appl_Hyb: te_Hyb -> te_Hyb -> te_Hyb
+| box_Hyb: te_Hyb -> te_Hyb
+| unbox_fetch_Hyb: vwo -> te_Hyb -> te_Hyb
+| get_here_Hyb: vwo -> te_Hyb -> te_Hyb
+| letdia_get_Hyb: vwo -> te_Hyb -> te_Hyb -> te_Hyb
 .
 
 
 (* Calculate set of free worlds used in term M *)
-Fixpoint free_worlds_LF (M: te_LF) : fset var :=
+Fixpoint free_worlds_Hyb (M: te_Hyb) : fset var :=
 match M with
-| hyp_LF _ => \{}
-| lam_LF _ M => free_worlds_LF M
-| appl_LF M N => free_worlds_LF M \u free_worlds_LF N
-| box_LF M => free_worlds_LF M
-| unbox_fetch_LF (fwo w) M => \{w} \u free_worlds_LF M
-| unbox_fetch_LF _ M => free_worlds_LF M
-| get_here_LF (fwo w) M => \{w} \u free_worlds_LF M
-| get_here_LF _ M => free_worlds_LF M
-| letdia_get_LF (fwo w) M N => \{w} \u free_worlds_LF M \u free_worlds_LF N
-| letdia_get_LF _ M N => free_worlds_LF M \u free_worlds_LF N
+| hyp_Hyb _ => \{}
+| lam_Hyb _ M => free_worlds_Hyb M
+| appl_Hyb M N => free_worlds_Hyb M \u free_worlds_Hyb N
+| box_Hyb M => free_worlds_Hyb M
+| unbox_fetch_Hyb (fwo w) M => \{w} \u free_worlds_Hyb M
+| unbox_fetch_Hyb _ M => free_worlds_Hyb M
+| get_here_Hyb (fwo w) M => \{w} \u free_worlds_Hyb M
+| get_here_Hyb _ M => free_worlds_Hyb M
+| letdia_get_Hyb (fwo w) M N => \{w} \u free_worlds_Hyb M \u free_worlds_Hyb N
+| letdia_get_Hyb _ M N => free_worlds_Hyb M \u free_worlds_Hyb N
 end.
 
 (* Calculate set of free variables used in term M *)
-Fixpoint free_vars_LF (M: te_LF) : fset var :=
+Fixpoint free_vars_Hyb (M: te_Hyb) : fset var :=
 match M with
-| hyp_LF (fte v) => \{v}
-| hyp_LF (bte _) => \{}
-| lam_LF _ M => free_vars_LF M
-| appl_LF M N => free_vars_LF M \u free_vars_LF N
-| box_LF M => free_vars_LF M
-| unbox_fetch_LF _ M => free_vars_LF M
-| get_here_LF _ M => free_vars_LF M
-| letdia_get_LF _ M N => free_vars_LF M \u free_vars_LF N
+| hyp_Hyb (fte v) => \{v}
+| hyp_Hyb (bte _) => \{}
+| lam_Hyb _ M => free_vars_Hyb M
+| appl_Hyb M N => free_vars_Hyb M \u free_vars_Hyb N
+| box_Hyb M => free_vars_Hyb M
+| unbox_fetch_Hyb _ M => free_vars_Hyb M
+| get_here_Hyb _ M => free_vars_Hyb M
+| letdia_get_Hyb _ M N => free_vars_Hyb M \u free_vars_Hyb N
 end.
 
 
@@ -60,64 +60,64 @@ Property: term is locally closed
  This means that there are no bound variables.
 *)
 
-Inductive lc_t_n_LF : nat -> te_LF -> Prop :=
- | lct_hyp_bte_LF: forall v n, n > v -> lc_t_n_LF n (hyp_LF (bte v))
- | lct_hyp_fte_LF: forall v n, lc_t_n_LF n (hyp_LF (fte v))
- | lct_lam_LF: forall M t n,
-     lc_t_n_LF (S n) M ->
-     lc_t_n_LF n (lam_LF t M)
- | lct_appl_LF: forall M N n,
-     lc_t_n_LF n M -> lc_t_n_LF n N ->
-     lc_t_n_LF n (appl_LF M N)
- | lct_box_LF: forall M n,
-     lc_t_n_LF n M ->
-     lc_t_n_LF n (box_LF M)
- | lct_unbox_fetch_LF: forall M w n,
-     lc_t_n_LF n M ->
-     lc_t_n_LF n (unbox_fetch_LF (fwo w) M)
- | lct_get_here_LF: forall M w n,
-     lc_t_n_LF n M ->
-     lc_t_n_LF n (get_here_LF (fwo w) M)
- | lct_letdia_get_LF: forall M N w n,
-     lc_t_n_LF (S n) N -> lc_t_n_LF n M ->
-     lc_t_n_LF n (letdia_get_LF (fwo w) M N)
+Inductive lc_t_n_Hyb : nat -> te_Hyb -> Prop :=
+ | lct_hyp_bte_Hyb: forall v n, n > v -> lc_t_n_Hyb n (hyp_Hyb (bte v))
+ | lct_hyp_fte_Hyb: forall v n, lc_t_n_Hyb n (hyp_Hyb (fte v))
+ | lct_lam_Hyb: forall M t n,
+     lc_t_n_Hyb (S n) M ->
+     lc_t_n_Hyb n (lam_Hyb t M)
+ | lct_appl_Hyb: forall M N n,
+     lc_t_n_Hyb n M -> lc_t_n_Hyb n N ->
+     lc_t_n_Hyb n (appl_Hyb M N)
+ | lct_box_Hyb: forall M n,
+     lc_t_n_Hyb n M ->
+     lc_t_n_Hyb n (box_Hyb M)
+ | lct_unbox_fetch_Hyb: forall M w n,
+     lc_t_n_Hyb n M ->
+     lc_t_n_Hyb n (unbox_fetch_Hyb (fwo w) M)
+ | lct_get_here_Hyb: forall M w n,
+     lc_t_n_Hyb n M ->
+     lc_t_n_Hyb n (get_here_Hyb (fwo w) M)
+ | lct_letdia_get_Hyb: forall M N w n,
+     lc_t_n_Hyb (S n) N -> lc_t_n_Hyb n M ->
+     lc_t_n_Hyb n (letdia_get_Hyb (fwo w) M N)
 .
 
-Definition lc_t_LF M := lc_t_n_LF 0 M.
+Definition lc_t_Hyb M := lc_t_n_Hyb 0 M.
 
 
-Inductive lc_w_n_LF: nat -> te_LF -> Prop :=
-| lcw_hyp_LF: forall v n, lc_w_n_LF n (hyp_LF v)
-| lcw_lam_LF: forall t M n,
-    lc_w_n_LF n M ->
-    lc_w_n_LF n (lam_LF t M)
-| lcw_appl_LF: forall M N n,
-    lc_w_n_LF n M -> lc_w_n_LF n N ->
-    lc_w_n_LF n (appl_LF M N)
-| lcw_box_LF: forall M n,
-    lc_w_n_LF (S n) M ->
-    lc_w_n_LF n (box_LF M)
-| lcw_unbox_fetch_LF: forall M w n,
-    lc_w_n_LF n M ->
-    lc_w_n_LF n (unbox_fetch_LF (fwo w) M)
-| lcw_get_here_LF: forall M w n,
-    lc_w_n_LF n M ->
-    lc_w_n_LF n (get_here_LF (fwo w) M)
-| lcw_letdia_get_LF: forall M N w n,
-    lc_w_n_LF (S n) N ->
-    lc_w_n_LF n M ->
-    lc_w_n_LF n (letdia_get_LF (fwo w) M N)
+Inductive lc_w_n_Hyb: nat -> te_Hyb -> Prop :=
+| lcw_hyp_Hyb: forall v n, lc_w_n_Hyb n (hyp_Hyb v)
+| lcw_lam_Hyb: forall t M n,
+    lc_w_n_Hyb n M ->
+    lc_w_n_Hyb n (lam_Hyb t M)
+| lcw_appl_Hyb: forall M N n,
+    lc_w_n_Hyb n M -> lc_w_n_Hyb n N ->
+    lc_w_n_Hyb n (appl_Hyb M N)
+| lcw_box_Hyb: forall M n,
+    lc_w_n_Hyb (S n) M ->
+    lc_w_n_Hyb n (box_Hyb M)
+| lcw_unbox_fetch_Hyb: forall M w n,
+    lc_w_n_Hyb n M ->
+    lc_w_n_Hyb n (unbox_fetch_Hyb (fwo w) M)
+| lcw_get_here_Hyb: forall M w n,
+    lc_w_n_Hyb n M ->
+    lc_w_n_Hyb n (get_here_Hyb (fwo w) M)
+| lcw_letdia_get_Hyb: forall M N w n,
+    lc_w_n_Hyb (S n) N ->
+    lc_w_n_Hyb n M ->
+    lc_w_n_Hyb n (letdia_get_Hyb (fwo w) M N)
 .
 
-Definition lc_w_LF M := lc_w_n_LF 0 M.
+Definition lc_w_Hyb M := lc_w_n_Hyb 0 M.
 
 
 (*** Properties ***)
 
 
 (* For each pair of contexts, they are either equivalent or not. *)
-Theorem permut_context_LF_dec:
-forall (c1 c2: Context_LF),
+Theorem permut_context_Hyb_dec:
+forall (c1 c2: ctx_Hyb),
   {  permut (snd c1) (snd c2) /\ (fst c1) = (fst c2)} +
   { ~permut (snd c1) (snd c2) \/ (fst c1) <> (fst c2)}.
 intros; destruct c1 as (w, a); destruct c2 as (w', a');
@@ -129,28 +129,28 @@ apply eq_var_dec.
 Qed.
 
 
-(* Propagation of lc_*_n_LF property *)
+(* Propagation of lc_*_n_Hyb property *)
 
 Lemma closed_w_succ:
 forall M n,
-  lc_w_n_LF n M -> lc_w_n_LF (S n) M.
+  lc_w_n_Hyb n M -> lc_w_n_Hyb (S n) M.
 intros; generalize dependent n;
 induction M; intros; inversion H; subst;
-eauto using lc_w_n_LF.
+eauto using lc_w_n_Hyb.
 Qed.
 
 Lemma closed_t_succ:
 forall M n,
-  lc_t_n_LF n M -> lc_t_n_LF (S n) M.
+  lc_t_n_Hyb n M -> lc_t_n_Hyb (S n) M.
 intros; generalize dependent n;
 induction M; intros; inversion H; subst;
-eauto using lc_t_n_LF.
+eauto using lc_t_n_Hyb.
 Qed.
 
 
 Lemma closed_w_addition:
 forall M n m,
-  lc_w_n_LF n M -> lc_w_n_LF (n + m) M.
+  lc_w_n_Hyb n M -> lc_w_n_Hyb (n + m) M.
 intros; induction m;
 [ replace (n+0) with n by auto |
   replace (n+ S m) with (S (n+m)) by auto] ;
@@ -160,7 +160,7 @@ Qed.
 
 Lemma closed_t_addition:
 forall M n m,
-  lc_t_n_LF n M -> lc_t_n_LF (n + m) M.
+  lc_t_n_Hyb n M -> lc_t_n_Hyb (n + m) M.
 intros; induction m;
 [ replace (n+0) with n by auto |
   replace (n + S m) with (S (n+m)) by auto] ;
